<?xml version="1.0"?>
<rdf:RDF xmlns="http://www.semanticweb.org/cra/ontologies/AgriWaterMgmt/"
     xml:base="http://www.semanticweb.org/cra/ontologies/AgriWaterMgmt/"
     xmlns:owl="http://www.w3.org/2002/07/owl#"
     xmlns:rdf="http://www.w3.org/1999/02/22-rdf-syntax-ns#"
     xmlns:xml="http://www.w3.org/XML/1998/namespace"
     xmlns:xsd="http://www.w3.org/2001/XMLSchema#"
     xmlns:rdfs="http://www.w3.org/2000/01/rdf-schema#"
     xmlns:AgriWaterMgmt="http://www.semanticweb.org/cra/ontologies/AgriWaterMgmt#">
    <owl:Ontology rdf:about="http://www.semanticweb.org/cra/ontologies/AgriWaterMgmt"/>
    


    <!-- 
    ///////////////////////////////////////////////////////////////////////////////////////
    //
    // Object Properties
    //
    ///////////////////////////////////////////////////////////////////////////////////////
     -->

    


    <!-- http://www.semanticweb.org/cra/ontologies/AgriWaterMgmt#allocates -->

    <owl:ObjectProperty rdf:about="http://www.semanticweb.org/cra/ontologies/AgriWaterMgmt#allocates"/>
    


    <!-- http://www.semanticweb.org/cra/ontologies/AgriWaterMgmt#causes -->

    <owl:ObjectProperty rdf:about="http://www.semanticweb.org/cra/ontologies/AgriWaterMgmt#causes"/>
    


    <!-- http://www.semanticweb.org/cra/ontologies/AgriWaterMgmt#controls -->

    <owl:ObjectProperty rdf:about="http://www.semanticweb.org/cra/ontologies/AgriWaterMgmt#controls"/>
    


    <!-- http://www.semanticweb.org/cra/ontologies/AgriWaterMgmt#deliversWaterTo -->

    <owl:ObjectProperty rdf:about="http://www.semanticweb.org/cra/ontologies/AgriWaterMgmt#deliversWaterTo">
        <rdfs:subPropertyOf rdf:resource="http://www.w3.org/2002/07/owl#topObjectProperty"/>
    </owl:ObjectProperty>
    


    <!-- http://www.semanticweb.org/cra/ontologies/AgriWaterMgmt#enhances -->

    <owl:ObjectProperty rdf:about="http://www.semanticweb.org/cra/ontologies/AgriWaterMgmt#enhances"/>
    


    <!-- http://www.semanticweb.org/cra/ontologies/AgriWaterMgmt#hasPart -->

    <owl:ObjectProperty rdf:about="http://www.semanticweb.org/cra/ontologies/AgriWaterMgmt#hasPart">
        <owl:inverseOf rdf:resource="http://www.semanticweb.org/cra/ontologies/AgriWaterMgmt#isPartOf"/>
        <rdf:type rdf:resource="http://www.w3.org/2002/07/owl#InverseFunctionalProperty"/>
    </owl:ObjectProperty>
    


    <!-- http://www.semanticweb.org/cra/ontologies/AgriWaterMgmt#improves -->

    <owl:ObjectProperty rdf:about="http://www.semanticweb.org/cra/ontologies/AgriWaterMgmt#improves"/>
    


    <!-- http://www.semanticweb.org/cra/ontologies/AgriWaterMgmt#increasesNeedFor -->

    <owl:ObjectProperty rdf:about="http://www.semanticweb.org/cra/ontologies/AgriWaterMgmt#increasesNeedFor"/>
    


    <!-- http://www.semanticweb.org/cra/ontologies/AgriWaterMgmt#isMetBy -->

    <owl:ObjectProperty rdf:about="http://www.semanticweb.org/cra/ontologies/AgriWaterMgmt#isMetBy"/>
    


    <!-- http://www.semanticweb.org/cra/ontologies/AgriWaterMgmt#isMitigatedBy -->

    <owl:ObjectProperty rdf:about="http://www.semanticweb.org/cra/ontologies/AgriWaterMgmt#isMitigatedBy"/>
    


    <!-- http://www.semanticweb.org/cra/ontologies/AgriWaterMgmt#isPartOf -->

    <owl:ObjectProperty rdf:about="http://www.semanticweb.org/cra/ontologies/AgriWaterMgmt#isPartOf">
        <rdf:type rdf:resource="http://www.w3.org/2002/07/owl#InverseFunctionalProperty"/>
    </owl:ObjectProperty>
    


    <!-- http://www.semanticweb.org/cra/ontologies/AgriWaterMgmt#isUsedIn -->

    <owl:ObjectProperty rdf:about="http://www.semanticweb.org/cra/ontologies/AgriWaterMgmt#isUsedIn"/>
    


    <!-- http://www.semanticweb.org/cra/ontologies/AgriWaterMgmt#maintains -->

    <owl:ObjectProperty rdf:about="http://www.semanticweb.org/cra/ontologies/AgriWaterMgmt#maintains"/>
    


    <!-- http://www.semanticweb.org/cra/ontologies/AgriWaterMgmt#optimizes -->

    <owl:ObjectProperty rdf:about="http://www.semanticweb.org/cra/ontologies/AgriWaterMgmt#optimizes">
        <rdfs:subPropertyOf rdf:resource="http://www.w3.org/2002/07/owl#topObjectProperty"/>
        <rdfs:domain rdf:resource="http://www.semanticweb.org/cra/ontologies/AgriWaterMgmt#WaterConservation"/>
        <rdfs:range rdf:resource="http://www.semanticweb.org/cra/ontologies/AgriWaterMgmt#WaterUse"/>
    </owl:ObjectProperty>
    


    <!-- http://www.semanticweb.org/cra/ontologies/AgriWaterMgmt#reduces -->

    <owl:ObjectProperty rdf:about="http://www.semanticweb.org/cra/ontologies/AgriWaterMgmt#reduces"/>
    


    <!-- http://www.semanticweb.org/cra/ontologies/AgriWaterMgmt#requires -->

    <owl:ObjectProperty rdf:about="http://www.semanticweb.org/cra/ontologies/AgriWaterMgmt#requires"/>
    


    <!-- http://www.semanticweb.org/cra/ontologies/AgriWaterMgmt#supplements -->

    <owl:ObjectProperty rdf:about="http://www.semanticweb.org/cra/ontologies/AgriWaterMgmt#supplements"/>
    


    <!-- http://www.semanticweb.org/cra/ontologies/AgriWaterMgmt#supports -->

    <owl:ObjectProperty rdf:about="http://www.semanticweb.org/cra/ontologies/AgriWaterMgmt#supports"/>
    


    <!-- 
    ///////////////////////////////////////////////////////////////////////////////////////
    //
    // Data properties
    //
    ///////////////////////////////////////////////////////////////////////////////////////
     -->

    


    <!-- http://www.semanticweb.org/cra/ontologies/AgriWaterMgmt#hasAccessToWater -->

    <owl:DatatypeProperty rdf:about="http://www.semanticweb.org/cra/ontologies/AgriWaterMgmt#hasAccessToWater">
        <rdfs:domain rdf:resource="http://www.semanticweb.org/cra/ontologies/AgriWaterMgmt#RuralAreas"/>
        <rdfs:domain>
            <owl:Class>
                <owl:unionOf rdf:parseType="Collection">
                    <owl:Restriction>
                        <owl:onProperty rdf:resource="http://www.semanticweb.org/cra/ontologies/AgriWaterMgmt#hasAccessToWater"/>
                        <owl:hasValue>Full Access</owl:hasValue>
                    </owl:Restriction>
                    <owl:Restriction>
                        <owl:onProperty rdf:resource="http://www.semanticweb.org/cra/ontologies/AgriWaterMgmt#hasAccessToWater"/>
                        <owl:hasValue>Limited Access</owl:hasValue>
                    </owl:Restriction>
                    <owl:Restriction>
                        <owl:onProperty rdf:resource="http://www.semanticweb.org/cra/ontologies/AgriWaterMgmt#hasAccessToWater"/>
                        <owl:hasValue>Moderate Access</owl:hasValue>
                    </owl:Restriction>
                </owl:unionOf>
            </owl:Class>
        </rdfs:domain>
        <rdfs:range rdf:resource="http://www.w3.org/2001/XMLSchema#string"/>
        <rdfs:comment xml:lang="en">Indicates the accessibility of water resources in rural areas, with possible values such as &quot;Limited Access&quot;, &quot;Moderate Access&quot;, and &quot;Full Access&quot;.</rdfs:comment>
        <rdfs:label xml:lang="en">hasAccessToWater</rdfs:label>
    </owl:DatatypeProperty>
    


    <!-- http://www.semanticweb.org/cra/ontologies/AgriWaterMgmt#hasAccuracy -->

    <owl:DatatypeProperty rdf:about="http://www.semanticweb.org/cra/ontologies/AgriWaterMgmt#hasAccuracy">
        <rdfs:domain rdf:resource="http://www.semanticweb.org/cra/ontologies/AgriWaterMgmt#WaterSensors"/>
        <rdfs:range rdf:resource="http://www.w3.org/2001/XMLSchema#decimal"/>
        <rdfs:comment xml:lang="en">Measures the accuracy of the sensor, expressed as a percentage.</rdfs:comment>
        <rdfs:label xml:lang="en">hasAccuracy</rdfs:label>
    </owl:DatatypeProperty>
    


    <!-- http://www.semanticweb.org/cra/ontologies/AgriWaterMgmt#hasAdaptationLevel -->

    <owl:DatatypeProperty rdf:about="http://www.semanticweb.org/cra/ontologies/AgriWaterMgmt#hasAdaptationLevel">
        <rdfs:domain rdf:resource="http://www.semanticweb.org/cra/ontologies/AgriWaterMgmt#ClimateChange"/>
        <rdfs:domain>
            <owl:Class>
                <owl:unionOf rdf:parseType="Collection">
                    <owl:Restriction>
                        <owl:onProperty rdf:resource="http://www.semanticweb.org/cra/ontologies/AgriWaterMgmt#hasAdaptationLevel"/>
                        <owl:hasValue>High Adaptation</owl:hasValue>
                    </owl:Restriction>
                    <owl:Restriction>
                        <owl:onProperty rdf:resource="http://www.semanticweb.org/cra/ontologies/AgriWaterMgmt#hasAdaptationLevel"/>
                        <owl:hasValue>Low Adaptation</owl:hasValue>
                    </owl:Restriction>
                    <owl:Restriction>
                        <owl:onProperty rdf:resource="http://www.semanticweb.org/cra/ontologies/AgriWaterMgmt#hasAdaptationLevel"/>
                        <owl:hasValue>Moderate Adaptation</owl:hasValue>
                    </owl:Restriction>
                </owl:unionOf>
            </owl:Class>
        </rdfs:domain>
        <rdfs:range rdf:resource="http://www.w3.org/2001/XMLSchema#string"/>
        <rdfs:comment xml:lang="en">Represents how extensively adaptation strategies for climate change have been implemented. Possible values include &quot;Low Adaptation&quot;, &quot;Moderate Adaptation&quot;, and &quot;High Adaptation&quot;.</rdfs:comment>
        <rdfs:label xml:lang="en">hasAdaptationLevel</rdfs:label>
    </owl:DatatypeProperty>
    


    <!-- http://www.semanticweb.org/cra/ontologies/AgriWaterMgmt#hasApplicationRate -->

    <owl:DatatypeProperty rdf:about="http://www.semanticweb.org/cra/ontologies/AgriWaterMgmt#hasApplicationRate">
        <rdfs:domain rdf:resource="http://www.semanticweb.org/cra/ontologies/AgriWaterMgmt#SprinklerHead"/>
        <rdfs:range rdf:resource="http://www.w3.org/2001/XMLSchema#decimal"/>
        <rdfs:comment xml:lang="en">Measures the rate at which water is applied to the soil, expressed in millimeters per hour (mm/h).</rdfs:comment>
        <rdfs:label xml:lang="en">hasApplicationRate</rdfs:label>
    </owl:DatatypeProperty>
    


    <!-- http://www.semanticweb.org/cra/ontologies/AgriWaterMgmt#hasAutomationLevel -->

    <owl:DatatypeProperty rdf:about="http://www.semanticweb.org/cra/ontologies/AgriWaterMgmt#hasAutomationLevel">
        <rdfs:domain rdf:resource="http://www.semanticweb.org/cra/ontologies/AgriWaterMgmt#IrrigationTechnology"/>
        <rdfs:domain>
            <owl:Class>
                <owl:unionOf rdf:parseType="Collection">
                    <owl:Restriction>
                        <owl:onProperty rdf:resource="http://www.semanticweb.org/cra/ontologies/AgriWaterMgmt#hasAutomationLevel"/>
                        <owl:hasValue>Fully Automatic</owl:hasValue>
                    </owl:Restriction>
                    <owl:Restriction>
                        <owl:onProperty rdf:resource="http://www.semanticweb.org/cra/ontologies/AgriWaterMgmt#hasAutomationLevel"/>
                        <owl:hasValue>Manual</owl:hasValue>
                    </owl:Restriction>
                    <owl:Restriction>
                        <owl:onProperty rdf:resource="http://www.semanticweb.org/cra/ontologies/AgriWaterMgmt#hasAutomationLevel"/>
                        <owl:hasValue>Semi-Automatic</owl:hasValue>
                    </owl:Restriction>
                </owl:unionOf>
            </owl:Class>
        </rdfs:domain>
        <rdfs:range rdf:resource="http://www.w3.org/2001/XMLSchema#string"/>
        <rdfs:comment xml:lang="en">This attribute measures the level of automation in the irrigation system. Possible values may include &quot;Manual&quot;, &quot;Semi-Automatic&quot;, and &quot;Fully Automatic&quot;.</rdfs:comment>
        <rdfs:label xml:lang="en">hasAutomationLevel</rdfs:label>
    </owl:DatatypeProperty>
    


    <!-- http://www.semanticweb.org/cra/ontologies/AgriWaterMgmt#hasAvailableWaterContent -->

    <owl:DatatypeProperty rdf:about="http://www.semanticweb.org/cra/ontologies/AgriWaterMgmt#hasAvailableWaterContent">
        <rdfs:domain rdf:resource="http://www.semanticweb.org/cra/ontologies/AgriWaterMgmt#Soil_Water"/>
        <rdfs:domain>
            <owl:Class>
                <owl:unionOf rdf:parseType="Collection">
                    <owl:Restriction>
                        <owl:onProperty rdf:resource="http://www.semanticweb.org/cra/ontologies/AgriWaterMgmt#hasAvailableWaterContent"/>
                        <owl:hasValue>High Availability</owl:hasValue>
                    </owl:Restriction>
                    <owl:Restriction>
                        <owl:onProperty rdf:resource="http://www.semanticweb.org/cra/ontologies/AgriWaterMgmt#hasAvailableWaterContent"/>
                        <owl:hasValue>Low Availability</owl:hasValue>
                    </owl:Restriction>
                    <owl:Restriction>
                        <owl:onProperty rdf:resource="http://www.semanticweb.org/cra/ontologies/AgriWaterMgmt#hasAvailableWaterContent"/>
                        <owl:hasValue>Moderate Availability</owl:hasValue>
                    </owl:Restriction>
                </owl:unionOf>
            </owl:Class>
        </rdfs:domain>
        <rdfs:range rdf:resource="http://www.w3.org/2001/XMLSchema#string"/>
        <rdfs:comment xml:lang="en">Indicates the amount of water in the soil that is available for plants. Possible values can be &quot;Low Availability&quot;, &quot;Moderate Availability&quot;, and &quot;High Availability&quot;.</rdfs:comment>
        <rdfs:label xml:lang="en">hasAvailableWaterContent</rdfs:label>
    </owl:DatatypeProperty>
    


    <!-- http://www.semanticweb.org/cra/ontologies/AgriWaterMgmt#hasCarbonFootprint -->

    <owl:DatatypeProperty rdf:about="http://www.semanticweb.org/cra/ontologies/AgriWaterMgmt#hasCarbonFootprint">
        <rdfs:domain rdf:resource="http://www.semanticweb.org/cra/ontologies/AgriWaterMgmt#Environmental_Impact"/>
        <rdfs:domain>
            <owl:Class>
                <owl:unionOf rdf:parseType="Collection">
                    <owl:Restriction>
                        <owl:onProperty rdf:resource="http://www.semanticweb.org/cra/ontologies/AgriWaterMgmt#hasCarbonFootprint"/>
                        <owl:hasValue>High Emission</owl:hasValue>
                    </owl:Restriction>
                    <owl:Restriction>
                        <owl:onProperty rdf:resource="http://www.semanticweb.org/cra/ontologies/AgriWaterMgmt#hasCarbonFootprint"/>
                        <owl:hasValue>Low Emission</owl:hasValue>
                    </owl:Restriction>
                    <owl:Restriction>
                        <owl:onProperty rdf:resource="http://www.semanticweb.org/cra/ontologies/AgriWaterMgmt#hasCarbonFootprint"/>
                        <owl:hasValue>Medium Emission</owl:hasValue>
                    </owl:Restriction>
                </owl:unionOf>
            </owl:Class>
        </rdfs:domain>
        <rdfs:range rdf:resource="http://www.w3.org/2001/XMLSchema#string"/>
        <rdfs:comment xml:lang="en">Represents the estimated carbon footprint associated with a particular practice, indicating its greenhouse gas emissions and its impact on climate change. Possible values are &quot;Low Emission&quot;, &quot;Medium Emission&quot;, and &quot;High Emission&quot;.</rdfs:comment>
        <rdfs:label xml:lang="en">hasCarbonFootprint</rdfs:label>
    </owl:DatatypeProperty>
    


    <!-- http://www.semanticweb.org/cra/ontologies/AgriWaterMgmt#hasClimateType -->

    <owl:DatatypeProperty rdf:about="http://www.semanticweb.org/cra/ontologies/AgriWaterMgmt#hasClimateType">
        <rdfs:domain rdf:resource="http://www.semanticweb.org/cra/ontologies/AgriWaterMgmt#Regions"/>
        <rdfs:domain>
            <owl:Class>
                <owl:unionOf rdf:parseType="Collection">
                    <owl:Restriction>
                        <owl:onProperty rdf:resource="http://www.semanticweb.org/cra/ontologies/AgriWaterMgmt#hasClimateType"/>
                        <owl:hasValue>Arid</owl:hasValue>
                    </owl:Restriction>
                    <owl:Restriction>
                        <owl:onProperty rdf:resource="http://www.semanticweb.org/cra/ontologies/AgriWaterMgmt#hasClimateType"/>
                        <owl:hasValue>Humid</owl:hasValue>
                    </owl:Restriction>
                    <owl:Restriction>
                        <owl:onProperty rdf:resource="http://www.semanticweb.org/cra/ontologies/AgriWaterMgmt#hasClimateType"/>
                        <owl:hasValue>Semi-Arid</owl:hasValue>
                    </owl:Restriction>
                </owl:unionOf>
            </owl:Class>
        </rdfs:domain>
        <rdfs:range rdf:resource="http://www.w3.org/2001/XMLSchema#string"/>
        <rdfs:comment xml:lang="en">Represents the climate type in a region, which influences water availability and agricultural viability. Its values include &quot;Arid&quot;, &quot;Semi-Arid&quot;, &quot;Humid&quot;, and &quot;Mediterranean&quot;.</rdfs:comment>
        <rdfs:label xml:lang="en">hasClimateType</rdfs:label>
    </owl:DatatypeProperty>
    


    <!-- http://www.semanticweb.org/cra/ontologies/AgriWaterMgmt#hasCollectionEfficiency -->

    <owl:DatatypeProperty rdf:about="http://www.semanticweb.org/cra/ontologies/AgriWaterMgmt#hasCollectionEfficiency">
        <rdfs:domain rdf:resource="http://www.semanticweb.org/cra/ontologies/AgriWaterMgmt#RainwaterHarvesting"/>
        <rdfs:domain>
            <owl:Class>
                <owl:unionOf rdf:parseType="Collection">
                    <owl:Restriction>
                        <owl:onProperty rdf:resource="http://www.semanticweb.org/cra/ontologies/AgriWaterMgmt#hasCollectionEfficiency"/>
                        <owl:hasValue>High Efficiency</owl:hasValue>
                    </owl:Restriction>
                    <owl:Restriction>
                        <owl:onProperty rdf:resource="http://www.semanticweb.org/cra/ontologies/AgriWaterMgmt#hasCollectionEfficiency"/>
                        <owl:hasValue>Low Efficiency</owl:hasValue>
                    </owl:Restriction>
                    <owl:Restriction>
                        <owl:onProperty rdf:resource="http://www.semanticweb.org/cra/ontologies/AgriWaterMgmt#hasCollectionEfficiency"/>
                        <owl:hasValue>Medium Efficiency</owl:hasValue>
                    </owl:Restriction>
                </owl:unionOf>
            </owl:Class>
        </rdfs:domain>
        <rdfs:range rdf:resource="http://www.w3.org/2001/XMLSchema#string"/>
        <rdfs:comment xml:lang="en">Indicates how effectively the rainwater collection system captures and stores rainwater. Possible values include &quot;Low Efficiency&quot;, &quot;Medium Efficiency&quot;, and &quot;High Efficiency&quot;.</rdfs:comment>
        <rdfs:label xml:lang="en">hasCollectionEfficiency</rdfs:label>
    </owl:DatatypeProperty>
    


    <!-- http://www.semanticweb.org/cra/ontologies/AgriWaterMgmt#hasComplianceLevel -->

    <owl:DatatypeProperty rdf:about="http://www.semanticweb.org/cra/ontologies/AgriWaterMgmt#hasComplianceLevel">
        <rdfs:domain rdf:resource="http://www.semanticweb.org/cra/ontologies/AgriWaterMgmt#WaterRights"/>
        <rdfs:domain>
            <owl:Class>
                <owl:unionOf rdf:parseType="Collection">
                    <owl:Restriction>
                        <owl:onProperty rdf:resource="http://www.semanticweb.org/cra/ontologies/AgriWaterMgmt#hasComplianceLevel"/>
                        <owl:hasValue>Fully Compliant</owl:hasValue>
                    </owl:Restriction>
                    <owl:Restriction>
                        <owl:onProperty rdf:resource="http://www.semanticweb.org/cra/ontologies/AgriWaterMgmt#hasComplianceLevel"/>
                        <owl:hasValue>Non-Compliant</owl:hasValue>
                    </owl:Restriction>
                    <owl:Restriction>
                        <owl:onProperty rdf:resource="http://www.semanticweb.org/cra/ontologies/AgriWaterMgmt#hasComplianceLevel"/>
                        <owl:hasValue>Partially Compliant</owl:hasValue>
                    </owl:Restriction>
                </owl:unionOf>
            </owl:Class>
        </rdfs:domain>
        <rdfs:range rdf:resource="http://www.w3.org/2001/XMLSchema#string"/>
        <rdfs:comment xml:lang="en">Indicates the level of compliance with established water rights regulations. Its values include &quot;Fully Compliant&quot;, &quot;Partially Compliant&quot; and &quot;Non-Compliant&quot;.</rdfs:comment>
        <rdfs:label xml:lang="en">hasComplianceLevel</rdfs:label>
    </owl:DatatypeProperty>
    


    <!-- http://www.semanticweb.org/cra/ontologies/AgriWaterMgmt#hasConservationMethod -->

    <owl:DatatypeProperty rdf:about="http://www.semanticweb.org/cra/ontologies/AgriWaterMgmt#hasConservationMethod">
        <rdfs:domain rdf:resource="http://www.semanticweb.org/cra/ontologies/AgriWaterMgmt#SoilConservation"/>
        <rdfs:domain>
            <owl:Class>
                <owl:unionOf rdf:parseType="Collection">
                    <owl:Restriction>
                        <owl:onProperty rdf:resource="http://www.semanticweb.org/cra/ontologies/AgriWaterMgmt#hasConservationMethod"/>
                        <owl:hasValue>Contour Farming</owl:hasValue>
                    </owl:Restriction>
                    <owl:Restriction>
                        <owl:onProperty rdf:resource="http://www.semanticweb.org/cra/ontologies/AgriWaterMgmt#hasConservationMethod"/>
                        <owl:hasValue>Cover Cropping</owl:hasValue>
                    </owl:Restriction>
                    <owl:Restriction>
                        <owl:onProperty rdf:resource="http://www.semanticweb.org/cra/ontologies/AgriWaterMgmt#hasConservationMethod"/>
                        <owl:hasValue>No-Till Farming</owl:hasValue>
                    </owl:Restriction>
                </owl:unionOf>
            </owl:Class>
        </rdfs:domain>
        <rdfs:range rdf:resource="http://www.w3.org/2001/XMLSchema#string"/>
        <rdfs:comment xml:lang="en">Represents the techniques used to maintain soil health and prevent erosion. Examples include &quot;Contour Farming&quot;, &quot;No-Till Farming&quot;, and &quot;Cover Cropping&quot;.</rdfs:comment>
        <rdfs:label xml:lang="en">hasConservationMethod</rdfs:label>
    </owl:DatatypeProperty>
    


    <!-- http://www.semanticweb.org/cra/ontologies/AgriWaterMgmt#hasCost -->

    <owl:DatatypeProperty rdf:about="http://www.semanticweb.org/cra/ontologies/AgriWaterMgmt#hasCost">
        <rdfs:domain rdf:resource="http://www.semanticweb.org/cra/ontologies/AgriWaterMgmt#Accessories"/>
        <rdfs:domain rdf:resource="http://www.semanticweb.org/cra/ontologies/AgriWaterMgmt#Couplers"/>
        <rdfs:domain rdf:resource="http://www.semanticweb.org/cra/ontologies/AgriWaterMgmt#DripIrrigation"/>
        <rdfs:domain rdf:resource="http://www.semanticweb.org/cra/ontologies/AgriWaterMgmt#IrrigationSystems"/>
        <rdfs:domain rdf:resource="http://www.semanticweb.org/cra/ontologies/AgriWaterMgmt#IrrigationTechnology"/>
        <rdfs:domain rdf:resource="http://www.semanticweb.org/cra/ontologies/AgriWaterMgmt#PumpUnit"/>
        <rdfs:domain rdf:resource="http://www.semanticweb.org/cra/ontologies/AgriWaterMgmt#RegulatedDeficitIrrigation"/>
        <rdfs:domain rdf:resource="http://www.semanticweb.org/cra/ontologies/AgriWaterMgmt#SprinklerHead"/>
        <rdfs:domain rdf:resource="http://www.semanticweb.org/cra/ontologies/AgriWaterMgmt#SprinklerIrrigation"/>
        <rdfs:domain rdf:resource="http://www.semanticweb.org/cra/ontologies/AgriWaterMgmt#SubsurfaceIrrigation"/>
        <rdfs:domain rdf:resource="http://www.semanticweb.org/cra/ontologies/AgriWaterMgmt#SurfaceIrrigation"/>
        <rdfs:domain rdf:resource="http://www.semanticweb.org/cra/ontologies/AgriWaterMgmt#Tubings"/>
        <rdfs:domain rdf:resource="http://www.semanticweb.org/cra/ontologies/AgriWaterMgmt#WaterSensors"/>
        <rdfs:range rdf:resource="http://www.w3.org/2001/XMLSchema#decimal"/>
        <rdfs:comment xml:lang="en">Represents the monetary cost of accessory components or irrigation technology, using numeric values.</rdfs:comment>
        <rdfs:label xml:lang="en">hasCost</rdfs:label>
    </owl:DatatypeProperty>
    


    <!-- http://www.semanticweb.org/cra/ontologies/AgriWaterMgmt#hasCostEffectiveness -->

    <owl:DatatypeProperty rdf:about="http://www.semanticweb.org/cra/ontologies/AgriWaterMgmt#hasCostEffectiveness">
        <rdfs:domain rdf:resource="http://www.semanticweb.org/cra/ontologies/AgriWaterMgmt#WaterConservation"/>
        <rdfs:domain>
            <owl:Class>
                <owl:unionOf rdf:parseType="Collection">
                    <owl:Restriction>
                        <owl:onProperty rdf:resource="http://www.semanticweb.org/cra/ontologies/AgriWaterMgmt#hasCostEffectiveness"/>
                        <owl:hasValue>High Cost</owl:hasValue>
                    </owl:Restriction>
                    <owl:Restriction>
                        <owl:onProperty rdf:resource="http://www.semanticweb.org/cra/ontologies/AgriWaterMgmt#hasCostEffectiveness"/>
                        <owl:hasValue>Low Cost</owl:hasValue>
                    </owl:Restriction>
                    <owl:Restriction>
                        <owl:onProperty rdf:resource="http://www.semanticweb.org/cra/ontologies/AgriWaterMgmt#hasCostEffectiveness"/>
                        <owl:hasValue>Moderate Cost</owl:hasValue>
                    </owl:Restriction>
                </owl:unionOf>
            </owl:Class>
        </rdfs:domain>
        <rdfs:range rdf:resource="http://www.w3.org/2001/XMLSchema#string"/>
        <rdfs:comment xml:lang="en">Indicates how cost-effective water conservation measures are, evaluating their economic viability. Its values include &quot;Low Cost&quot;, &quot;Moderate Cost&quot;, and &quot;High Cost&quot;.</rdfs:comment>
        <rdfs:label xml:lang="en">hasCostEffectiveness</rdfs:label>
    </owl:DatatypeProperty>
    


    <!-- http://www.semanticweb.org/cra/ontologies/AgriWaterMgmt#hasDataSource -->

    <owl:DatatypeProperty rdf:about="http://www.semanticweb.org/cra/ontologies/AgriWaterMgmt#hasDataSource">
        <rdfs:domain rdf:resource="http://www.semanticweb.org/cra/ontologies/AgriWaterMgmt#PrecisionAgriculture"/>
        <rdfs:domain>
            <owl:Class>
                <owl:unionOf rdf:parseType="Collection">
                    <owl:Restriction>
                        <owl:onProperty rdf:resource="http://www.semanticweb.org/cra/ontologies/AgriWaterMgmt#hasDataSource"/>
                        <owl:hasValue>Drones</owl:hasValue>
                    </owl:Restriction>
                    <owl:Restriction>
                        <owl:onProperty rdf:resource="http://www.semanticweb.org/cra/ontologies/AgriWaterMgmt#hasDataSource"/>
                        <owl:hasValue>Satellite Imagery</owl:hasValue>
                    </owl:Restriction>
                    <owl:Restriction>
                        <owl:onProperty rdf:resource="http://www.semanticweb.org/cra/ontologies/AgriWaterMgmt#hasDataSource"/>
                        <owl:hasValue>Soil Sensors</owl:hasValue>
                    </owl:Restriction>
                    <owl:Restriction>
                        <owl:onProperty rdf:resource="http://www.semanticweb.org/cra/ontologies/AgriWaterMgmt#hasDataSource"/>
                        <owl:hasValue>Weather Stations</owl:hasValue>
                    </owl:Restriction>
                </owl:unionOf>
            </owl:Class>
        </rdfs:domain>
        <rdfs:range rdf:resource="http://www.w3.org/2001/XMLSchema#string"/>
        <rdfs:comment xml:lang="en">Identifies the sources of data used in precision agriculture, which may include &quot;Satellite Imagery&quot;, &quot;Soil Sensors&quot;, &quot;Weather Stations&quot;, or &quot;Drones&quot;.</rdfs:comment>
        <rdfs:label xml:lang="en">hasDataSource</rdfs:label>
    </owl:DatatypeProperty>
    


    <!-- http://www.semanticweb.org/cra/ontologies/AgriWaterMgmt#hasDiameter -->

    <owl:DatatypeProperty rdf:about="http://www.semanticweb.org/cra/ontologies/AgriWaterMgmt#hasDiameter">
        <rdfs:domain rdf:resource="http://www.semanticweb.org/cra/ontologies/AgriWaterMgmt#Tubings"/>
        <rdfs:range rdf:resource="http://www.w3.org/2001/XMLSchema#decimal"/>
        <rdfs:comment xml:lang="en">Defines the diameter of the tubing, expressed in millimeters.</rdfs:comment>
        <rdfs:label xml:lang="en">hasDiameter</rdfs:label>
    </owl:DatatypeProperty>
    


    <!-- http://www.semanticweb.org/cra/ontologies/AgriWaterMgmt#hasDurabilityLevel -->

    <owl:DatatypeProperty rdf:about="http://www.semanticweb.org/cra/ontologies/AgriWaterMgmt#hasDurabilityLevel">
        <rdfs:domain rdf:resource="http://www.semanticweb.org/cra/ontologies/AgriWaterMgmt#Accessories"/>
        <rdfs:domain rdf:resource="http://www.semanticweb.org/cra/ontologies/AgriWaterMgmt#Couplers"/>
        <rdfs:domain>
            <owl:Class>
                <owl:unionOf rdf:parseType="Collection">
                    <owl:Restriction>
                        <owl:onProperty rdf:resource="http://www.semanticweb.org/cra/ontologies/AgriWaterMgmt#hasDurabilityLevel"/>
                        <owl:hasValue>High Durability</owl:hasValue>
                    </owl:Restriction>
                    <owl:Restriction>
                        <owl:onProperty rdf:resource="http://www.semanticweb.org/cra/ontologies/AgriWaterMgmt#hasDurabilityLevel"/>
                        <owl:hasValue>Low Durability</owl:hasValue>
                    </owl:Restriction>
                    <owl:Restriction>
                        <owl:onProperty rdf:resource="http://www.semanticweb.org/cra/ontologies/AgriWaterMgmt#hasDurabilityLevel"/>
                        <owl:hasValue>Medium Durability</owl:hasValue>
                    </owl:Restriction>
                </owl:unionOf>
            </owl:Class>
        </rdfs:domain>
        <rdfs:range rdf:resource="http://www.w3.org/2001/XMLSchema#string"/>
        <rdfs:comment xml:lang="en">Indicates the durability of the accessory components. Values include &quot;Low Durability&quot;, &quot;Medium Durability&quot; and &quot;High Durability&quot;.</rdfs:comment>
        <rdfs:label xml:lang="en">hasDurabilityLevel</rdfs:label>
    </owl:DatatypeProperty>
    


    <!-- http://www.semanticweb.org/cra/ontologies/AgriWaterMgmt#hasDuration -->

    <owl:DatatypeProperty rdf:about="http://www.semanticweb.org/cra/ontologies/AgriWaterMgmt#hasDuration">
        <rdfs:domain rdf:resource="http://www.semanticweb.org/cra/ontologies/AgriWaterMgmt#Drought"/>
        <rdfs:range rdf:resource="http://www.w3.org/2001/XMLSchema#positiveInteger"/>
        <rdfs:comment xml:lang="en">Represents the length of time (in days) that drought conditions persist. It is expressed as a positive integer.</rdfs:comment>
        <rdfs:label xml:lang="en">hasDuration</rdfs:label>
    </owl:DatatypeProperty>
    


    <!-- http://www.semanticweb.org/cra/ontologies/AgriWaterMgmt#hasEconomicImpact -->

    <owl:DatatypeProperty rdf:about="http://www.semanticweb.org/cra/ontologies/AgriWaterMgmt#hasEconomicImpact">
        <rdfs:domain rdf:resource="http://www.semanticweb.org/cra/ontologies/AgriWaterMgmt#PrecisionAgriculture"/>
        <rdfs:domain rdf:resource="http://www.semanticweb.org/cra/ontologies/AgriWaterMgmt#WaterOptimization"/>
        <rdfs:domain>
            <owl:Class>
                <owl:unionOf rdf:parseType="Collection">
                    <owl:Restriction>
                        <owl:onProperty rdf:resource="http://www.semanticweb.org/cra/ontologies/AgriWaterMgmt#hasEconomicImpact"/>
                        <owl:hasValue>Negative Impact</owl:hasValue>
                    </owl:Restriction>
                    <owl:Restriction>
                        <owl:onProperty rdf:resource="http://www.semanticweb.org/cra/ontologies/AgriWaterMgmt#hasEconomicImpact"/>
                        <owl:hasValue>Neutral Impact</owl:hasValue>
                    </owl:Restriction>
                    <owl:Restriction>
                        <owl:onProperty rdf:resource="http://www.semanticweb.org/cra/ontologies/AgriWaterMgmt#hasEconomicImpact"/>
                        <owl:hasValue>Positive Impact</owl:hasValue>
                    </owl:Restriction>
                </owl:unionOf>
            </owl:Class>
        </rdfs:domain>
        <rdfs:range rdf:resource="http://www.w3.org/2001/XMLSchema#string"/>
        <rdfs:comment xml:lang="en">Represents the economic impact of water optimization and precision agriculture practices. This attribute evaluates how optimized water use affects the financial aspects of agricultural practices. Its values include &quot;Positive Impact&quot;, &quot;Neutral Impact&quot;, and &quot;Negative Impact&quot;.</rdfs:comment>
        <rdfs:label xml:lang="en">hasEconomicImpact</rdfs:label>
    </owl:DatatypeProperty>
    


    <!-- http://www.semanticweb.org/cra/ontologies/AgriWaterMgmt#hasEfficiencyLevel -->

    <owl:DatatypeProperty rdf:about="http://www.semanticweb.org/cra/ontologies/AgriWaterMgmt#hasEfficiencyLevel">
        <rdfs:domain rdf:resource="http://www.semanticweb.org/cra/ontologies/AgriWaterMgmt#DripIrrigation"/>
        <rdfs:domain rdf:resource="http://www.semanticweb.org/cra/ontologies/AgriWaterMgmt#IrrigationSystems"/>
        <rdfs:domain rdf:resource="http://www.semanticweb.org/cra/ontologies/AgriWaterMgmt#RegulatedDeficitIrrigation"/>
        <rdfs:domain rdf:resource="http://www.semanticweb.org/cra/ontologies/AgriWaterMgmt#SprinklerIrrigation"/>
        <rdfs:domain rdf:resource="http://www.semanticweb.org/cra/ontologies/AgriWaterMgmt#SubsurfaceIrrigation"/>
        <rdfs:domain rdf:resource="http://www.semanticweb.org/cra/ontologies/AgriWaterMgmt#SurfaceIrrigation"/>
        <rdfs:domain rdf:resource="http://www.semanticweb.org/cra/ontologies/AgriWaterMgmt#SustainableAgriculture"/>
        <rdfs:domain rdf:resource="http://www.semanticweb.org/cra/ontologies/AgriWaterMgmt#WaterConservation"/>
        <rdfs:domain rdf:resource="http://www.semanticweb.org/cra/ontologies/AgriWaterMgmt#WaterEfficiency"/>
        <rdfs:domain rdf:resource="http://www.semanticweb.org/cra/ontologies/AgriWaterMgmt#WaterUse"/>
        <rdfs:domain>
            <owl:Class>
                <owl:unionOf rdf:parseType="Collection">
                    <owl:Restriction>
                        <owl:onProperty rdf:resource="http://www.semanticweb.org/cra/ontologies/AgriWaterMgmt#hasEfficiencyLevel"/>
                        <owl:hasValue>Efficient</owl:hasValue>
                    </owl:Restriction>
                    <owl:Restriction>
                        <owl:onProperty rdf:resource="http://www.semanticweb.org/cra/ontologies/AgriWaterMgmt#hasEfficiencyLevel"/>
                        <owl:hasValue>High Efficient</owl:hasValue>
                    </owl:Restriction>
                    <owl:Restriction>
                        <owl:onProperty rdf:resource="http://www.semanticweb.org/cra/ontologies/AgriWaterMgmt#hasEfficiencyLevel"/>
                        <owl:hasValue>Low Efficient</owl:hasValue>
                    </owl:Restriction>
                </owl:unionOf>
            </owl:Class>
        </rdfs:domain>
        <rdfs:range rdf:resource="http://www.w3.org/2001/XMLSchema#string"/>
        <rdfs:comment xml:lang="en">Degree of effectiveness in water conservation practices, water efficiency strategies and water use in agricultural practices. It indicates how efficiently water is used or conserved in a particular method or system. Its values include &quot;Low Efficient&quot;, &quot;Efficient&quot;, and &quot;Highly Efficient&quot;.</rdfs:comment>
        <rdfs:label xml:lang="en">hasEfficiencyLevel</rdfs:label>
    </owl:DatatypeProperty>
    


    <!-- http://www.semanticweb.org/cra/ontologies/AgriWaterMgmt#hasElectricalConductivity -->

    <owl:DatatypeProperty rdf:about="http://www.semanticweb.org/cra/ontologies/AgriWaterMgmt#hasElectricalConductivity">
        <rdfs:domain rdf:resource="http://www.semanticweb.org/cra/ontologies/AgriWaterMgmt#SoilSalinity"/>
        <rdfs:domain>
            <owl:Class>
                <owl:unionOf rdf:parseType="Collection">
                    <owl:Restriction>
                        <owl:onProperty rdf:resource="http://www.semanticweb.org/cra/ontologies/AgriWaterMgmt#hasElectricalConductivity"/>
                        <owl:hasValue>High Conductivity</owl:hasValue>
                    </owl:Restriction>
                    <owl:Restriction>
                        <owl:onProperty rdf:resource="http://www.semanticweb.org/cra/ontologies/AgriWaterMgmt#hasElectricalConductivity"/>
                        <owl:hasValue>Low Conductivity</owl:hasValue>
                    </owl:Restriction>
                    <owl:Restriction>
                        <owl:onProperty rdf:resource="http://www.semanticweb.org/cra/ontologies/AgriWaterMgmt#hasElectricalConductivity"/>
                        <owl:hasValue>Medium Conductivity</owl:hasValue>
                    </owl:Restriction>
                </owl:unionOf>
            </owl:Class>
        </rdfs:domain>
        <rdfs:range rdf:resource="http://www.w3.org/2001/XMLSchema#string"/>
        <rdfs:comment xml:lang="en">Measures the ability of soil to conduct electrical current, which is related to salinity levels. Possible values can be &quot;Low Conductivity&quot;, &quot;Medium Conductivity&quot;, and &quot;High Conductivity&quot;.</rdfs:comment>
        <rdfs:label xml:lang="en">hasElectricalConductivity</rdfs:label>
    </owl:DatatypeProperty>
    


    <!-- http://www.semanticweb.org/cra/ontologies/AgriWaterMgmt#hasEmitterType -->

    <owl:DatatypeProperty rdf:about="http://www.semanticweb.org/cra/ontologies/AgriWaterMgmt#hasEmitterType">
        <rdfs:domain rdf:resource="http://www.semanticweb.org/cra/ontologies/AgriWaterMgmt#DripIrrigation"/>
        <rdfs:domain>
            <owl:Class>
                <owl:unionOf rdf:parseType="Collection">
                    <owl:Restriction>
                        <owl:onProperty rdf:resource="http://www.semanticweb.org/cra/ontologies/AgriWaterMgmt#hasEmitterType"/>
                        <owl:hasValue>Bubbler</owl:hasValue>
                    </owl:Restriction>
                    <owl:Restriction>
                        <owl:onProperty rdf:resource="http://www.semanticweb.org/cra/ontologies/AgriWaterMgmt#hasEmitterType"/>
                        <owl:hasValue>In-line Emitter</owl:hasValue>
                    </owl:Restriction>
                    <owl:Restriction>
                        <owl:onProperty rdf:resource="http://www.semanticweb.org/cra/ontologies/AgriWaterMgmt#hasEmitterType"/>
                        <owl:hasValue>Point Source Emitter</owl:hasValue>
                    </owl:Restriction>
                </owl:unionOf>
            </owl:Class>
        </rdfs:domain>
        <rdfs:range rdf:resource="http://www.w3.org/2001/XMLSchema#string"/>
        <rdfs:comment xml:lang="en">Specifies the type of emitter used in the drip irrigation system, which controls the flow of water to crops, with possible values such as &quot;Point Source Emitter&quot;, &quot;In-line Emitter&quot;, and &quot;Bubbler&quot;.</rdfs:comment>
        <rdfs:label xml:lang="en">hasEmitterType</rdfs:label>
    </owl:DatatypeProperty>
    


    <!-- http://www.semanticweb.org/cra/ontologies/AgriWaterMgmt#hasEnergyConsumption -->

    <owl:DatatypeProperty rdf:about="http://www.semanticweb.org/cra/ontologies/AgriWaterMgmt#hasEnergyConsumption">
        <rdfs:domain rdf:resource="http://www.semanticweb.org/cra/ontologies/AgriWaterMgmt#PumpUnit"/>
        <rdfs:range rdf:resource="http://www.w3.org/2001/XMLSchema#decimal"/>
        <rdfs:comment xml:lang="en">Quantifies the energy consumption of the pump unit, expressed in kilowatt-hours (kWh).</rdfs:comment>
        <rdfs:label xml:lang="en">hasEnergyConsumption</rdfs:label>
    </owl:DatatypeProperty>
    


    <!-- http://www.semanticweb.org/cra/ontologies/AgriWaterMgmt#hasEngagementLevel -->

    <owl:DatatypeProperty rdf:about="http://www.semanticweb.org/cra/ontologies/AgriWaterMgmt#hasEngagementLevel">
        <rdfs:domain rdf:resource="http://www.semanticweb.org/cra/ontologies/AgriWaterMgmt#WaterPolicy"/>
        <rdfs:domain>
            <owl:Class>
                <owl:unionOf rdf:parseType="Collection">
                    <owl:Restriction>
                        <owl:onProperty rdf:resource="http://www.semanticweb.org/cra/ontologies/AgriWaterMgmt#hasEngagementLevel"/>
                        <owl:hasValue>High Engagement</owl:hasValue>
                    </owl:Restriction>
                    <owl:Restriction>
                        <owl:onProperty rdf:resource="http://www.semanticweb.org/cra/ontologies/AgriWaterMgmt#hasEngagementLevel"/>
                        <owl:hasValue>Low Engagement</owl:hasValue>
                    </owl:Restriction>
                    <owl:Restriction>
                        <owl:onProperty rdf:resource="http://www.semanticweb.org/cra/ontologies/AgriWaterMgmt#hasEngagementLevel"/>
                        <owl:hasValue>Moderate Engagement</owl:hasValue>
                    </owl:Restriction>
                </owl:unionOf>
            </owl:Class>
        </rdfs:domain>
        <rdfs:range rdf:resource="http://www.w3.org/2001/XMLSchema#string"/>
        <rdfs:comment xml:lang="en">Measures the level of engagement in water policy decisions. Its values include &quot;High Engagement&quot;, &quot;Moderate Engagement&quot; and &quot;Low Engagement&quot;.</rdfs:comment>
        <rdfs:label xml:lang="en">hasEngagementLevel</rdfs:label>
    </owl:DatatypeProperty>
    


    <!-- http://www.semanticweb.org/cra/ontologies/AgriWaterMgmt#hasEnvironmentalImpactLevel -->

    <owl:DatatypeProperty rdf:about="http://www.semanticweb.org/cra/ontologies/AgriWaterMgmt#hasEnvironmentalImpactLevel">
        <rdfs:domain rdf:resource="http://www.semanticweb.org/cra/ontologies/AgriWaterMgmt#Environmental_Impact"/>
        <rdfs:domain rdf:resource="http://www.semanticweb.org/cra/ontologies/AgriWaterMgmt#SustainabilityAndEnvironmentalImpact"/>
        <rdfs:domain>
            <owl:Class>
                <owl:unionOf rdf:parseType="Collection">
                    <owl:Restriction>
                        <owl:onProperty rdf:resource="http://www.semanticweb.org/cra/ontologies/AgriWaterMgmt#hasEnvironmentalImpactLevel"/>
                        <owl:hasValue>High Impact</owl:hasValue>
                    </owl:Restriction>
                    <owl:Restriction>
                        <owl:onProperty rdf:resource="http://www.semanticweb.org/cra/ontologies/AgriWaterMgmt#hasEnvironmentalImpactLevel"/>
                        <owl:hasValue>Low Impact</owl:hasValue>
                    </owl:Restriction>
                    <owl:Restriction>
                        <owl:onProperty rdf:resource="http://www.semanticweb.org/cra/ontologies/AgriWaterMgmt#hasEnvironmentalImpactLevel"/>
                        <owl:hasValue>Medium Impact</owl:hasValue>
                    </owl:Restriction>
                </owl:unionOf>
            </owl:Class>
        </rdfs:domain>
        <rdfs:range rdf:resource="http://www.w3.org/2001/XMLSchema#string"/>
        <rdfs:comment xml:lang="en">Indicates the degree of environmental impact associated with a specific practice. It helps in assessing the negative or positive effects on the environment. Possible values can be &quot;Low Impact&quot;, &quot;Medium Impact&quot;, and &quot;High Impact&quot;.</rdfs:comment>
        <rdfs:label xml:lang="en">hasEnvironmentalImpactLevel</rdfs:label>
    </owl:DatatypeProperty>
    


    <!-- http://www.semanticweb.org/cra/ontologies/AgriWaterMgmt#hasErosionRiskLevel -->

    <owl:DatatypeProperty rdf:about="http://www.semanticweb.org/cra/ontologies/AgriWaterMgmt#hasErosionRiskLevel">
        <rdfs:domain rdf:resource="http://www.semanticweb.org/cra/ontologies/AgriWaterMgmt#SoilConservation"/>
        <rdfs:domain>
            <owl:Class>
                <owl:unionOf rdf:parseType="Collection">
                    <owl:Restriction>
                        <owl:onProperty rdf:resource="http://www.semanticweb.org/cra/ontologies/AgriWaterMgmt#hasErosionRiskLevel"/>
                        <owl:hasValue>High Risk</owl:hasValue>
                    </owl:Restriction>
                    <owl:Restriction>
                        <owl:onProperty rdf:resource="http://www.semanticweb.org/cra/ontologies/AgriWaterMgmt#hasErosionRiskLevel"/>
                        <owl:hasValue>Low Risk</owl:hasValue>
                    </owl:Restriction>
                    <owl:Restriction>
                        <owl:onProperty rdf:resource="http://www.semanticweb.org/cra/ontologies/AgriWaterMgmt#hasErosionRiskLevel"/>
                        <owl:hasValue>Moderate Risk</owl:hasValue>
                    </owl:Restriction>
                </owl:unionOf>
            </owl:Class>
        </rdfs:domain>
        <rdfs:range rdf:resource="http://www.w3.org/2001/XMLSchema#string"/>
        <rdfs:comment xml:lang="en">Indicates the level of risk of soil erosion based on current practices and environmental conditions. Possible values are &quot;Low Risk&quot;, &quot;Moderate Risk&quot;, and &quot;High Risk&quot;.</rdfs:comment>
        <rdfs:label xml:lang="en">hasErosionRiskLevel</rdfs:label>
    </owl:DatatypeProperty>
    


    <!-- http://www.semanticweb.org/cra/ontologies/AgriWaterMgmt#hasEvapotranspirationRate -->

    <owl:DatatypeProperty rdf:about="http://www.semanticweb.org/cra/ontologies/AgriWaterMgmt#hasEvapotranspirationRate">
        <rdfs:domain rdf:resource="http://www.semanticweb.org/cra/ontologies/AgriWaterMgmt#CropEvapotranspiration"/>
        <rdfs:domain>
            <owl:Class>
                <owl:unionOf rdf:parseType="Collection">
                    <owl:Restriction>
                        <owl:onProperty rdf:resource="http://www.semanticweb.org/cra/ontologies/AgriWaterMgmt#hasEvapotranspirationRate"/>
                        <owl:hasValue>High Rate</owl:hasValue>
                    </owl:Restriction>
                    <owl:Restriction>
                        <owl:onProperty rdf:resource="http://www.semanticweb.org/cra/ontologies/AgriWaterMgmt#hasEvapotranspirationRate"/>
                        <owl:hasValue>Low Rate</owl:hasValue>
                    </owl:Restriction>
                    <owl:Restriction>
                        <owl:onProperty rdf:resource="http://www.semanticweb.org/cra/ontologies/AgriWaterMgmt#hasEvapotranspirationRate"/>
                        <owl:hasValue>Medium Rate</owl:hasValue>
                    </owl:Restriction>
                </owl:unionOf>
            </owl:Class>
        </rdfs:domain>
        <rdfs:range rdf:resource="http://www.w3.org/2001/XMLSchema#string"/>
        <rdfs:comment xml:lang="en">Rate at which water is lost from the crop surface and soil through evaporation and transpiration. Its values include &quot;Low Rate&quot;, &quot;Medium Rate&quot; and &quot;High Rate&quot;.</rdfs:comment>
        <rdfs:label xml:lang="en">hasEvapotranspirationRate</rdfs:label>
    </owl:DatatypeProperty>
    


    <!-- http://www.semanticweb.org/cra/ontologies/AgriWaterMgmt#hasFlowRate -->

    <owl:DatatypeProperty rdf:about="http://www.semanticweb.org/cra/ontologies/AgriWaterMgmt#hasFlowRate">
        <rdfs:domain rdf:resource="http://www.semanticweb.org/cra/ontologies/AgriWaterMgmt#PumpUnit"/>
        <rdfs:range rdf:resource="http://www.w3.org/2001/XMLSchema#decimal"/>
        <rdfs:comment xml:lang="en">Specifies the flow rate of the pump unit, measured in liters per minute (L/min). It indicates the volume of water that the pump can deliver over a specified time period.</rdfs:comment>
        <rdfs:label xml:lang="en">hasFlowRate</rdfs:label>
    </owl:DatatypeProperty>
    


    <!-- http://www.semanticweb.org/cra/ontologies/AgriWaterMgmt#hasFrecuency -->

    <owl:DatatypeProperty rdf:about="http://www.semanticweb.org/cra/ontologies/AgriWaterMgmt#hasFrecuency">
        <rdfs:domain rdf:resource="http://www.semanticweb.org/cra/ontologies/AgriWaterMgmt#IrrigationScheduling"/>
        <rdfs:domain>
            <owl:Class>
                <owl:unionOf rdf:parseType="Collection">
                    <owl:Restriction>
                        <owl:onProperty rdf:resource="http://www.semanticweb.org/cra/ontologies/AgriWaterMgmt#hasFrecuency"/>
                        <owl:hasValue>Daily</owl:hasValue>
                    </owl:Restriction>
                    <owl:Restriction>
                        <owl:onProperty rdf:resource="http://www.semanticweb.org/cra/ontologies/AgriWaterMgmt#hasFrecuency"/>
                        <owl:hasValue>Monthly</owl:hasValue>
                    </owl:Restriction>
                    <owl:Restriction>
                        <owl:onProperty rdf:resource="http://www.semanticweb.org/cra/ontologies/AgriWaterMgmt#hasFrecuency"/>
                        <owl:hasValue>Weekly</owl:hasValue>
                    </owl:Restriction>
                </owl:unionOf>
            </owl:Class>
        </rdfs:domain>
        <rdfs:range rdf:resource="http://www.w3.org/2001/XMLSchema#string"/>
        <rdfs:comment xml:lang="en">Indicates the frecuency of irrigation in an agricultural system. Possible values include &quot;Daily&quot;, &quot;Weekly&quot; and &quot;Monthly&quot;.</rdfs:comment>
        <rdfs:label xml:lang="en">hasFrequency</rdfs:label>
    </owl:DatatypeProperty>
    


    <!-- http://www.semanticweb.org/cra/ontologies/AgriWaterMgmt#hasGrowthDuration -->

    <owl:DatatypeProperty rdf:about="http://www.semanticweb.org/cra/ontologies/AgriWaterMgmt#hasGrowthDuration">
        <rdfs:domain rdf:resource="http://www.semanticweb.org/cra/ontologies/AgriWaterMgmt#Crops"/>
        <rdfs:range rdf:resource="http://www.w3.org/2001/XMLSchema#positiveInteger"/>
        <rdfs:comment xml:lang="en">Represents the time it takes for a crop to reach maturity, measured in days.</rdfs:comment>
        <rdfs:label xml:lang="en">hasGrowthDuration</rdfs:label>
    </owl:DatatypeProperty>
    


    <!-- http://www.semanticweb.org/cra/ontologies/AgriWaterMgmt#hasGrowthStage -->

    <owl:DatatypeProperty rdf:about="http://www.semanticweb.org/cra/ontologies/AgriWaterMgmt#hasGrowthStage">
        <rdfs:domain rdf:resource="http://www.semanticweb.org/cra/ontologies/AgriWaterMgmt#CropGrowthStages"/>
        <rdfs:domain>
            <owl:Class>
                <owl:unionOf rdf:parseType="Collection">
                    <owl:Restriction>
                        <owl:onProperty rdf:resource="http://www.semanticweb.org/cra/ontologies/AgriWaterMgmt#hasGrowthStage"/>
                        <owl:hasValue>Flowering</owl:hasValue>
                    </owl:Restriction>
                    <owl:Restriction>
                        <owl:onProperty rdf:resource="http://www.semanticweb.org/cra/ontologies/AgriWaterMgmt#hasGrowthStage"/>
                        <owl:hasValue>Germination</owl:hasValue>
                    </owl:Restriction>
                    <owl:Restriction>
                        <owl:onProperty rdf:resource="http://www.semanticweb.org/cra/ontologies/AgriWaterMgmt#hasGrowthStage"/>
                        <owl:hasValue>Maturity</owl:hasValue>
                    </owl:Restriction>
                    <owl:Restriction>
                        <owl:onProperty rdf:resource="http://www.semanticweb.org/cra/ontologies/AgriWaterMgmt#hasGrowthStage"/>
                        <owl:hasValue>Vegetative</owl:hasValue>
                    </owl:Restriction>
                </owl:unionOf>
            </owl:Class>
        </rdfs:domain>
        <rdfs:range rdf:resource="http://www.w3.org/2001/XMLSchema#string"/>
        <rdfs:comment xml:lang="en">Refers to the specific stages of crop development, which require different water and nutrient resources. Its values include &quot;Germination&quot;, &quot;Vegetative&quot;, Flowering and Maturity.</rdfs:comment>
        <rdfs:label xml:lang="en">hasGrowthStage</rdfs:label>
    </owl:DatatypeProperty>
    


    <!-- http://www.semanticweb.org/cra/ontologies/AgriWaterMgmt#hasImpactLevel -->

    <owl:DatatypeProperty rdf:about="http://www.semanticweb.org/cra/ontologies/AgriWaterMgmt#hasImpactLevel">
        <rdfs:domain rdf:resource="http://www.semanticweb.org/cra/ontologies/AgriWaterMgmt#AgriculturalEngineering"/>
        <rdfs:domain rdf:resource="http://www.semanticweb.org/cra/ontologies/AgriWaterMgmt#WaterConservation"/>
        <rdfs:domain rdf:resource="http://www.semanticweb.org/cra/ontologies/AgriWaterMgmt#WaterUse"/>
        <rdfs:domain>
            <owl:Class>
                <owl:unionOf rdf:parseType="Collection">
                    <owl:Restriction>
                        <owl:onProperty rdf:resource="http://www.semanticweb.org/cra/ontologies/AgriWaterMgmt#hasImpactLevel"/>
                        <owl:hasValue>High Impact</owl:hasValue>
                    </owl:Restriction>
                    <owl:Restriction>
                        <owl:onProperty rdf:resource="http://www.semanticweb.org/cra/ontologies/AgriWaterMgmt#hasImpactLevel"/>
                        <owl:hasValue>Low Impact</owl:hasValue>
                    </owl:Restriction>
                    <owl:Restriction>
                        <owl:onProperty rdf:resource="http://www.semanticweb.org/cra/ontologies/AgriWaterMgmt#hasImpactLevel"/>
                        <owl:hasValue>Medium Impact</owl:hasValue>
                    </owl:Restriction>
                </owl:unionOf>
            </owl:Class>
        </rdfs:domain>
        <rdfs:range rdf:resource="http://www.w3.org/2001/XMLSchema#string"/>
        <rdfs:comment xml:lang="en">Environmental or operational impact of water conservation and water use measures, as well as agriculture engineering solutions. It classifies practices based on their overall effect on the environment or agricultural system, with possible values such as &quot;Low Impact&quot;, &quot;Medium Impact&quot;, and &quot;High Impact&quot;.</rdfs:comment>
        <rdfs:label xml:lang="en">hasImpactLevel</rdfs:label>
    </owl:DatatypeProperty>
    


    <!-- http://www.semanticweb.org/cra/ontologies/AgriWaterMgmt#hasImpactOnStakeholders -->

    <owl:DatatypeProperty rdf:about="http://www.semanticweb.org/cra/ontologies/AgriWaterMgmt#hasImpactOnStakeholders">
        <rdfs:domain rdf:resource="http://www.semanticweb.org/cra/ontologies/AgriWaterMgmt#WaterRights"/>
        <rdfs:domain>
            <owl:Class>
                <owl:unionOf rdf:parseType="Collection">
                    <owl:Restriction>
                        <owl:onProperty rdf:resource="http://www.semanticweb.org/cra/ontologies/AgriWaterMgmt#hasImpactOnStakeholders"/>
                        <owl:hasValue>Negative Impact</owl:hasValue>
                    </owl:Restriction>
                    <owl:Restriction>
                        <owl:onProperty rdf:resource="http://www.semanticweb.org/cra/ontologies/AgriWaterMgmt#hasImpactOnStakeholders"/>
                        <owl:hasValue>Neutral Impact</owl:hasValue>
                    </owl:Restriction>
                    <owl:Restriction>
                        <owl:onProperty rdf:resource="http://www.semanticweb.org/cra/ontologies/AgriWaterMgmt#hasImpactOnStakeholders"/>
                        <owl:hasValue>Positive Impact</owl:hasValue>
                    </owl:Restriction>
                </owl:unionOf>
            </owl:Class>
        </rdfs:domain>
        <rdfs:range rdf:resource="http://www.w3.org/2001/XMLSchema#string"/>
        <rdfs:comment xml:lang="en">Evaluates how water rights impact stakeholders. Its values include &quot;Positive Impact&quot;, &quot;Neutral Impact&quot; and &quot;Negative Impact&quot;.</rdfs:comment>
        <rdfs:label xml:lang="en">hasImpactOnStakeholders</rdfs:label>
    </owl:DatatypeProperty>
    


    <!-- http://www.semanticweb.org/cra/ontologies/AgriWaterMgmt#hasImpactSeverity -->

    <owl:DatatypeProperty rdf:about="http://www.semanticweb.org/cra/ontologies/AgriWaterMgmt#hasImpactSeverity">
        <rdfs:domain rdf:resource="http://www.semanticweb.org/cra/ontologies/AgriWaterMgmt#ClimateChange"/>
        <rdfs:domain>
            <owl:Class>
                <owl:unionOf rdf:parseType="Collection">
                    <owl:Restriction>
                        <owl:onProperty rdf:resource="http://www.semanticweb.org/cra/ontologies/AgriWaterMgmt#hasImpactSeverity"/>
                        <owl:hasValue>High Impact</owl:hasValue>
                    </owl:Restriction>
                    <owl:Restriction>
                        <owl:onProperty rdf:resource="http://www.semanticweb.org/cra/ontologies/AgriWaterMgmt#hasImpactSeverity"/>
                        <owl:hasValue>Low Impact</owl:hasValue>
                    </owl:Restriction>
                    <owl:Restriction>
                        <owl:onProperty rdf:resource="http://www.semanticweb.org/cra/ontologies/AgriWaterMgmt#hasImpactSeverity"/>
                        <owl:hasValue>Moderate Impact</owl:hasValue>
                    </owl:Restriction>
                </owl:unionOf>
            </owl:Class>
        </rdfs:domain>
        <rdfs:range rdf:resource="http://www.w3.org/2001/XMLSchema#string"/>
        <rdfs:comment xml:lang="en">Indicates the severity of climate change effects on agriculture and water resources. Possible values include &quot;Low Impact&quot;, &quot;Moderate Impact&quot;, and &quot;High Impact&quot;.</rdfs:comment>
        <rdfs:label xml:lang="en">hasImpactSeverity</rdfs:label>
    </owl:DatatypeProperty>
    


    <!-- http://www.semanticweb.org/cra/ontologies/AgriWaterMgmt#hasImplementationStatus -->

    <owl:DatatypeProperty rdf:about="http://www.semanticweb.org/cra/ontologies/AgriWaterMgmt#hasImplementationStatus">
        <rdfs:domain rdf:resource="http://www.semanticweb.org/cra/ontologies/AgriWaterMgmt#AgriculturalEngineering"/>
        <rdfs:domain rdf:resource="http://www.semanticweb.org/cra/ontologies/AgriWaterMgmt#WaterEfficiency"/>
        <rdfs:domain rdf:resource="http://www.semanticweb.org/cra/ontologies/AgriWaterMgmt#WaterManagement"/>
        <rdfs:domain>
            <owl:Class>
                <owl:unionOf rdf:parseType="Collection">
                    <owl:Restriction>
                        <owl:onProperty rdf:resource="http://www.semanticweb.org/cra/ontologies/AgriWaterMgmt#hasImplementationStatus"/>
                        <owl:hasValue>Fully Implemented</owl:hasValue>
                    </owl:Restriction>
                    <owl:Restriction>
                        <owl:onProperty rdf:resource="http://www.semanticweb.org/cra/ontologies/AgriWaterMgmt#hasImplementationStatus"/>
                        <owl:hasValue>Not Implemented</owl:hasValue>
                    </owl:Restriction>
                    <owl:Restriction>
                        <owl:onProperty rdf:resource="http://www.semanticweb.org/cra/ontologies/AgriWaterMgmt#hasImplementationStatus"/>
                        <owl:hasValue>Partially Implemented</owl:hasValue>
                    </owl:Restriction>
                </owl:unionOf>
            </owl:Class>
        </rdfs:domain>
        <rdfs:range rdf:resource="http://www.w3.org/2001/XMLSchema#string"/>
        <rdfs:comment xml:lang="en">Current status of implementation of water management practices and water efficiency measures, as well as agricultural engineering technologies in farming practices. Its values include Fully Implemented, Partially Implemented, and Not Implemented.</rdfs:comment>
        <rdfs:label xml:lang="en">hasImplementationStatus</rdfs:label>
    </owl:DatatypeProperty>
    


    <!-- http://www.semanticweb.org/cra/ontologies/AgriWaterMgmt#hasInnovationRate -->

    <owl:DatatypeProperty rdf:about="http://www.semanticweb.org/cra/ontologies/AgriWaterMgmt#hasInnovationRate">
        <rdfs:domain rdf:resource="http://www.semanticweb.org/cra/ontologies/AgriWaterMgmt#AgriculturalEngineering"/>
        <rdfs:domain>
            <owl:Class>
                <owl:unionOf rdf:parseType="Collection">
                    <owl:Restriction>
                        <owl:onProperty rdf:resource="http://www.semanticweb.org/cra/ontologies/AgriWaterMgmt#hasInnovationRate"/>
                        <owl:hasValue>Moderate Innovation</owl:hasValue>
                    </owl:Restriction>
                    <owl:Restriction>
                        <owl:onProperty rdf:resource="http://www.semanticweb.org/cra/ontologies/AgriWaterMgmt#hasInnovationRate"/>
                        <owl:hasValue>Rapid Innovation</owl:hasValue>
                    </owl:Restriction>
                    <owl:Restriction>
                        <owl:onProperty rdf:resource="http://www.semanticweb.org/cra/ontologies/AgriWaterMgmt#hasInnovationRate"/>
                        <owl:hasValue>Slow Innovation</owl:hasValue>
                    </owl:Restriction>
                </owl:unionOf>
            </owl:Class>
        </rdfs:domain>
        <rdfs:range rdf:resource="http://www.w3.org/2001/XMLSchema#string"/>
        <rdfs:comment xml:lang="en">Reflects the rate of innovation and new technology adoption in agricultural engineering. Values include &quot;Slow Innovation&quot;, &quot;Moderate Innovation&quot; and &quot;Rapid Innovation&quot;.</rdfs:comment>
        <rdfs:label xml:lang="en">hasInnovationRate</rdfs:label>
    </owl:DatatypeProperty>
    


    <!-- http://www.semanticweb.org/cra/ontologies/AgriWaterMgmt#hasInstallationComplexity -->

    <owl:DatatypeProperty rdf:about="http://www.semanticweb.org/cra/ontologies/AgriWaterMgmt#hasInstallationComplexity">
        <rdfs:domain rdf:resource="http://www.semanticweb.org/cra/ontologies/AgriWaterMgmt#SubsurfaceIrrigation"/>
        <rdfs:domain>
            <owl:Class>
                <owl:unionOf rdf:parseType="Collection">
                    <owl:Restriction>
                        <owl:onProperty rdf:resource="http://www.semanticweb.org/cra/ontologies/AgriWaterMgmt#hasInstallationComplexity"/>
                        <owl:hasValue>High Complexity</owl:hasValue>
                    </owl:Restriction>
                    <owl:Restriction>
                        <owl:onProperty rdf:resource="http://www.semanticweb.org/cra/ontologies/AgriWaterMgmt#hasInstallationComplexity"/>
                        <owl:hasValue>Low Complexity</owl:hasValue>
                    </owl:Restriction>
                    <owl:Restriction>
                        <owl:onProperty rdf:resource="http://www.semanticweb.org/cra/ontologies/AgriWaterMgmt#hasInstallationComplexity"/>
                        <owl:hasValue>Medium Complexity</owl:hasValue>
                    </owl:Restriction>
                </owl:unionOf>
            </owl:Class>
        </rdfs:domain>
        <rdfs:range rdf:resource="http://www.w3.org/2001/XMLSchema#string"/>
        <rdfs:comment xml:lang="en">Refers to the level of complexity involved in installing subsurface irrigation systems. These systems often require careful placement of pipes below the soil surface. Possible values include &quot;Low Complexity&quot;, &quot;Medium Complexity&quot; and &quot;High Complexity&quot;.</rdfs:comment>
        <rdfs:label xml:lang="en">hasInstallationComplexity</rdfs:label>
    </owl:DatatypeProperty>
    


    <!-- http://www.semanticweb.org/cra/ontologies/AgriWaterMgmt#hasIrrigationDependence -->

    <owl:DatatypeProperty rdf:about="http://www.semanticweb.org/cra/ontologies/AgriWaterMgmt#hasIrrigationDependence">
        <rdfs:domain rdf:resource="http://www.semanticweb.org/cra/ontologies/AgriWaterMgmt#IrrigatedAreas"/>
        <rdfs:domain>
            <owl:Class>
                <owl:unionOf rdf:parseType="Collection">
                    <owl:Restriction>
                        <owl:onProperty rdf:resource="http://www.semanticweb.org/cra/ontologies/AgriWaterMgmt#hasIrrigationDependence"/>
                        <owl:hasValue>High Dependence</owl:hasValue>
                    </owl:Restriction>
                    <owl:Restriction>
                        <owl:onProperty rdf:resource="http://www.semanticweb.org/cra/ontologies/AgriWaterMgmt#hasIrrigationDependence"/>
                        <owl:hasValue>Low Dependence</owl:hasValue>
                    </owl:Restriction>
                    <owl:Restriction>
                        <owl:onProperty rdf:resource="http://www.semanticweb.org/cra/ontologies/AgriWaterMgmt#hasIrrigationDependence"/>
                        <owl:hasValue>Moderate Dependence</owl:hasValue>
                    </owl:Restriction>
                </owl:unionOf>
            </owl:Class>
        </rdfs:domain>
        <rdfs:range rdf:resource="http://www.w3.org/2001/XMLSchema#string"/>
        <rdfs:comment xml:lang="en">Represents the dependence of agriculture in irrigated areas on artificial irrigation systems. Possible values include &quot;High Dependence&quot;, &quot;Moderate Dependence&quot;, and &quot;Low Dependence&quot;.</rdfs:comment>
        <rdfs:label xml:lang="en">hasIrrigationDependence</rdfs:label>
    </owl:DatatypeProperty>
    


    <!-- http://www.semanticweb.org/cra/ontologies/AgriWaterMgmt#hasIrrigationDuration -->

    <owl:DatatypeProperty rdf:about="http://www.semanticweb.org/cra/ontologies/AgriWaterMgmt#hasIrrigationDuration">
        <rdfs:domain rdf:resource="http://www.semanticweb.org/cra/ontologies/AgriWaterMgmt#IrrigationScheduling"/>
        <rdfs:range rdf:resource="http://www.w3.org/2001/XMLSchema#positiveInteger"/>
        <rdfs:comment xml:lang="en">Refers to the duration of each irrigation session, measured in minutes.</rdfs:comment>
        <rdfs:label xml:lang="en">hasIrrigationDuration</rdfs:label>
    </owl:DatatypeProperty>
    


    <!-- http://www.semanticweb.org/cra/ontologies/AgriWaterMgmt#hasIrrigationSchedule -->

    <owl:DatatypeProperty rdf:about="http://www.semanticweb.org/cra/ontologies/AgriWaterMgmt#hasIrrigationSchedule">
        <rdfs:domain rdf:resource="http://www.semanticweb.org/cra/ontologies/AgriWaterMgmt#RegulatedDeficitIrrigation"/>
        <rdfs:domain>
            <owl:Class>
                <owl:unionOf rdf:parseType="Collection">
                    <owl:Restriction>
                        <owl:onProperty rdf:resource="http://www.semanticweb.org/cra/ontologies/AgriWaterMgmt#hasIrrigationSchedule"/>
                        <owl:hasValue>Fixed Schedule</owl:hasValue>
                    </owl:Restriction>
                    <owl:Restriction>
                        <owl:onProperty rdf:resource="http://www.semanticweb.org/cra/ontologies/AgriWaterMgmt#hasIrrigationSchedule"/>
                        <owl:hasValue>Flexible Schedule</owl:hasValue>
                    </owl:Restriction>
                    <owl:Restriction>
                        <owl:onProperty rdf:resource="http://www.semanticweb.org/cra/ontologies/AgriWaterMgmt#hasIrrigationSchedule"/>
                        <owl:hasValue>Seasonal Schedule</owl:hasValue>
                    </owl:Restriction>
                </owl:unionOf>
            </owl:Class>
        </rdfs:domain>
        <rdfs:range rdf:resource="http://www.w3.org/2001/XMLSchema#string"/>
        <rdfs:comment xml:lang="en">Represents the scheduling of water applications in the regulated deficit irrigation system, which strategically withholds water during non-critical growth stages. Values include &quot;Flexible Schedule&quot;, &quot;Fixed Schedule&quot;, and &quot;Seasonal Schedule&quot;.</rdfs:comment>
        <rdfs:label xml:lang="en">hasIrrigationSchedule</rdfs:label>
    </owl:DatatypeProperty>
    


    <!-- http://www.semanticweb.org/cra/ontologies/AgriWaterMgmt#hasLegalCompliance -->

    <owl:DatatypeProperty rdf:about="http://www.semanticweb.org/cra/ontologies/AgriWaterMgmt#hasLegalCompliance">
        <rdfs:domain rdf:resource="http://www.semanticweb.org/cra/ontologies/AgriWaterMgmt#Water"/>
        <rdfs:domain>
            <owl:Class>
                <owl:unionOf rdf:parseType="Collection">
                    <owl:Restriction>
                        <owl:onProperty rdf:resource="http://www.semanticweb.org/cra/ontologies/AgriWaterMgmt#hasLegalCompliance"/>
                        <owl:hasValue>Fully Compliant</owl:hasValue>
                    </owl:Restriction>
                    <owl:Restriction>
                        <owl:onProperty rdf:resource="http://www.semanticweb.org/cra/ontologies/AgriWaterMgmt#hasLegalCompliance"/>
                        <owl:hasValue>Non-Compliant</owl:hasValue>
                    </owl:Restriction>
                    <owl:Restriction>
                        <owl:onProperty rdf:resource="http://www.semanticweb.org/cra/ontologies/AgriWaterMgmt#hasLegalCompliance"/>
                        <owl:hasValue>Partially Compliant</owl:hasValue>
                    </owl:Restriction>
                </owl:unionOf>
            </owl:Class>
        </rdfs:domain>
        <rdfs:range rdf:resource="http://www.w3.org/2001/XMLSchema#string"/>
        <rdfs:comment xml:lang="en">Describes how well sustainable water management practices adhere to legal requirements and environmental standards. Possible values include &quot;Fully Compliant&quot;, &quot;Partially Compliant&quot;, and &quot;Non-Compliant&quot;.</rdfs:comment>
        <rdfs:label xml:lang="en">hasLegalCompliance</rdfs:label>
    </owl:DatatypeProperty>
    


    <!-- http://www.semanticweb.org/cra/ontologies/AgriWaterMgmt#hasLength -->

    <owl:DatatypeProperty rdf:about="http://www.semanticweb.org/cra/ontologies/AgriWaterMgmt#hasLength">
        <rdfs:domain rdf:resource="http://www.semanticweb.org/cra/ontologies/AgriWaterMgmt#Tubings"/>
        <rdfs:range rdf:resource="http://www.w3.org/2001/XMLSchema#decimal"/>
        <rdfs:comment xml:lang="en">Specifies the length of the tubing, measured in meters.</rdfs:comment>
        <rdfs:label xml:lang="en">hasLength</rdfs:label>
    </owl:DatatypeProperty>
    


    <!-- http://www.semanticweb.org/cra/ontologies/AgriWaterMgmt#hasMaintenanceFrequency -->

    <owl:DatatypeProperty rdf:about="http://www.semanticweb.org/cra/ontologies/AgriWaterMgmt#hasMaintenanceFrequency">
        <rdfs:domain rdf:resource="http://www.semanticweb.org/cra/ontologies/AgriWaterMgmt#IrrigationSystems"/>
        <rdfs:domain rdf:resource="http://www.semanticweb.org/cra/ontologies/AgriWaterMgmt#PumpUnit"/>
        <rdfs:domain>
            <owl:Class>
                <owl:unionOf rdf:parseType="Collection">
                    <owl:Restriction>
                        <owl:onProperty rdf:resource="http://www.semanticweb.org/cra/ontologies/AgriWaterMgmt#hasMaintenanceFrequency"/>
                        <owl:hasValue>Annually</owl:hasValue>
                    </owl:Restriction>
                    <owl:Restriction>
                        <owl:onProperty rdf:resource="http://www.semanticweb.org/cra/ontologies/AgriWaterMgmt#hasMaintenanceFrequency"/>
                        <owl:hasValue>Monthly</owl:hasValue>
                    </owl:Restriction>
                    <owl:Restriction>
                        <owl:onProperty rdf:resource="http://www.semanticweb.org/cra/ontologies/AgriWaterMgmt#hasMaintenanceFrequency"/>
                        <owl:hasValue>Quarterly</owl:hasValue>
                    </owl:Restriction>
                </owl:unionOf>
            </owl:Class>
        </rdfs:domain>
        <rdfs:range rdf:resource="http://www.w3.org/2001/XMLSchema#string"/>
        <rdfs:comment xml:lang="en">Indicates the recommended frequency of maintenance for the pump unit or an irrigation system, with values such as &quot;Monthly&quot;, &quot;Quarterly&quot;, or &quot;Annually&quot;.</rdfs:comment>
        <rdfs:label xml:lang="en">hasMaintenanceFrequency</rdfs:label>
    </owl:DatatypeProperty>
    


    <!-- http://www.semanticweb.org/cra/ontologies/AgriWaterMgmt#hasMaterial -->

    <owl:DatatypeProperty rdf:about="http://www.semanticweb.org/cra/ontologies/AgriWaterMgmt#hasMaterial">
        <rdfs:domain rdf:resource="http://www.semanticweb.org/cra/ontologies/AgriWaterMgmt#Tubings"/>
        <rdfs:domain>
            <owl:Class>
                <owl:unionOf rdf:parseType="Collection">
                    <owl:Restriction>
                        <owl:onProperty rdf:resource="http://www.semanticweb.org/cra/ontologies/AgriWaterMgmt#hasMaterial"/>
                        <owl:hasValue>Metal</owl:hasValue>
                    </owl:Restriction>
                    <owl:Restriction>
                        <owl:onProperty rdf:resource="http://www.semanticweb.org/cra/ontologies/AgriWaterMgmt#hasMaterial"/>
                        <owl:hasValue>PVC</owl:hasValue>
                    </owl:Restriction>
                    <owl:Restriction>
                        <owl:onProperty rdf:resource="http://www.semanticweb.org/cra/ontologies/AgriWaterMgmt#hasMaterial"/>
                        <owl:hasValue>Polyethylene</owl:hasValue>
                    </owl:Restriction>
                </owl:unionOf>
            </owl:Class>
        </rdfs:domain>
        <rdfs:range rdf:resource="http://www.w3.org/2001/XMLSchema#string"/>
        <rdfs:comment xml:lang="en">Specifies the material from which the tubing is made, such as &quot;PVC&quot;, &quot;Polyethylene&quot;, or &quot;Metal&quot;.</rdfs:comment>
        <rdfs:label xml:lang="en">hasMaterial</rdfs:label>
    </owl:DatatypeProperty>
    


    <!-- http://www.semanticweb.org/cra/ontologies/AgriWaterMgmt#hasMaterialType -->

    <owl:DatatypeProperty rdf:about="http://www.semanticweb.org/cra/ontologies/AgriWaterMgmt#hasMaterialType">
        <rdfs:domain rdf:resource="http://www.semanticweb.org/cra/ontologies/AgriWaterMgmt#Accessories"/>
        <rdfs:domain>
            <owl:Class>
                <owl:unionOf rdf:parseType="Collection">
                    <owl:Restriction>
                        <owl:onProperty rdf:resource="http://www.semanticweb.org/cra/ontologies/AgriWaterMgmt#hasMaterialType"/>
                        <owl:hasValue>Composite Materials</owl:hasValue>
                    </owl:Restriction>
                    <owl:Restriction>
                        <owl:onProperty rdf:resource="http://www.semanticweb.org/cra/ontologies/AgriWaterMgmt#hasMaterialType"/>
                        <owl:hasValue>Metal</owl:hasValue>
                    </owl:Restriction>
                    <owl:Restriction>
                        <owl:onProperty rdf:resource="http://www.semanticweb.org/cra/ontologies/AgriWaterMgmt#hasMaterialType"/>
                        <owl:hasValue>Plastic</owl:hasValue>
                    </owl:Restriction>
                </owl:unionOf>
            </owl:Class>
        </rdfs:domain>
        <rdfs:range rdf:resource="http://www.w3.org/2001/XMLSchema#string"/>
        <rdfs:comment xml:lang="en">Specifies the type of material used in manufacturing accessories. Values include &quot;Plastic&quot;, &quot;Metal&quot; and &quot;Composite Materials&quot;.</rdfs:comment>
        <rdfs:label xml:lang="en">hasMaterialType</rdfs:label>
    </owl:DatatypeProperty>
    


    <!-- http://www.semanticweb.org/cra/ontologies/AgriWaterMgmt#hasMeasurementPeriod -->

    <owl:DatatypeProperty rdf:about="http://www.semanticweb.org/cra/ontologies/AgriWaterMgmt#hasMeasurementPeriod">
        <rdfs:domain rdf:resource="http://www.semanticweb.org/cra/ontologies/AgriWaterMgmt#CropEvapotranspiration"/>
        <rdfs:domain>
            <owl:Class>
                <owl:unionOf rdf:parseType="Collection">
                    <owl:Restriction>
                        <owl:onProperty rdf:resource="http://www.semanticweb.org/cra/ontologies/AgriWaterMgmt#hasMeasurementPeriod"/>
                        <owl:hasValue>Daily</owl:hasValue>
                    </owl:Restriction>
                    <owl:Restriction>
                        <owl:onProperty rdf:resource="http://www.semanticweb.org/cra/ontologies/AgriWaterMgmt#hasMeasurementPeriod"/>
                        <owl:hasValue>Monthly</owl:hasValue>
                    </owl:Restriction>
                    <owl:Restriction>
                        <owl:onProperty rdf:resource="http://www.semanticweb.org/cra/ontologies/AgriWaterMgmt#hasMeasurementPeriod"/>
                        <owl:hasValue>Weekly</owl:hasValue>
                    </owl:Restriction>
                </owl:unionOf>
            </owl:Class>
        </rdfs:domain>
        <rdfs:range rdf:resource="http://www.w3.org/2001/XMLSchema#string"/>
        <rdfs:comment xml:lang="en">Indicates how frequently evapotranspiration data is collected for the crop. Its values include Daily, Weekly and Monthly.</rdfs:comment>
        <rdfs:label xml:lang="en">hasMeasurementPeriod</rdfs:label>
    </owl:DatatypeProperty>
    


    <!-- http://www.semanticweb.org/cra/ontologies/AgriWaterMgmt#hasMoistureLevel -->

    <owl:DatatypeProperty rdf:about="http://www.semanticweb.org/cra/ontologies/AgriWaterMgmt#hasMoistureLevel">
        <rdfs:domain rdf:resource="http://www.semanticweb.org/cra/ontologies/AgriWaterMgmt#SoilMoisture"/>
        <rdfs:domain>
            <owl:Class>
                <owl:unionOf rdf:parseType="Collection">
                    <owl:Restriction>
                        <owl:onProperty rdf:resource="http://www.semanticweb.org/cra/ontologies/AgriWaterMgmt#hasMoistureLevel"/>
                        <owl:hasValue>Dry</owl:hasValue>
                    </owl:Restriction>
                    <owl:Restriction>
                        <owl:onProperty rdf:resource="http://www.semanticweb.org/cra/ontologies/AgriWaterMgmt#hasMoistureLevel"/>
                        <owl:hasValue>Optimal</owl:hasValue>
                    </owl:Restriction>
                    <owl:Restriction>
                        <owl:onProperty rdf:resource="http://www.semanticweb.org/cra/ontologies/AgriWaterMgmt#hasMoistureLevel"/>
                        <owl:hasValue>Saturated</owl:hasValue>
                    </owl:Restriction>
                </owl:unionOf>
            </owl:Class>
        </rdfs:domain>
        <rdfs:range rdf:resource="http://www.w3.org/2001/XMLSchema#string"/>
        <rdfs:comment xml:lang="en">Represents the current level of moisture in the soil. It indicates how wet or dry the soil is, with possible values such as &quot;Dry&quot;, &quot;Optimal&quot;, and &quot;Saturated&quot;.</rdfs:comment>
        <rdfs:label xml:lang="en">hasMoistureLevel</rdfs:label>
    </owl:DatatypeProperty>
    


    <!-- http://www.semanticweb.org/cra/ontologies/AgriWaterMgmt#hasMoistureRetentionCapacity -->

    <owl:DatatypeProperty rdf:about="http://www.semanticweb.org/cra/ontologies/AgriWaterMgmt#hasMoistureRetentionCapacity">
        <rdfs:domain rdf:resource="http://www.semanticweb.org/cra/ontologies/AgriWaterMgmt#SoilMoisture"/>
        <rdfs:domain>
            <owl:Class>
                <owl:unionOf rdf:parseType="Collection">
                    <owl:Restriction>
                        <owl:onProperty rdf:resource="http://www.semanticweb.org/cra/ontologies/AgriWaterMgmt#hasMoistureRetentionCapacity"/>
                        <owl:hasValue>High Retention</owl:hasValue>
                    </owl:Restriction>
                    <owl:Restriction>
                        <owl:onProperty rdf:resource="http://www.semanticweb.org/cra/ontologies/AgriWaterMgmt#hasMoistureRetentionCapacity"/>
                        <owl:hasValue>Low Retention</owl:hasValue>
                    </owl:Restriction>
                    <owl:Restriction>
                        <owl:onProperty rdf:resource="http://www.semanticweb.org/cra/ontologies/AgriWaterMgmt#hasMoistureRetentionCapacity"/>
                        <owl:hasValue>Medium Retention</owl:hasValue>
                    </owl:Restriction>
                </owl:unionOf>
            </owl:Class>
        </rdfs:domain>
        <rdfs:range rdf:resource="http://www.w3.org/2001/XMLSchema#string"/>
        <rdfs:comment xml:lang="en">Refers to the ability of the soil to retain moisture over time. It ensures that plants receive the necessary water for growth. Possible values can be &quot;Low Retention&quot;, &quot;Medium Retention&quot;, and &quot;High Retention&quot;.</rdfs:comment>
        <rdfs:label xml:lang="en">hasMoistureRetentionCapacity</rdfs:label>
    </owl:DatatypeProperty>
    


    <!-- http://www.semanticweb.org/cra/ontologies/AgriWaterMgmt#hasNutrientContent -->

    <owl:DatatypeProperty rdf:about="http://www.semanticweb.org/cra/ontologies/AgriWaterMgmt#hasNutrientContent">
        <rdfs:domain rdf:resource="http://www.semanticweb.org/cra/ontologies/AgriWaterMgmt#SoilAnalysis"/>
        <rdfs:domain rdf:resource="http://www.semanticweb.org/cra/ontologies/AgriWaterMgmt#SoilQuality"/>
        <rdfs:domain>
            <owl:Class>
                <owl:unionOf rdf:parseType="Collection">
                    <owl:Restriction>
                        <owl:onProperty rdf:resource="http://www.semanticweb.org/cra/ontologies/AgriWaterMgmt#hasNutrientContent"/>
                        <owl:hasValue>High Content</owl:hasValue>
                    </owl:Restriction>
                    <owl:Restriction>
                        <owl:onProperty rdf:resource="http://www.semanticweb.org/cra/ontologies/AgriWaterMgmt#hasNutrientContent"/>
                        <owl:hasValue>Low Content</owl:hasValue>
                    </owl:Restriction>
                    <owl:Restriction>
                        <owl:onProperty rdf:resource="http://www.semanticweb.org/cra/ontologies/AgriWaterMgmt#hasNutrientContent"/>
                        <owl:hasValue>Medium Content</owl:hasValue>
                    </owl:Restriction>
                </owl:unionOf>
            </owl:Class>
        </rdfs:domain>
        <rdfs:range rdf:resource="http://www.w3.org/2001/XMLSchema#string"/>
        <rdfs:comment xml:lang="en">Indicates the levels of essential nutrients in the soil, such as nitrogen, phosphorus, and potassium. Possible values can include ranges like &quot;Low Content&quot;, &quot;Medium Content&quot;, and &quot;High Content&quot;.</rdfs:comment>
        <rdfs:label xml:lang="en">hasNutrientContent</rdfs:label>
    </owl:DatatypeProperty>
    


    <!-- http://www.semanticweb.org/cra/ontologies/AgriWaterMgmt#hasNutrientManagementStrategy -->

    <owl:DatatypeProperty rdf:about="http://www.semanticweb.org/cra/ontologies/AgriWaterMgmt#hasNutrientManagementStrategy">
        <rdfs:domain rdf:resource="http://www.semanticweb.org/cra/ontologies/AgriWaterMgmt#SoilConservation"/>
        <rdfs:domain>
            <owl:Class>
                <owl:unionOf rdf:parseType="Collection">
                    <owl:Restriction>
                        <owl:onProperty rdf:resource="http://www.semanticweb.org/cra/ontologies/AgriWaterMgmt#hasNutrientManagementStrategy"/>
                        <owl:hasValue>Crop Rotation</owl:hasValue>
                    </owl:Restriction>
                    <owl:Restriction>
                        <owl:onProperty rdf:resource="http://www.semanticweb.org/cra/ontologies/AgriWaterMgmt#hasNutrientManagementStrategy"/>
                        <owl:hasValue>Organic Amendments</owl:hasValue>
                    </owl:Restriction>
                    <owl:Restriction>
                        <owl:onProperty rdf:resource="http://www.semanticweb.org/cra/ontologies/AgriWaterMgmt#hasNutrientManagementStrategy"/>
                        <owl:hasValue>Precision Fertilization</owl:hasValue>
                    </owl:Restriction>
                </owl:unionOf>
            </owl:Class>
        </rdfs:domain>
        <rdfs:range rdf:resource="http://www.w3.org/2001/XMLSchema#string"/>
        <rdfs:comment xml:lang="en">Refers to the strategies for managing soil nutrients effectively. It includes &quot;Organic Amendments&quot;, &quot;Crop Rotation&quot;, and &quot;Precision Fertilization&quot;.</rdfs:comment>
        <rdfs:label xml:lang="en">hasNutrientManagementStrategy</rdfs:label>
    </owl:DatatypeProperty>
    


    <!-- http://www.semanticweb.org/cra/ontologies/AgriWaterMgmt#hasOptimizationLevel -->

    <owl:DatatypeProperty rdf:about="http://www.semanticweb.org/cra/ontologies/AgriWaterMgmt#hasOptimizationLevel">
        <rdfs:domain rdf:resource="http://www.semanticweb.org/cra/ontologies/AgriWaterMgmt#WaterManagement"/>
        <rdfs:domain rdf:resource="http://www.semanticweb.org/cra/ontologies/AgriWaterMgmt#WaterOptimization"/>
        <rdfs:domain>
            <owl:Class>
                <owl:unionOf rdf:parseType="Collection">
                    <owl:Restriction>
                        <owl:onProperty rdf:resource="http://www.semanticweb.org/cra/ontologies/AgriWaterMgmt#hasOptimizationLevel"/>
                        <owl:hasValue>High Optimization</owl:hasValue>
                    </owl:Restriction>
                    <owl:Restriction>
                        <owl:onProperty rdf:resource="http://www.semanticweb.org/cra/ontologies/AgriWaterMgmt#hasOptimizationLevel"/>
                        <owl:hasValue>Low Optimization</owl:hasValue>
                    </owl:Restriction>
                    <owl:Restriction>
                        <owl:onProperty rdf:resource="http://www.semanticweb.org/cra/ontologies/AgriWaterMgmt#hasOptimizationLevel"/>
                        <owl:hasValue>Medium Optimization</owl:hasValue>
                    </owl:Restriction>
                </owl:unionOf>
            </owl:Class>
        </rdfs:domain>
        <rdfs:range rdf:resource="http://www.w3.org/2001/XMLSchema#string"/>
        <rdfs:comment xml:lang="en">Degree to which water management practices optimize resource use. It reflects how effectively water resources are utilized through various optimization strategies in both water management and water optimization practices. Its values include &quot;Low Optimization&quot;, &quot;Medium Optimization&quot;, and &quot;High Optimization&quot;.</rdfs:comment>
        <rdfs:label xml:lang="en">hasOptimizationLevel</rdfs:label>
    </owl:DatatypeProperty>
    


    <!-- http://www.semanticweb.org/cra/ontologies/AgriWaterMgmt#hasOrganicMatterContent -->

    <owl:DatatypeProperty rdf:about="http://www.semanticweb.org/cra/ontologies/AgriWaterMgmt#hasOrganicMatterContent">
        <rdfs:domain rdf:resource="http://www.semanticweb.org/cra/ontologies/AgriWaterMgmt#SoilHealth"/>
        <rdfs:domain rdf:resource="http://www.semanticweb.org/cra/ontologies/AgriWaterMgmt#SoilManagement"/>
        <rdfs:domain rdf:resource="http://www.semanticweb.org/cra/ontologies/AgriWaterMgmt#SoilQuality"/>
        <rdfs:range rdf:resource="http://www.w3.org/2001/XMLSchema#decimal"/>
        <rdfs:comment xml:lang="en">Represents the percentage of organic matter in the soil, which is crucial for soil fertility. It is expressed as a percentage.</rdfs:comment>
        <rdfs:label xml:lang="en">hasOrganicMatterContent</rdfs:label>
    </owl:DatatypeProperty>
    


    <!-- http://www.semanticweb.org/cra/ontologies/AgriWaterMgmt#hasOverallEfficiency -->

    <owl:DatatypeProperty rdf:about="http://www.semanticweb.org/cra/ontologies/AgriWaterMgmt#hasOverallEfficiency">
        <rdfs:domain rdf:resource="http://www.semanticweb.org/cra/ontologies/AgriWaterMgmt#Water"/>
        <rdfs:domain>
            <owl:Class>
                <owl:unionOf rdf:parseType="Collection">
                    <owl:Restriction>
                        <owl:onProperty rdf:resource="http://www.semanticweb.org/cra/ontologies/AgriWaterMgmt#hasOverallEfficiency"/>
                        <owl:hasValue>High Efficiency</owl:hasValue>
                    </owl:Restriction>
                    <owl:Restriction>
                        <owl:onProperty rdf:resource="http://www.semanticweb.org/cra/ontologies/AgriWaterMgmt#hasOverallEfficiency"/>
                        <owl:hasValue>Low Efficiency</owl:hasValue>
                    </owl:Restriction>
                    <owl:Restriction>
                        <owl:onProperty rdf:resource="http://www.semanticweb.org/cra/ontologies/AgriWaterMgmt#hasOverallEfficiency"/>
                        <owl:hasValue>Medium Efficiency</owl:hasValue>
                    </owl:Restriction>
                </owl:unionOf>
            </owl:Class>
        </rdfs:domain>
        <rdfs:range rdf:resource="http://www.w3.org/2001/XMLSchema#string"/>
        <rdfs:comment xml:lang="en">Indicates the overall efficiency of sustainable water management practices in optimizing water use. It assesses how effectively water resources are managed to achieve sustainability. Possible values include &quot;Low Efficiency&quot;, &quot;Medium Efficiency&quot;, and &quot;High Efficiency&quot;.</rdfs:comment>
        <rdfs:label xml:lang="en">hasOverallEfficiency</rdfs:label>
    </owl:DatatypeProperty>
    


    <!-- http://www.semanticweb.org/cra/ontologies/AgriWaterMgmt#hasPollutionLevel -->

    <owl:DatatypeProperty rdf:about="http://www.semanticweb.org/cra/ontologies/AgriWaterMgmt#hasPollutionLevel">
        <rdfs:domain rdf:resource="http://www.semanticweb.org/cra/ontologies/AgriWaterMgmt#Environmental_Impact"/>
        <rdfs:domain rdf:resource="http://www.semanticweb.org/cra/ontologies/AgriWaterMgmt#SurfaceWater"/>
        <rdfs:domain>
            <owl:Class>
                <owl:unionOf rdf:parseType="Collection">
                    <owl:Restriction>
                        <owl:onProperty rdf:resource="http://www.semanticweb.org/cra/ontologies/AgriWaterMgmt#hasPollutionLevel"/>
                        <owl:hasValue>High Pollution</owl:hasValue>
                    </owl:Restriction>
                    <owl:Restriction>
                        <owl:onProperty rdf:resource="http://www.semanticweb.org/cra/ontologies/AgriWaterMgmt#hasPollutionLevel"/>
                        <owl:hasValue>Low Pollution</owl:hasValue>
                    </owl:Restriction>
                    <owl:Restriction>
                        <owl:onProperty rdf:resource="http://www.semanticweb.org/cra/ontologies/AgriWaterMgmt#hasPollutionLevel"/>
                        <owl:hasValue>Moderate Pollution</owl:hasValue>
                    </owl:Restriction>
                </owl:unionOf>
            </owl:Class>
        </rdfs:domain>
        <rdfs:range rdf:resource="http://www.w3.org/2001/XMLSchema#string"/>
        <rdfs:comment xml:lang="en">Indicates the level of pollution produced by a specific water management or agricultural practice, that is, the degree of contamination that may affect soil, water, and air quality. Possible values include &quot;Low Pollution&quot;, &quot;Moderate Pollution&quot;, and &quot;High Pollution&quot;.</rdfs:comment>
        <rdfs:label xml:lang="en">hasPollutionLevel</rdfs:label>
    </owl:DatatypeProperty>
    


    <!-- http://www.semanticweb.org/cra/ontologies/AgriWaterMgmt#hasPopulationDensity -->

    <owl:DatatypeProperty rdf:about="http://www.semanticweb.org/cra/ontologies/AgriWaterMgmt#hasPopulationDensity">
        <rdfs:domain rdf:resource="http://www.semanticweb.org/cra/ontologies/AgriWaterMgmt#RuralAreas"/>
        <rdfs:domain>
            <owl:Class>
                <owl:unionOf rdf:parseType="Collection">
                    <owl:Restriction>
                        <owl:onProperty rdf:resource="http://www.semanticweb.org/cra/ontologies/AgriWaterMgmt#hasPopulationDensity"/>
                        <owl:hasValue>High Density</owl:hasValue>
                    </owl:Restriction>
                    <owl:Restriction>
                        <owl:onProperty rdf:resource="http://www.semanticweb.org/cra/ontologies/AgriWaterMgmt#hasPopulationDensity"/>
                        <owl:hasValue>Low Density</owl:hasValue>
                    </owl:Restriction>
                    <owl:Restriction>
                        <owl:onProperty rdf:resource="http://www.semanticweb.org/cra/ontologies/AgriWaterMgmt#hasPopulationDensity"/>
                        <owl:hasValue>Medium Density</owl:hasValue>
                    </owl:Restriction>
                </owl:unionOf>
            </owl:Class>
        </rdfs:domain>
        <rdfs:range rdf:resource="http://www.w3.org/2001/XMLSchema#string"/>
        <rdfs:comment xml:lang="en">Represents the number of people per unit area in rural regions. Values can be categorized as &quot;Low Density&quot;, &quot;Medium Density&quot; and &quot;High Density&quot;.</rdfs:comment>
        <rdfs:label xml:lang="en">hasPopulationDensity</rdfs:label>
    </owl:DatatypeProperty>
    


    <!-- http://www.semanticweb.org/cra/ontologies/AgriWaterMgmt#hasProductionCost -->

    <owl:DatatypeProperty rdf:about="http://www.semanticweb.org/cra/ontologies/AgriWaterMgmt#hasProductionCost">
        <rdfs:domain rdf:resource="http://www.semanticweb.org/cra/ontologies/AgriWaterMgmt#DesalinatedWater"/>
        <rdfs:range rdf:resource="http://www.w3.org/2001/XMLSchema#decimal"/>
        <rdfs:comment xml:lang="en">Indicates the cost associated with producing desalinated water. This helps evaluate the economic feasibility of using desalinated water in agriculture. Values are numeric.</rdfs:comment>
        <rdfs:label xml:lang="en">hasProductionCost</rdfs:label>
    </owl:DatatypeProperty>
    


    <!-- http://www.semanticweb.org/cra/ontologies/AgriWaterMgmt#hasPurityLevel -->

    <owl:DatatypeProperty rdf:about="http://www.semanticweb.org/cra/ontologies/AgriWaterMgmt#hasPurityLevel">
        <rdfs:domain rdf:resource="http://www.semanticweb.org/cra/ontologies/AgriWaterMgmt#DesalinatedWater"/>
        <rdfs:domain>
            <owl:Class>
                <owl:unionOf rdf:parseType="Collection">
                    <owl:Restriction>
                        <owl:onProperty rdf:resource="http://www.semanticweb.org/cra/ontologies/AgriWaterMgmt#hasPurityLevel"/>
                        <owl:hasValue>High Purity</owl:hasValue>
                    </owl:Restriction>
                    <owl:Restriction>
                        <owl:onProperty rdf:resource="http://www.semanticweb.org/cra/ontologies/AgriWaterMgmt#hasPurityLevel"/>
                        <owl:hasValue>Low Purity</owl:hasValue>
                    </owl:Restriction>
                    <owl:Restriction>
                        <owl:onProperty rdf:resource="http://www.semanticweb.org/cra/ontologies/AgriWaterMgmt#hasPurityLevel"/>
                        <owl:hasValue>Moderate Purity</owl:hasValue>
                    </owl:Restriction>
                </owl:unionOf>
            </owl:Class>
        </rdfs:domain>
        <rdfs:range rdf:resource="http://www.w3.org/2001/XMLSchema#string"/>
        <rdfs:comment xml:lang="en">Represents the purity level of desalinated water, for studying how suitable water is for crops. Possible values include &quot;Low Purity&quot;, &quot;Moderate Purity&quot;, and &quot;High Purity&quot;.</rdfs:comment>
        <rdfs:label xml:lang="en">hasPurityLevel</rdfs:label>
    </owl:DatatypeProperty>
    


    <!-- http://www.semanticweb.org/cra/ontologies/AgriWaterMgmt#hasQualityLevel -->

    <owl:DatatypeProperty rdf:about="http://www.semanticweb.org/cra/ontologies/AgriWaterMgmt#hasQualityLevel">
        <rdfs:domain rdf:resource="http://www.semanticweb.org/cra/ontologies/AgriWaterMgmt#DesalinatedWater"/>
        <rdfs:domain rdf:resource="http://www.semanticweb.org/cra/ontologies/AgriWaterMgmt#GroundWater"/>
        <rdfs:domain rdf:resource="http://www.semanticweb.org/cra/ontologies/AgriWaterMgmt#RecycledWater"/>
        <rdfs:domain rdf:resource="http://www.semanticweb.org/cra/ontologies/AgriWaterMgmt#SurfaceWater"/>
        <rdfs:domain rdf:resource="http://www.semanticweb.org/cra/ontologies/AgriWaterMgmt#WaterResources"/>
        <rdfs:domain>
            <owl:Class>
                <owl:unionOf rdf:parseType="Collection">
                    <owl:Restriction>
                        <owl:onProperty rdf:resource="http://www.semanticweb.org/cra/ontologies/AgriWaterMgmt#hasQualityLevel"/>
                        <owl:hasValue>High Quality</owl:hasValue>
                    </owl:Restriction>
                    <owl:Restriction>
                        <owl:onProperty rdf:resource="http://www.semanticweb.org/cra/ontologies/AgriWaterMgmt#hasQualityLevel"/>
                        <owl:hasValue>Low Quality</owl:hasValue>
                    </owl:Restriction>
                    <owl:Restriction>
                        <owl:onProperty rdf:resource="http://www.semanticweb.org/cra/ontologies/AgriWaterMgmt#hasQualityLevel"/>
                        <owl:hasValue>Moderate Quality</owl:hasValue>
                    </owl:Restriction>
                </owl:unionOf>
            </owl:Class>
        </rdfs:domain>
        <rdfs:range rdf:resource="http://www.w3.org/2001/XMLSchema#string"/>
        <rdfs:comment xml:lang="en">Represents the quality level of water resources, which is essential for determining its suitability for agricultural use. Possible values are &quot;Low Quality&quot;, &quot;Moderate Quality&quot;, and &quot;High Quality&quot;.</rdfs:comment>
        <rdfs:label xml:lang="en">hasQualityLevel</rdfs:label>
    </owl:DatatypeProperty>
    


    <!-- http://www.semanticweb.org/cra/ontologies/AgriWaterMgmt#hasRainfallLevel -->

    <owl:DatatypeProperty rdf:about="http://www.semanticweb.org/cra/ontologies/AgriWaterMgmt#hasRainfallLevel">
        <rdfs:domain rdf:resource="http://www.semanticweb.org/cra/ontologies/AgriWaterMgmt#WeatherCondition"/>
        <rdfs:domain>
            <owl:Class>
                <owl:unionOf rdf:parseType="Collection">
                    <owl:Restriction>
                        <owl:onProperty rdf:resource="http://www.semanticweb.org/cra/ontologies/AgriWaterMgmt#hasRainfallLevel"/>
                        <owl:hasValue>High Rainfall</owl:hasValue>
                    </owl:Restriction>
                    <owl:Restriction>
                        <owl:onProperty rdf:resource="http://www.semanticweb.org/cra/ontologies/AgriWaterMgmt#hasRainfallLevel"/>
                        <owl:hasValue>Low Rainfall</owl:hasValue>
                    </owl:Restriction>
                    <owl:Restriction>
                        <owl:onProperty rdf:resource="http://www.semanticweb.org/cra/ontologies/AgriWaterMgmt#hasRainfallLevel"/>
                        <owl:hasValue>Moderate Rainfall</owl:hasValue>
                    </owl:Restriction>
                </owl:unionOf>
            </owl:Class>
        </rdfs:domain>
        <rdfs:range rdf:resource="http://www.w3.org/2001/XMLSchema#string"/>
        <rdfs:comment xml:lang="en">Indicates the average rainfall in a specific region, which is essential for determining natural water availability for crops. Possible values include &quot;Low Rainfall&quot;, &quot;Moderate Rainfall&quot;, and &quot;High Rainfall&quot;.</rdfs:comment>
        <rdfs:label xml:lang="en">hasRainfallLevel</rdfs:label>
    </owl:DatatypeProperty>
    


    <!-- http://www.semanticweb.org/cra/ontologies/AgriWaterMgmt#hasRange -->

    <owl:DatatypeProperty rdf:about="http://www.semanticweb.org/cra/ontologies/AgriWaterMgmt#hasRange">
        <rdfs:domain rdf:resource="http://www.semanticweb.org/cra/ontologies/AgriWaterMgmt#WaterSensors"/>
        <rdfs:domain>
            <owl:Class>
                <owl:unionOf rdf:parseType="Collection">
                    <owl:Restriction>
                        <owl:onProperty rdf:resource="http://www.semanticweb.org/cra/ontologies/AgriWaterMgmt#hasRange"/>
                        <owl:hasValue>0-100 cm</owl:hasValue>
                    </owl:Restriction>
                    <owl:Restriction>
                        <owl:onProperty rdf:resource="http://www.semanticweb.org/cra/ontologies/AgriWaterMgmt#hasRange"/>
                        <owl:hasValue>0-200 cm</owl:hasValue>
                    </owl:Restriction>
                    <owl:Restriction>
                        <owl:onProperty rdf:resource="http://www.semanticweb.org/cra/ontologies/AgriWaterMgmt#hasRange"/>
                        <owl:hasValue>0-50 cm</owl:hasValue>
                    </owl:Restriction>
                </owl:unionOf>
            </owl:Class>
        </rdfs:domain>
        <rdfs:range rdf:resource="http://www.w3.org/2001/XMLSchema#string"/>
        <rdfs:comment xml:lang="en">Defines the range of the sensor, indicating the limits within which it can accurately measure.</rdfs:comment>
        <rdfs:label xml:lang="en">hasRange</rdfs:label>
    </owl:DatatypeProperty>
    


    <!-- http://www.semanticweb.org/cra/ontologies/AgriWaterMgmt#hasRecoveryRate -->

    <owl:DatatypeProperty rdf:about="http://www.semanticweb.org/cra/ontologies/AgriWaterMgmt#hasRecoveryRate">
        <rdfs:domain rdf:resource="http://www.semanticweb.org/cra/ontologies/AgriWaterMgmt#CropWaterStress"/>
        <rdfs:domain>
            <owl:Class>
                <owl:unionOf rdf:parseType="Collection">
                    <owl:Restriction>
                        <owl:onProperty rdf:resource="http://www.semanticweb.org/cra/ontologies/AgriWaterMgmt#hasRecoveryRate"/>
                        <owl:hasValue>Fast Recovery</owl:hasValue>
                    </owl:Restriction>
                    <owl:Restriction>
                        <owl:onProperty rdf:resource="http://www.semanticweb.org/cra/ontologies/AgriWaterMgmt#hasRecoveryRate"/>
                        <owl:hasValue>Moderate Recovery</owl:hasValue>
                    </owl:Restriction>
                    <owl:Restriction>
                        <owl:onProperty rdf:resource="http://www.semanticweb.org/cra/ontologies/AgriWaterMgmt#hasRecoveryRate"/>
                        <owl:hasValue>Slow Recovery</owl:hasValue>
                    </owl:Restriction>
                </owl:unionOf>
            </owl:Class>
        </rdfs:domain>
        <rdfs:range rdf:resource="http://www.w3.org/2001/XMLSchema#string"/>
        <rdfs:comment xml:lang="en">Refers to the crops ability to recover from water stress. Values might include &quot;Fast Recovery&quot;, &quot;Moderate Recovery&quot;, and &quot;Slow Recovery&quot;.</rdfs:comment>
        <rdfs:label xml:lang="en">hasRecoveryRate</rdfs:label>
    </owl:DatatypeProperty>
    


    <!-- http://www.semanticweb.org/cra/ontologies/AgriWaterMgmt#hasRegulatoryFramework -->

    <owl:DatatypeProperty rdf:about="http://www.semanticweb.org/cra/ontologies/AgriWaterMgmt#hasRegulatoryFramework">
        <rdfs:domain rdf:resource="http://www.semanticweb.org/cra/ontologies/AgriWaterMgmt#WaterPolicy"/>
        <rdfs:domain>
            <owl:Class>
                <owl:unionOf rdf:parseType="Collection">
                    <owl:Restriction>
                        <owl:onProperty rdf:resource="http://www.semanticweb.org/cra/ontologies/AgriWaterMgmt#hasRegulatoryFramework"/>
                        <owl:hasValue>Moderate Regulatory Framework</owl:hasValue>
                    </owl:Restriction>
                    <owl:Restriction>
                        <owl:onProperty rdf:resource="http://www.semanticweb.org/cra/ontologies/AgriWaterMgmt#hasRegulatoryFramework"/>
                        <owl:hasValue>Strong Regulatory Framework</owl:hasValue>
                    </owl:Restriction>
                    <owl:Restriction>
                        <owl:onProperty rdf:resource="http://www.semanticweb.org/cra/ontologies/AgriWaterMgmt#hasRegulatoryFramework"/>
                        <owl:hasValue>Weak Regulatory Framework</owl:hasValue>
                    </owl:Restriction>
                </owl:unionOf>
            </owl:Class>
        </rdfs:domain>
        <rdfs:range rdf:resource="http://www.w3.org/2001/XMLSchema#string"/>
        <rdfs:comment xml:lang="en">Indicates the existence of legal and regulatory frameworks governing water use. Its values include &quot;Strong Regulatory Framework&quot;, &quot;Moderate Regulatory Framework&quot; and &quot;Weak Regulatory Framework&quot;.</rdfs:comment>
        <rdfs:label xml:lang="en">hasRegulatoryFramework</rdfs:label>
    </owl:DatatypeProperty>
    


    <!-- http://www.semanticweb.org/cra/ontologies/AgriWaterMgmt#hasRightsType -->

    <owl:DatatypeProperty rdf:about="http://www.semanticweb.org/cra/ontologies/AgriWaterMgmt#hasRightsType">
        <rdfs:domain rdf:resource="http://www.semanticweb.org/cra/ontologies/AgriWaterMgmt#WaterRights"/>
        <rdfs:domain>
            <owl:Class>
                <owl:unionOf rdf:parseType="Collection">
                    <owl:Restriction>
                        <owl:onProperty rdf:resource="http://www.semanticweb.org/cra/ontologies/AgriWaterMgmt#hasRightsType"/>
                        <owl:hasValue>Conditional Rights</owl:hasValue>
                    </owl:Restriction>
                    <owl:Restriction>
                        <owl:onProperty rdf:resource="http://www.semanticweb.org/cra/ontologies/AgriWaterMgmt#hasRightsType"/>
                        <owl:hasValue>Permanent Rights</owl:hasValue>
                    </owl:Restriction>
                    <owl:Restriction>
                        <owl:onProperty rdf:resource="http://www.semanticweb.org/cra/ontologies/AgriWaterMgmt#hasRightsType"/>
                        <owl:hasValue>Temporary Rights</owl:hasValue>
                    </owl:Restriction>
                </owl:unionOf>
            </owl:Class>
        </rdfs:domain>
        <rdfs:range rdf:resource="http://www.w3.org/2001/XMLSchema#string"/>
        <rdfs:comment xml:lang="en">Describes the type of water rights, including &quot;Permanent Rights&quot;, &quot;Temporary Rights&quot; and &quot;Conditional Rights&quot;.</rdfs:comment>
        <rdfs:label xml:lang="en">hasRightsType</rdfs:label>
    </owl:DatatypeProperty>
    


    <!-- http://www.semanticweb.org/cra/ontologies/AgriWaterMgmt#hasSalinityLevel -->

    <owl:DatatypeProperty rdf:about="http://www.semanticweb.org/cra/ontologies/AgriWaterMgmt#hasSalinityLevel">
        <rdfs:domain rdf:resource="http://www.semanticweb.org/cra/ontologies/AgriWaterMgmt#SoilSalinity"/>
        <rdfs:domain>
            <owl:Class>
                <owl:unionOf rdf:parseType="Collection">
                    <owl:Restriction>
                        <owl:onProperty rdf:resource="http://www.semanticweb.org/cra/ontologies/AgriWaterMgmt#hasSalinityLevel"/>
                        <owl:hasValue>High Salinity</owl:hasValue>
                    </owl:Restriction>
                    <owl:Restriction>
                        <owl:onProperty rdf:resource="http://www.semanticweb.org/cra/ontologies/AgriWaterMgmt#hasSalinityLevel"/>
                        <owl:hasValue>Low Salinity</owl:hasValue>
                    </owl:Restriction>
                    <owl:Restriction>
                        <owl:onProperty rdf:resource="http://www.semanticweb.org/cra/ontologies/AgriWaterMgmt#hasSalinityLevel"/>
                        <owl:hasValue>Moderate Salinity</owl:hasValue>
                    </owl:Restriction>
                </owl:unionOf>
            </owl:Class>
        </rdfs:domain>
        <rdfs:range rdf:resource="http://www.w3.org/2001/XMLSchema#string"/>
        <rdfs:comment xml:lang="en">Refers to the concentration of salts in the soil, which can affect plant growth and crop yields. Possible values can include &quot;Low Salinity&quot;, &quot;Moderate Salinity&quot;, and &quot;High Salinity&quot;.</rdfs:comment>
        <rdfs:label xml:lang="en">hasSalinityLevel</rdfs:label>
    </owl:DatatypeProperty>
    


    <!-- http://www.semanticweb.org/cra/ontologies/AgriWaterMgmt#hasSeasonalVariabilitySurface -->

    <owl:DatatypeProperty rdf:about="http://www.semanticweb.org/cra/ontologies/AgriWaterMgmt#hasSeasonalVariabilitySurface">
        <rdfs:domain rdf:resource="http://www.semanticweb.org/cra/ontologies/AgriWaterMgmt#SurfaceWater"/>
        <rdfs:domain>
            <owl:Class>
                <owl:unionOf rdf:parseType="Collection">
                    <owl:Restriction>
                        <owl:onProperty rdf:resource="http://www.semanticweb.org/cra/ontologies/AgriWaterMgmt#hasSeasonalVariabilitySurface"/>
                        <owl:hasValue>High Variability</owl:hasValue>
                    </owl:Restriction>
                    <owl:Restriction>
                        <owl:onProperty rdf:resource="http://www.semanticweb.org/cra/ontologies/AgriWaterMgmt#hasSeasonalVariabilitySurface"/>
                        <owl:hasValue>Low Variability</owl:hasValue>
                    </owl:Restriction>
                    <owl:Restriction>
                        <owl:onProperty rdf:resource="http://www.semanticweb.org/cra/ontologies/AgriWaterMgmt#hasSeasonalVariabilitySurface"/>
                        <owl:hasValue>Moderate Variability</owl:hasValue>
                    </owl:Restriction>
                </owl:unionOf>
            </owl:Class>
        </rdfs:domain>
        <rdfs:range rdf:resource="http://www.w3.org/2001/XMLSchema#string"/>
        <rdfs:comment xml:lang="en">Indicates the level of seasonal variability in the availability of surface water. Possible values include &quot;High Variability&quot;, &quot;Moderate Variability&quot;, and &quot;Low Variability&quot;.</rdfs:comment>
        <rdfs:label xml:lang="en">hasSeasonalVariabilitySurface</rdfs:label>
    </owl:DatatypeProperty>
    


    <!-- http://www.semanticweb.org/cra/ontologies/AgriWaterMgmt#hasSeasonalVariation -->

    <owl:DatatypeProperty rdf:about="http://www.semanticweb.org/cra/ontologies/AgriWaterMgmt#hasSeasonalVariation">
        <rdfs:domain rdf:resource="http://www.semanticweb.org/cra/ontologies/AgriWaterMgmt#CropIrrigationRequirements"/>
        <rdfs:domain>
            <owl:Class>
                <owl:unionOf rdf:parseType="Collection">
                    <owl:Restriction>
                        <owl:onProperty rdf:resource="http://www.semanticweb.org/cra/ontologies/AgriWaterMgmt#hasSeasonalVariation"/>
                        <owl:hasValue>Consistent</owl:hasValue>
                    </owl:Restriction>
                    <owl:Restriction>
                        <owl:onProperty rdf:resource="http://www.semanticweb.org/cra/ontologies/AgriWaterMgmt#hasSeasonalVariation"/>
                        <owl:hasValue>Highly Variable</owl:hasValue>
                    </owl:Restriction>
                    <owl:Restriction>
                        <owl:onProperty rdf:resource="http://www.semanticweb.org/cra/ontologies/AgriWaterMgmt#hasSeasonalVariation"/>
                        <owl:hasValue>Slightly Variable</owl:hasValue>
                    </owl:Restriction>
                </owl:unionOf>
            </owl:Class>
        </rdfs:domain>
        <rdfs:range rdf:resource="http://www.w3.org/2001/XMLSchema#string"/>
        <rdfs:comment xml:lang="en">Refers to how irrigation requirements change throughout the growing season due to climate and crop growth stages. Its values include &quot;Consistent&quot;, &quot;Slightly Variable&quot; and &quot;Highly Variable&quot;.</rdfs:comment>
        <rdfs:label xml:lang="en">hasSeasonalVariation</rdfs:label>
    </owl:DatatypeProperty>
    


    <!-- http://www.semanticweb.org/cra/ontologies/AgriWaterMgmt#hasSensorType -->

    <owl:DatatypeProperty rdf:about="http://www.semanticweb.org/cra/ontologies/AgriWaterMgmt#hasSensorType">
        <rdfs:domain rdf:resource="http://www.semanticweb.org/cra/ontologies/AgriWaterMgmt#WaterSensors"/>
        <rdfs:domain>
            <owl:Class>
                <owl:unionOf rdf:parseType="Collection">
                    <owl:Restriction>
                        <owl:onProperty rdf:resource="http://www.semanticweb.org/cra/ontologies/AgriWaterMgmt#hasSensorType"/>
                        <owl:hasValue>Flow Sensor</owl:hasValue>
                    </owl:Restriction>
                    <owl:Restriction>
                        <owl:onProperty rdf:resource="http://www.semanticweb.org/cra/ontologies/AgriWaterMgmt#hasSensorType"/>
                        <owl:hasValue>Soil Moisture Sensor</owl:hasValue>
                    </owl:Restriction>
                    <owl:Restriction>
                        <owl:onProperty rdf:resource="http://www.semanticweb.org/cra/ontologies/AgriWaterMgmt#hasSensorType"/>
                        <owl:hasValue>Water Quality Sensor</owl:hasValue>
                    </owl:Restriction>
                </owl:unionOf>
            </owl:Class>
        </rdfs:domain>
        <rdfs:range rdf:resource="http://www.w3.org/2001/XMLSchema#string"/>
        <rdfs:comment xml:lang="en">Specifies the type of water sensor, such as &quot;Soil Moisture Sensor&quot;, &quot;Flow Sensor&quot;, or &quot;Water Quality Sensor&quot;.</rdfs:comment>
        <rdfs:label xml:lang="en">hasSensorType</rdfs:label>
    </owl:DatatypeProperty>
    


    <!-- http://www.semanticweb.org/cra/ontologies/AgriWaterMgmt#hasSeverityLevel -->

    <owl:DatatypeProperty rdf:about="http://www.semanticweb.org/cra/ontologies/AgriWaterMgmt#hasSeverityLevel">
        <rdfs:domain rdf:resource="http://www.semanticweb.org/cra/ontologies/AgriWaterMgmt#Drought"/>
        <rdfs:domain>
            <owl:Class>
                <owl:unionOf rdf:parseType="Collection">
                    <owl:Restriction>
                        <owl:onProperty rdf:resource="http://www.semanticweb.org/cra/ontologies/AgriWaterMgmt#hasSeverityLevel"/>
                        <owl:hasValue>Mild Drought</owl:hasValue>
                    </owl:Restriction>
                    <owl:Restriction>
                        <owl:onProperty rdf:resource="http://www.semanticweb.org/cra/ontologies/AgriWaterMgmt#hasSeverityLevel"/>
                        <owl:hasValue>Moderate Drought</owl:hasValue>
                    </owl:Restriction>
                    <owl:Restriction>
                        <owl:onProperty rdf:resource="http://www.semanticweb.org/cra/ontologies/AgriWaterMgmt#hasSeverityLevel"/>
                        <owl:hasValue>Severe Drought</owl:hasValue>
                    </owl:Restriction>
                </owl:unionOf>
            </owl:Class>
        </rdfs:domain>
        <rdfs:range rdf:resource="http://www.w3.org/2001/XMLSchema#string"/>
        <rdfs:comment xml:lang="en">Indicates the severity of drought conditions affecting water resources and agriculture. Possible values include &quot;Mild Drought&quot;, &quot;Moderate Drought&quot;, and &quot;Severe Drought&quot;.</rdfs:comment>
        <rdfs:label xml:lang="en">hasSeverityLevel</rdfs:label>
    </owl:DatatypeProperty>
    


    <!-- http://www.semanticweb.org/cra/ontologies/AgriWaterMgmt#hasSoilFertilityLevel -->

    <owl:DatatypeProperty rdf:about="http://www.semanticweb.org/cra/ontologies/AgriWaterMgmt#hasSoilFertilityLevel">
        <rdfs:domain rdf:resource="http://www.semanticweb.org/cra/ontologies/AgriWaterMgmt#IrrigatedAreas"/>
        <rdfs:domain>
            <owl:Class>
                <owl:unionOf rdf:parseType="Collection">
                    <owl:Restriction>
                        <owl:onProperty rdf:resource="http://www.semanticweb.org/cra/ontologies/AgriWaterMgmt#hasSoilFertilityLevel"/>
                        <owl:hasValue>High Fertility</owl:hasValue>
                    </owl:Restriction>
                    <owl:Restriction>
                        <owl:onProperty rdf:resource="http://www.semanticweb.org/cra/ontologies/AgriWaterMgmt#hasSoilFertilityLevel"/>
                        <owl:hasValue>Low Fertility</owl:hasValue>
                    </owl:Restriction>
                    <owl:Restriction>
                        <owl:onProperty rdf:resource="http://www.semanticweb.org/cra/ontologies/AgriWaterMgmt#hasSoilFertilityLevel"/>
                        <owl:hasValue>Medium Fertility</owl:hasValue>
                    </owl:Restriction>
                </owl:unionOf>
            </owl:Class>
        </rdfs:domain>
        <rdfs:range rdf:resource="http://www.w3.org/2001/XMLSchema#string"/>
        <rdfs:comment xml:lang="en">Indicates the soil fertility level in irrigated areas. Its values include &quot;High Fertility&quot;, &quot;Medium Fertility&quot;, and &quot;Low Fertility&quot;.</rdfs:comment>
        <rdfs:label xml:lang="en">hasSoilFertilityLevel</rdfs:label>
    </owl:DatatypeProperty>
    


    <!-- http://www.semanticweb.org/cra/ontologies/AgriWaterMgmt#hasSoilMicrobialActivity -->

    <owl:DatatypeProperty rdf:about="http://www.semanticweb.org/cra/ontologies/AgriWaterMgmt#hasSoilMicrobialActivity">
        <rdfs:domain rdf:resource="http://www.semanticweb.org/cra/ontologies/AgriWaterMgmt#SoilHealth"/>
        <rdfs:domain>
            <owl:Class>
                <owl:unionOf rdf:parseType="Collection">
                    <owl:Restriction>
                        <owl:onProperty rdf:resource="http://www.semanticweb.org/cra/ontologies/AgriWaterMgmt#hasSoilMicrobialActivity"/>
                        <owl:hasValue>High Microbial Activity</owl:hasValue>
                    </owl:Restriction>
                    <owl:Restriction>
                        <owl:onProperty rdf:resource="http://www.semanticweb.org/cra/ontologies/AgriWaterMgmt#hasSoilMicrobialActivity"/>
                        <owl:hasValue>Low Microbial Activity</owl:hasValue>
                    </owl:Restriction>
                    <owl:Restriction>
                        <owl:onProperty rdf:resource="http://www.semanticweb.org/cra/ontologies/AgriWaterMgmt#hasSoilMicrobialActivity"/>
                        <owl:hasValue>Moderate Microbial Activity</owl:hasValue>
                    </owl:Restriction>
                </owl:unionOf>
            </owl:Class>
        </rdfs:domain>
        <rdfs:range rdf:resource="http://www.w3.org/2001/XMLSchema#string"/>
        <rdfs:comment xml:lang="en">Indicates the level of microbial activity in the soil, which affects nutrients and soil health. Possible values include &quot;Low Microbial Activity&quot;, &quot;Moderate Microbial Activity&quot;, and &quot;High Microbial Activity&quot;.</rdfs:comment>
        <rdfs:label xml:lang="en">hasSoilMicrobialActivity</rdfs:label>
    </owl:DatatypeProperty>
    


    <!-- http://www.semanticweb.org/cra/ontologies/AgriWaterMgmt#hasSoilQuality -->

    <owl:DatatypeProperty rdf:about="http://www.semanticweb.org/cra/ontologies/AgriWaterMgmt#hasSoilQuality">
        <rdfs:domain rdf:resource="http://www.semanticweb.org/cra/ontologies/AgriWaterMgmt#SoilManagement"/>
        <rdfs:domain>
            <owl:Class>
                <owl:unionOf rdf:parseType="Collection">
                    <owl:Restriction>
                        <owl:onProperty rdf:resource="http://www.semanticweb.org/cra/ontologies/AgriWaterMgmt#hasSoilQuality"/>
                        <owl:hasValue>High Quality</owl:hasValue>
                    </owl:Restriction>
                    <owl:Restriction>
                        <owl:onProperty rdf:resource="http://www.semanticweb.org/cra/ontologies/AgriWaterMgmt#hasSoilQuality"/>
                        <owl:hasValue>Low Quality</owl:hasValue>
                    </owl:Restriction>
                    <owl:Restriction>
                        <owl:onProperty rdf:resource="http://www.semanticweb.org/cra/ontologies/AgriWaterMgmt#hasSoilQuality"/>
                        <owl:hasValue>Moderate Quality</owl:hasValue>
                    </owl:Restriction>
                </owl:unionOf>
            </owl:Class>
        </rdfs:domain>
        <rdfs:range rdf:resource="http://www.w3.org/2001/XMLSchema#string"/>
        <rdfs:comment xml:lang="en">Indicates the quality of the soil based on its ability to support plant growth. Possible values include &quot;High Quality&quot;, &quot;Moderate Quality&quot;, and &quot;Low Quality&quot;.</rdfs:comment>
        <rdfs:label xml:lang="en">hasSoilQuality</rdfs:label>
    </owl:DatatypeProperty>
    


    <!-- http://www.semanticweb.org/cra/ontologies/AgriWaterMgmt#hasSoilType -->

    <owl:DatatypeProperty rdf:about="http://www.semanticweb.org/cra/ontologies/AgriWaterMgmt#hasSoilType">
        <rdfs:domain rdf:resource="http://www.semanticweb.org/cra/ontologies/AgriWaterMgmt#SoilManagement"/>
        <rdfs:domain>
            <owl:Class>
                <owl:unionOf rdf:parseType="Collection">
                    <owl:Restriction>
                        <owl:onProperty rdf:resource="http://www.semanticweb.org/cra/ontologies/AgriWaterMgmt#hasSoilType"/>
                        <owl:hasValue>Clay Soil</owl:hasValue>
                    </owl:Restriction>
                    <owl:Restriction>
                        <owl:onProperty rdf:resource="http://www.semanticweb.org/cra/ontologies/AgriWaterMgmt#hasSoilType"/>
                        <owl:hasValue>Loamy Soil</owl:hasValue>
                    </owl:Restriction>
                    <owl:Restriction>
                        <owl:onProperty rdf:resource="http://www.semanticweb.org/cra/ontologies/AgriWaterMgmt#hasSoilType"/>
                        <owl:hasValue>Sandy Soil</owl:hasValue>
                    </owl:Restriction>
                    <owl:Restriction>
                        <owl:onProperty rdf:resource="http://www.semanticweb.org/cra/ontologies/AgriWaterMgmt#hasSoilType"/>
                        <owl:hasValue>Silty Soil</owl:hasValue>
                    </owl:Restriction>
                </owl:unionOf>
            </owl:Class>
        </rdfs:domain>
        <rdfs:range rdf:resource="http://www.w3.org/2001/XMLSchema#string"/>
        <rdfs:comment xml:lang="en">Represents the type of soil present in a specific area. Possible values include &quot;Sandy Soil&quot;, &quot;Clay Soil&quot;, &quot;Loamy Soil&quot;, and &quot;Silty Soil&quot;.</rdfs:comment>
        <rdfs:label xml:lang="en">hasSoilType</rdfs:label>
    </owl:DatatypeProperty>
    


    <!-- http://www.semanticweb.org/cra/ontologies/AgriWaterMgmt#hasSprayRadius -->

    <owl:DatatypeProperty rdf:about="http://www.semanticweb.org/cra/ontologies/AgriWaterMgmt#hasSprayRadius">
        <rdfs:domain rdf:resource="http://www.semanticweb.org/cra/ontologies/AgriWaterMgmt#SprinklerHead"/>
        <rdfs:range rdf:resource="http://www.w3.org/2001/XMLSchema#decimal"/>
        <rdfs:comment xml:lang="en">Specifies the spray radius of the sprinkler head, measured in meters. It indicates the maximum distance that water can be distributed from the sprinkler head.</rdfs:comment>
        <rdfs:label xml:lang="en">hasSprayRadius</rdfs:label>
    </owl:DatatypeProperty>
    


    <!-- http://www.semanticweb.org/cra/ontologies/AgriWaterMgmt#hasSprinklerRange -->

    <owl:DatatypeProperty rdf:about="http://www.semanticweb.org/cra/ontologies/AgriWaterMgmt#hasSprinklerRange">
        <rdfs:domain rdf:resource="http://www.semanticweb.org/cra/ontologies/AgriWaterMgmt#SprinklerIrrigation"/>
        <rdfs:domain>
            <owl:Class>
                <owl:unionOf rdf:parseType="Collection">
                    <owl:Restriction>
                        <owl:onProperty rdf:resource="http://www.semanticweb.org/cra/ontologies/AgriWaterMgmt#hasSprinklerRange"/>
                        <owl:hasValue>Long Range</owl:hasValue>
                    </owl:Restriction>
                    <owl:Restriction>
                        <owl:onProperty rdf:resource="http://www.semanticweb.org/cra/ontologies/AgriWaterMgmt#hasSprinklerRange"/>
                        <owl:hasValue>Medium Range</owl:hasValue>
                    </owl:Restriction>
                    <owl:Restriction>
                        <owl:onProperty rdf:resource="http://www.semanticweb.org/cra/ontologies/AgriWaterMgmt#hasSprinklerRange"/>
                        <owl:hasValue>Short Range</owl:hasValue>
                    </owl:Restriction>
                </owl:unionOf>
            </owl:Class>
        </rdfs:domain>
        <rdfs:range rdf:resource="http://www.w3.org/2001/XMLSchema#string"/>
        <rdfs:comment xml:lang="en">Refers to the range of the sprinklers used in the system, that is, the distance covered by the spray, which can be adjusted based on the type of crop and land size. The values can be &quot;Short Range&quot;, &quot;Medium Range&quot;, or &quot;Long Range&quot;.</rdfs:comment>
        <rdfs:label xml:lang="en">hasSprinklerRange</rdfs:label>
    </owl:DatatypeProperty>
    


    <!-- http://www.semanticweb.org/cra/ontologies/AgriWaterMgmt#hasStorageCapacity -->

    <owl:DatatypeProperty rdf:about="http://www.semanticweb.org/cra/ontologies/AgriWaterMgmt#hasStorageCapacity">
        <rdfs:domain rdf:resource="http://www.semanticweb.org/cra/ontologies/AgriWaterMgmt#RainwaterHarvesting"/>
        <rdfs:range rdf:resource="http://www.w3.org/2001/XMLSchema#positiveInteger"/>
        <rdfs:comment xml:lang="en">Indicates the maximum volume of rainwater that can be stored in the harvesting system, expressed in liters as a positive integer.</rdfs:comment>
        <rdfs:label xml:lang="en">hasStorageCapacity</rdfs:label>
    </owl:DatatypeProperty>
    


    <!-- http://www.semanticweb.org/cra/ontologies/AgriWaterMgmt#hasSustainabilityRating -->

    <owl:DatatypeProperty rdf:about="http://www.semanticweb.org/cra/ontologies/AgriWaterMgmt#hasSustainabilityRating">
        <rdfs:domain rdf:resource="http://www.semanticweb.org/cra/ontologies/AgriWaterMgmt#SustainabilityAndEnvironmentalImpact"/>
        <rdfs:domain rdf:resource="http://www.semanticweb.org/cra/ontologies/AgriWaterMgmt#SustainableAgriculture"/>
        <rdfs:domain rdf:resource="http://www.semanticweb.org/cra/ontologies/AgriWaterMgmt#WaterManagement"/>
        <rdfs:domain>
            <owl:Class>
                <owl:unionOf rdf:parseType="Collection">
                    <owl:Restriction>
                        <owl:onProperty rdf:resource="http://www.semanticweb.org/cra/ontologies/AgriWaterMgmt#hasSustainabilityRating"/>
                        <owl:hasValue>High Sustainability</owl:hasValue>
                    </owl:Restriction>
                    <owl:Restriction>
                        <owl:onProperty rdf:resource="http://www.semanticweb.org/cra/ontologies/AgriWaterMgmt#hasSustainabilityRating"/>
                        <owl:hasValue>Low Sustainability</owl:hasValue>
                    </owl:Restriction>
                    <owl:Restriction>
                        <owl:onProperty rdf:resource="http://www.semanticweb.org/cra/ontologies/AgriWaterMgmt#hasSustainabilityRating"/>
                        <owl:hasValue>Moderate Sustainability</owl:hasValue>
                    </owl:Restriction>
                </owl:unionOf>
            </owl:Class>
        </rdfs:domain>
        <rdfs:range rdf:resource="http://www.w3.org/2001/XMLSchema#string"/>
        <rdfs:comment xml:lang="en">The sustainability level of water management practices in the long term. Its values include &quot;Low Sustainability&quot;, &quot;Moderate Sustainability&quot;, and &quot;High Sustainability&quot;.</rdfs:comment>
        <rdfs:label xml:lang="en">hasSustainabilityRating</rdfs:label>
    </owl:DatatypeProperty>
    


    <!-- http://www.semanticweb.org/cra/ontologies/AgriWaterMgmt#hasTechnologicalAdvancement -->

    <owl:DatatypeProperty rdf:about="http://www.semanticweb.org/cra/ontologies/AgriWaterMgmt#hasTechnologicalAdvancement">
        <rdfs:domain rdf:resource="http://www.semanticweb.org/cra/ontologies/AgriWaterMgmt#AgriculturalEngineering"/>
        <rdfs:domain rdf:resource="http://www.semanticweb.org/cra/ontologies/AgriWaterMgmt#PrecisionAgriculture"/>
        <rdfs:domain rdf:resource="http://www.semanticweb.org/cra/ontologies/AgriWaterMgmt#WaterOptimization"/>
        <rdfs:domain>
            <owl:Class>
                <owl:unionOf rdf:parseType="Collection">
                    <owl:Restriction>
                        <owl:onProperty rdf:resource="http://www.semanticweb.org/cra/ontologies/AgriWaterMgmt#hasTechnologicalAdvancement"/>
                        <owl:hasValue>High Tech</owl:hasValue>
                    </owl:Restriction>
                    <owl:Restriction>
                        <owl:onProperty rdf:resource="http://www.semanticweb.org/cra/ontologies/AgriWaterMgmt#hasTechnologicalAdvancement"/>
                        <owl:hasValue>Low Tech</owl:hasValue>
                    </owl:Restriction>
                    <owl:Restriction>
                        <owl:onProperty rdf:resource="http://www.semanticweb.org/cra/ontologies/AgriWaterMgmt#hasTechnologicalAdvancement"/>
                        <owl:hasValue>Moderate Tech</owl:hasValue>
                    </owl:Restriction>
                </owl:unionOf>
            </owl:Class>
        </rdfs:domain>
        <rdfs:range rdf:resource="http://www.w3.org/2001/XMLSchema#string"/>
        <rdfs:comment xml:lang="en">Describes the level and sophistication of technology involved in water optimization and other agricultural practices. Its values include &quot;Low Tech&quot;, &quot;Moderate Tech&quot;, and &quot;High Tech&quot;.</rdfs:comment>
        <rdfs:label xml:lang="en">hasTechnologicalAdvancement</rdfs:label>
    </owl:DatatypeProperty>
    


    <!-- http://www.semanticweb.org/cra/ontologies/AgriWaterMgmt#hasTechnologyType -->

    <owl:DatatypeProperty rdf:about="http://www.semanticweb.org/cra/ontologies/AgriWaterMgmt#hasTechnologyType">
        <rdfs:domain rdf:resource="http://www.semanticweb.org/cra/ontologies/AgriWaterMgmt#IrrigationTechnology"/>
        <rdfs:domain>
            <owl:Class>
                <owl:unionOf rdf:parseType="Collection">
                    <owl:Restriction>
                        <owl:onProperty rdf:resource="http://www.semanticweb.org/cra/ontologies/AgriWaterMgmt#hasTechnologyType"/>
                        <owl:hasValue>Drip Irrigation</owl:hasValue>
                    </owl:Restriction>
                    <owl:Restriction>
                        <owl:onProperty rdf:resource="http://www.semanticweb.org/cra/ontologies/AgriWaterMgmt#hasTechnologyType"/>
                        <owl:hasValue>Regulated Deficit Irrigation</owl:hasValue>
                    </owl:Restriction>
                    <owl:Restriction>
                        <owl:onProperty rdf:resource="http://www.semanticweb.org/cra/ontologies/AgriWaterMgmt#hasTechnologyType"/>
                        <owl:hasValue>Sprinkler Irrigation</owl:hasValue>
                    </owl:Restriction>
                    <owl:Restriction>
                        <owl:onProperty rdf:resource="http://www.semanticweb.org/cra/ontologies/AgriWaterMgmt#hasTechnologyType"/>
                        <owl:hasValue>Subsurface Irrigation</owl:hasValue>
                    </owl:Restriction>
                    <owl:Restriction>
                        <owl:onProperty rdf:resource="http://www.semanticweb.org/cra/ontologies/AgriWaterMgmt#hasTechnologyType"/>
                        <owl:hasValue>Surface Irrigation</owl:hasValue>
                    </owl:Restriction>
                </owl:unionOf>
            </owl:Class>
        </rdfs:domain>
        <rdfs:range rdf:resource="http://www.w3.org/2001/XMLSchema#string"/>
        <rdfs:comment xml:lang="en">Specifies the type of irrigation technology used, such as &quot;Drip Irrigation&quot;, Localized Irrigation, Regulated Deficit Irrigation, &quot;Sprinkler Irrigation&quot;, &quot;Surface Irrigation&quot;, or &quot;Subsurface Irrigation&quot;.</rdfs:comment>
        <rdfs:label xml:lang="en">hasTechnologyType</rdfs:label>
    </owl:DatatypeProperty>
    


    <!-- http://www.semanticweb.org/cra/ontologies/AgriWaterMgmt#hasTemperatureRange -->

    <owl:DatatypeProperty rdf:about="http://www.semanticweb.org/cra/ontologies/AgriWaterMgmt#hasTemperatureRange">
        <rdfs:domain rdf:resource="http://www.semanticweb.org/cra/ontologies/AgriWaterMgmt#WeatherCondition"/>
        <rdfs:domain>
            <owl:Class>
                <owl:unionOf rdf:parseType="Collection">
                    <owl:Restriction>
                        <owl:onProperty rdf:resource="http://www.semanticweb.org/cra/ontologies/AgriWaterMgmt#hasTemperatureRange"/>
                        <owl:hasValue>High Temperature Range</owl:hasValue>
                    </owl:Restriction>
                    <owl:Restriction>
                        <owl:onProperty rdf:resource="http://www.semanticweb.org/cra/ontologies/AgriWaterMgmt#hasTemperatureRange"/>
                        <owl:hasValue>Low Temperature Range</owl:hasValue>
                    </owl:Restriction>
                    <owl:Restriction>
                        <owl:onProperty rdf:resource="http://www.semanticweb.org/cra/ontologies/AgriWaterMgmt#hasTemperatureRange"/>
                        <owl:hasValue>Moderate Temperature Range</owl:hasValue>
                    </owl:Restriction>
                </owl:unionOf>
            </owl:Class>
        </rdfs:domain>
        <rdfs:range rdf:resource="http://www.w3.org/2001/XMLSchema#string"/>
        <rdfs:comment xml:lang="en">Describes the typical range of temperatures in an area, influencing plant growth and water needs. Possible values include &quot;Low Temperature Range&quot;, &quot;Moderate Temperature Range&quot;, and &quot;High Temperature Range&quot;.</rdfs:comment>
        <rdfs:label xml:lang="en">hasTemperatureRange</rdfs:label>
    </owl:DatatypeProperty>
    


    <!-- http://www.semanticweb.org/cra/ontologies/AgriWaterMgmt#hasTreatmentLevel -->

    <owl:DatatypeProperty rdf:about="http://www.semanticweb.org/cra/ontologies/AgriWaterMgmt#hasTreatmentLevel">
        <rdfs:domain rdf:resource="http://www.semanticweb.org/cra/ontologies/AgriWaterMgmt#RecycledWater"/>
        <rdfs:domain>
            <owl:Class>
                <owl:unionOf rdf:parseType="Collection">
                    <owl:Restriction>
                        <owl:onProperty rdf:resource="http://www.semanticweb.org/cra/ontologies/AgriWaterMgmt#hasTreatmentLevel"/>
                        <owl:hasValue>Primary</owl:hasValue>
                    </owl:Restriction>
                    <owl:Restriction>
                        <owl:onProperty rdf:resource="http://www.semanticweb.org/cra/ontologies/AgriWaterMgmt#hasTreatmentLevel"/>
                        <owl:hasValue>Secondary</owl:hasValue>
                    </owl:Restriction>
                    <owl:Restriction>
                        <owl:onProperty rdf:resource="http://www.semanticweb.org/cra/ontologies/AgriWaterMgmt#hasTreatmentLevel"/>
                        <owl:hasValue>Tertiary</owl:hasValue>
                    </owl:Restriction>
                </owl:unionOf>
            </owl:Class>
        </rdfs:domain>
        <rdfs:range rdf:resource="http://www.w3.org/2001/XMLSchema#string"/>
        <rdfs:comment xml:lang="en">Indicates the level of treatment applied to recycled water, which determines its safety for irrigation use. Possible values include &quot;Primary&quot;, &quot;Secondary&quot;, and &quot;Tertiary&quot;.</rdfs:comment>
        <rdfs:label xml:lang="en">hasTreatmentLevel</rdfs:label>
    </owl:DatatypeProperty>
    


    <!-- http://www.semanticweb.org/cra/ontologies/AgriWaterMgmt#hasType -->

    <owl:DatatypeProperty rdf:about="http://www.semanticweb.org/cra/ontologies/AgriWaterMgmt#hasType">
        <rdfs:domain rdf:resource="http://www.semanticweb.org/cra/ontologies/AgriWaterMgmt#SprinklerHead"/>
        <rdfs:domain>
            <owl:Class>
                <owl:unionOf rdf:parseType="Collection">
                    <owl:Restriction>
                        <owl:onProperty rdf:resource="http://www.semanticweb.org/cra/ontologies/AgriWaterMgmt#hasType"/>
                        <owl:hasValue>Fixed</owl:hasValue>
                    </owl:Restriction>
                    <owl:Restriction>
                        <owl:onProperty rdf:resource="http://www.semanticweb.org/cra/ontologies/AgriWaterMgmt#hasType"/>
                        <owl:hasValue>Oscillating</owl:hasValue>
                    </owl:Restriction>
                    <owl:Restriction>
                        <owl:onProperty rdf:resource="http://www.semanticweb.org/cra/ontologies/AgriWaterMgmt#hasType"/>
                        <owl:hasValue>Rotary</owl:hasValue>
                    </owl:Restriction>
                </owl:unionOf>
            </owl:Class>
        </rdfs:domain>
        <rdfs:range rdf:resource="http://www.w3.org/2001/XMLSchema#string"/>
        <rdfs:label xml:lang="en">hasType</rdfs:label>
    </owl:DatatypeProperty>
    


    <!-- http://www.semanticweb.org/cra/ontologies/AgriWaterMgmt#hasUsageLevel -->

    <owl:DatatypeProperty rdf:about="http://www.semanticweb.org/cra/ontologies/AgriWaterMgmt#hasUsageLevel">
        <rdfs:domain rdf:resource="http://www.semanticweb.org/cra/ontologies/AgriWaterMgmt#WaterUse"/>
        <rdfs:domain>
            <owl:Class>
                <owl:unionOf rdf:parseType="Collection">
                    <owl:Restriction>
                        <owl:onProperty rdf:resource="http://www.semanticweb.org/cra/ontologies/AgriWaterMgmt#hasUsageLevel"/>
                        <owl:hasValue>High Usage</owl:hasValue>
                    </owl:Restriction>
                    <owl:Restriction>
                        <owl:onProperty rdf:resource="http://www.semanticweb.org/cra/ontologies/AgriWaterMgmt#hasUsageLevel"/>
                        <owl:hasValue>Low Usage</owl:hasValue>
                    </owl:Restriction>
                    <owl:Restriction>
                        <owl:onProperty rdf:resource="http://www.semanticweb.org/cra/ontologies/AgriWaterMgmt#hasUsageLevel"/>
                        <owl:hasValue>Medium Usage</owl:hasValue>
                    </owl:Restriction>
                </owl:unionOf>
            </owl:Class>
        </rdfs:domain>
        <rdfs:range rdf:resource="http://www.w3.org/2001/XMLSchema#string"/>
        <rdfs:comment xml:lang="en">Indicates the level of water use in specific agricultural practices. The values include &quot;Low Usage,&quot; &quot;Medium Usage&quot; and &quot;High Usage&quot;.</rdfs:comment>
        <rdfs:label xml:lang="en">hasUsageLevel</rdfs:label>
    </owl:DatatypeProperty>
    


    <!-- http://www.semanticweb.org/cra/ontologies/AgriWaterMgmt#hasUsagePotential -->

    <owl:DatatypeProperty rdf:about="http://www.semanticweb.org/cra/ontologies/AgriWaterMgmt#hasUsagePotential">
        <rdfs:domain rdf:resource="http://www.semanticweb.org/cra/ontologies/AgriWaterMgmt#RecycledWater"/>
        <rdfs:domain>
            <owl:Class>
                <owl:unionOf rdf:parseType="Collection">
                    <owl:Restriction>
                        <owl:onProperty rdf:resource="http://www.semanticweb.org/cra/ontologies/AgriWaterMgmt#hasUsagePotential"/>
                        <owl:hasValue>High Potential</owl:hasValue>
                    </owl:Restriction>
                    <owl:Restriction>
                        <owl:onProperty rdf:resource="http://www.semanticweb.org/cra/ontologies/AgriWaterMgmt#hasUsagePotential"/>
                        <owl:hasValue>Low Potential</owl:hasValue>
                    </owl:Restriction>
                    <owl:Restriction>
                        <owl:onProperty rdf:resource="http://www.semanticweb.org/cra/ontologies/AgriWaterMgmt#hasUsagePotential"/>
                        <owl:hasValue>Moderate Potential</owl:hasValue>
                    </owl:Restriction>
                </owl:unionOf>
            </owl:Class>
        </rdfs:domain>
        <rdfs:range rdf:resource="http://www.w3.org/2001/XMLSchema#string"/>
        <rdfs:comment xml:lang="en">Indicates the potential for using recycled water in agricultural practices based on its quality and treatment level. Values include &quot;High Potential&quot;, &quot;Moderate Potential&quot;, and &quot;Low Potential&quot;.</rdfs:comment>
        <rdfs:label xml:lang="en">hasUsagePotential</rdfs:label>
    </owl:DatatypeProperty>
    


    <!-- http://www.semanticweb.org/cra/ontologies/AgriWaterMgmt#hasVegetationPresence -->

    <owl:DatatypeProperty rdf:about="http://www.semanticweb.org/cra/ontologies/AgriWaterMgmt#hasVegetationPresence">
        <rdfs:domain rdf:resource="http://www.semanticweb.org/cra/ontologies/AgriWaterMgmt#AridRegions"/>
        <rdfs:domain>
            <owl:Class>
                <owl:unionOf rdf:parseType="Collection">
                    <owl:Restriction>
                        <owl:onProperty rdf:resource="http://www.semanticweb.org/cra/ontologies/AgriWaterMgmt#hasVegetationPresence"/>
                        <owl:hasValue>Minimal Presence</owl:hasValue>
                    </owl:Restriction>
                    <owl:Restriction>
                        <owl:onProperty rdf:resource="http://www.semanticweb.org/cra/ontologies/AgriWaterMgmt#hasVegetationPresence"/>
                        <owl:hasValue>No Presence</owl:hasValue>
                    </owl:Restriction>
                    <owl:Restriction>
                        <owl:onProperty rdf:resource="http://www.semanticweb.org/cra/ontologies/AgriWaterMgmt#hasVegetationPresence"/>
                        <owl:hasValue>Sparse Presence</owl:hasValue>
                    </owl:Restriction>
                </owl:unionOf>
            </owl:Class>
        </rdfs:domain>
        <rdfs:range rdf:resource="http://www.w3.org/2001/XMLSchema#string"/>
        <rdfs:comment xml:lang="en">Represents the level of vegetation presence in arid regions, as it impacts water conservation and land use. Values might include &quot;Sparse Presence&quot;, &quot;Minimal Presence&quot; and &quot;No Presence&quot;.</rdfs:comment>
        <rdfs:label xml:lang="en">hasVegetationPresence</rdfs:label>
    </owl:DatatypeProperty>
    


    <!-- http://www.semanticweb.org/cra/ontologies/AgriWaterMgmt#hasWaterAvailability -->

    <owl:DatatypeProperty rdf:about="http://www.semanticweb.org/cra/ontologies/AgriWaterMgmt#hasWaterAvailability">
        <rdfs:domain rdf:resource="http://www.semanticweb.org/cra/ontologies/AgriWaterMgmt#GroundWater"/>
        <rdfs:domain rdf:resource="http://www.semanticweb.org/cra/ontologies/AgriWaterMgmt#Regions"/>
        <rdfs:domain rdf:resource="http://www.semanticweb.org/cra/ontologies/AgriWaterMgmt#WaterResources"/>
        <rdfs:domain>
            <owl:Class>
                <owl:unionOf rdf:parseType="Collection">
                    <owl:Restriction>
                        <owl:onProperty rdf:resource="http://www.semanticweb.org/cra/ontologies/AgriWaterMgmt#hasWaterAvailability"/>
                        <owl:hasValue>High Availability</owl:hasValue>
                    </owl:Restriction>
                    <owl:Restriction>
                        <owl:onProperty rdf:resource="http://www.semanticweb.org/cra/ontologies/AgriWaterMgmt#hasWaterAvailability"/>
                        <owl:hasValue>Low Availability</owl:hasValue>
                    </owl:Restriction>
                    <owl:Restriction>
                        <owl:onProperty rdf:resource="http://www.semanticweb.org/cra/ontologies/AgriWaterMgmt#hasWaterAvailability"/>
                        <owl:hasValue>Moderate Availability</owl:hasValue>
                    </owl:Restriction>
                </owl:unionOf>
            </owl:Class>
        </rdfs:domain>
        <rdfs:range rdf:resource="http://www.w3.org/2001/XMLSchema#string"/>
        <rdfs:comment xml:lang="en">Describes the water availability in a region. Possible values include &quot;Low Availability&quot;, &quot;Moderate Availability&quot;, and &quot;High Availability&quot;.</rdfs:comment>
        <rdfs:label xml:lang="en">hasWaterAvailability</rdfs:label>
    </owl:DatatypeProperty>
    


    <!-- http://www.semanticweb.org/cra/ontologies/AgriWaterMgmt#hasWaterDemand -->

    <owl:DatatypeProperty rdf:about="http://www.semanticweb.org/cra/ontologies/AgriWaterMgmt#hasWaterDemand">
        <rdfs:domain rdf:resource="http://www.semanticweb.org/cra/ontologies/AgriWaterMgmt#CropIrrigationRequirements"/>
        <rdfs:domain rdf:resource="http://www.semanticweb.org/cra/ontologies/AgriWaterMgmt#Crops"/>
        <rdfs:domain>
            <owl:Class>
                <owl:unionOf rdf:parseType="Collection">
                    <owl:Restriction>
                        <owl:onProperty rdf:resource="http://www.semanticweb.org/cra/ontologies/AgriWaterMgmt#hasWaterDemand"/>
                        <owl:hasValue>High Demand</owl:hasValue>
                    </owl:Restriction>
                    <owl:Restriction>
                        <owl:onProperty rdf:resource="http://www.semanticweb.org/cra/ontologies/AgriWaterMgmt#hasWaterDemand"/>
                        <owl:hasValue>Low Demand</owl:hasValue>
                    </owl:Restriction>
                    <owl:Restriction>
                        <owl:onProperty rdf:resource="http://www.semanticweb.org/cra/ontologies/AgriWaterMgmt#hasWaterDemand"/>
                        <owl:hasValue>Medium Demand</owl:hasValue>
                    </owl:Restriction>
                </owl:unionOf>
            </owl:Class>
        </rdfs:domain>
        <rdfs:range rdf:resource="http://www.w3.org/2001/XMLSchema#string"/>
        <rdfs:comment xml:lang="en">Represents the amount of water required by a crop for optimal growth. Possible values include &quot;Low Demand&quot;, &quot;Medium Demand&quot; and &quot;High Demand&quot;.</rdfs:comment>
        <rdfs:label xml:lang="en">hasWaterDemand</rdfs:label>
    </owl:DatatypeProperty>
    


    <!-- http://www.semanticweb.org/cra/ontologies/AgriWaterMgmt#hasWaterDistributionMethod -->

    <owl:DatatypeProperty rdf:about="http://www.semanticweb.org/cra/ontologies/AgriWaterMgmt#hasWaterDistributionMethod">
        <rdfs:domain rdf:resource="http://www.semanticweb.org/cra/ontologies/AgriWaterMgmt#IrrigationSystems"/>
        <rdfs:domain>
            <owl:Class>
                <owl:unionOf rdf:parseType="Collection">
                    <owl:Restriction>
                        <owl:onProperty rdf:resource="http://www.semanticweb.org/cra/ontologies/AgriWaterMgmt#hasWaterDistributionMethod"/>
                        <owl:hasValue>Drip</owl:hasValue>
                    </owl:Restriction>
                    <owl:Restriction>
                        <owl:onProperty rdf:resource="http://www.semanticweb.org/cra/ontologies/AgriWaterMgmt#hasWaterDistributionMethod"/>
                        <owl:hasValue>Sprinkler</owl:hasValue>
                    </owl:Restriction>
                    <owl:Restriction>
                        <owl:onProperty rdf:resource="http://www.semanticweb.org/cra/ontologies/AgriWaterMgmt#hasWaterDistributionMethod"/>
                        <owl:hasValue>Subsurface</owl:hasValue>
                    </owl:Restriction>
                    <owl:Restriction>
                        <owl:onProperty rdf:resource="http://www.semanticweb.org/cra/ontologies/AgriWaterMgmt#hasWaterDistributionMethod"/>
                        <owl:hasValue>Surface</owl:hasValue>
                    </owl:Restriction>
                </owl:unionOf>
            </owl:Class>
        </rdfs:domain>
        <rdfs:range rdf:resource="http://www.w3.org/2001/XMLSchema#string"/>
        <rdfs:comment xml:lang="en">Represents the method used to distribute water within the irrigation system, with possible values such as &quot;Drip&quot;, &quot;Sprinkler&quot;, Surface or &quot;Subsurface&quot;.</rdfs:comment>
        <rdfs:label xml:lang="en">hasWaterDistributionMethod</rdfs:label>
    </owl:DatatypeProperty>
    


    <!-- http://www.semanticweb.org/cra/ontologies/AgriWaterMgmt#hasWaterDistributionMethodSprinkler -->

    <owl:DatatypeProperty rdf:about="http://www.semanticweb.org/cra/ontologies/AgriWaterMgmt#hasWaterDistributionMethodSprinkler">
        <rdfs:domain rdf:resource="http://www.semanticweb.org/cra/ontologies/AgriWaterMgmt#SprinklerIrrigation"/>
        <rdfs:domain>
            <owl:Class>
                <owl:unionOf rdf:parseType="Collection">
                    <owl:Restriction>
                        <owl:onProperty rdf:resource="http://www.semanticweb.org/cra/ontologies/AgriWaterMgmt#hasWaterDistributionMethodSprinkler"/>
                        <owl:hasValue>Targeted Distribution</owl:hasValue>
                    </owl:Restriction>
                    <owl:Restriction>
                        <owl:onProperty rdf:resource="http://www.semanticweb.org/cra/ontologies/AgriWaterMgmt#hasWaterDistributionMethodSprinkler"/>
                        <owl:hasValue>Uniform Distribution</owl:hasValue>
                    </owl:Restriction>
                    <owl:Restriction>
                        <owl:onProperty rdf:resource="http://www.semanticweb.org/cra/ontologies/AgriWaterMgmt#hasWaterDistributionMethodSprinkler"/>
                        <owl:hasValue>Variable Distribution</owl:hasValue>
                    </owl:Restriction>
                </owl:unionOf>
            </owl:Class>
        </rdfs:domain>
        <rdfs:range rdf:resource="http://www.w3.org/2001/XMLSchema#string"/>
        <rdfs:comment xml:lang="en">Describes how water is distributed by the sprinkler system, either uniformly or variably across the field. Possible values include &quot;Uniform Distribution&quot;, &quot;Variable Distribution&quot;, and &quot;Targeted Distribution&quot;.</rdfs:comment>
        <rdfs:label xml:lang="en">hasWaterDistributionMethodSprinkler</rdfs:label>
    </owl:DatatypeProperty>
    


    <!-- http://www.semanticweb.org/cra/ontologies/AgriWaterMgmt#hasWaterDistributionMethodSurface -->

    <owl:DatatypeProperty rdf:about="http://www.semanticweb.org/cra/ontologies/AgriWaterMgmt#hasWaterDistributionMethodSurface">
        <rdfs:domain rdf:resource="http://www.semanticweb.org/cra/ontologies/AgriWaterMgmt#SurfaceIrrigation"/>
        <rdfs:domain>
            <owl:Class>
                <owl:unionOf rdf:parseType="Collection">
                    <owl:Restriction>
                        <owl:onProperty rdf:resource="http://www.semanticweb.org/cra/ontologies/AgriWaterMgmt#hasWaterDistributionMethodSurface"/>
                        <owl:hasValue>Basin</owl:hasValue>
                    </owl:Restriction>
                    <owl:Restriction>
                        <owl:onProperty rdf:resource="http://www.semanticweb.org/cra/ontologies/AgriWaterMgmt#hasWaterDistributionMethodSurface"/>
                        <owl:hasValue>Border</owl:hasValue>
                    </owl:Restriction>
                    <owl:Restriction>
                        <owl:onProperty rdf:resource="http://www.semanticweb.org/cra/ontologies/AgriWaterMgmt#hasWaterDistributionMethodSurface"/>
                        <owl:hasValue>Flood</owl:hasValue>
                    </owl:Restriction>
                    <owl:Restriction>
                        <owl:onProperty rdf:resource="http://www.semanticweb.org/cra/ontologies/AgriWaterMgmt#hasWaterDistributionMethodSurface"/>
                        <owl:hasValue>Furrow</owl:hasValue>
                    </owl:Restriction>
                </owl:unionOf>
            </owl:Class>
        </rdfs:domain>
        <rdfs:range rdf:resource="http://www.w3.org/2001/XMLSchema#string"/>
        <rdfs:comment xml:lang="en">Describes the method by which water is distributed across the surface of the field. Possible values include &quot;Furrow&quot;, &quot;Basin&quot;, &quot;Border&quot;, and &quot;Flood&quot;.</rdfs:comment>
        <rdfs:label xml:lang="en">hasWaterDistributionMethodSurface</rdfs:label>
    </owl:DatatypeProperty>
    


    <!-- http://www.semanticweb.org/cra/ontologies/AgriWaterMgmt#hasWaterPressureLevel -->

    <owl:DatatypeProperty rdf:about="http://www.semanticweb.org/cra/ontologies/AgriWaterMgmt#hasWaterPressureLevel">
        <rdfs:domain rdf:resource="http://www.semanticweb.org/cra/ontologies/AgriWaterMgmt#SprinklerIrrigation"/>
        <rdfs:domain>
            <owl:Class>
                <owl:unionOf rdf:parseType="Collection">
                    <owl:Restriction>
                        <owl:onProperty rdf:resource="http://www.semanticweb.org/cra/ontologies/AgriWaterMgmt#hasWaterPressureLevel"/>
                        <owl:hasValue>High Pressure</owl:hasValue>
                    </owl:Restriction>
                    <owl:Restriction>
                        <owl:onProperty rdf:resource="http://www.semanticweb.org/cra/ontologies/AgriWaterMgmt#hasWaterPressureLevel"/>
                        <owl:hasValue>Low Pressure</owl:hasValue>
                    </owl:Restriction>
                    <owl:Restriction>
                        <owl:onProperty rdf:resource="http://www.semanticweb.org/cra/ontologies/AgriWaterMgmt#hasWaterPressureLevel"/>
                        <owl:hasValue>Medium Pressure</owl:hasValue>
                    </owl:Restriction>
                </owl:unionOf>
            </owl:Class>
        </rdfs:domain>
        <rdfs:range rdf:resource="http://www.w3.org/2001/XMLSchema#string"/>
        <rdfs:comment xml:lang="en">Measures the level of water pressure required for the sprinkler system. Possible values are &quot;Low Pressure&quot;, &quot;Medium Pressure&quot;, and &quot;High Pressure&quot;.</rdfs:comment>
        <rdfs:label xml:lang="en">hasWaterPressureLevel</rdfs:label>
    </owl:DatatypeProperty>
    


    <!-- http://www.semanticweb.org/cra/ontologies/AgriWaterMgmt#hasWaterReductionPercentage -->

    <owl:DatatypeProperty rdf:about="http://www.semanticweb.org/cra/ontologies/AgriWaterMgmt#hasWaterReductionPercentage">
        <rdfs:domain rdf:resource="http://www.semanticweb.org/cra/ontologies/AgriWaterMgmt#RegulatedDeficitIrrigation"/>
        <rdfs:domain>
            <owl:Class>
                <owl:unionOf rdf:parseType="Collection">
                    <owl:Restriction>
                        <owl:onProperty rdf:resource="http://www.semanticweb.org/cra/ontologies/AgriWaterMgmt#hasWaterReductionPercentage"/>
                        <owl:hasValue>High Reduction</owl:hasValue>
                    </owl:Restriction>
                    <owl:Restriction>
                        <owl:onProperty rdf:resource="http://www.semanticweb.org/cra/ontologies/AgriWaterMgmt#hasWaterReductionPercentage"/>
                        <owl:hasValue>Low Reduction</owl:hasValue>
                    </owl:Restriction>
                    <owl:Restriction>
                        <owl:onProperty rdf:resource="http://www.semanticweb.org/cra/ontologies/AgriWaterMgmt#hasWaterReductionPercentage"/>
                        <owl:hasValue>Medium Reduction</owl:hasValue>
                    </owl:Restriction>
                </owl:unionOf>
            </owl:Class>
        </rdfs:domain>
        <rdfs:range rdf:resource="http://www.w3.org/2001/XMLSchema#string"/>
        <rdfs:comment xml:lang="en">Represents the percentage of water reduction applied compared to the full irrigation requirement. This attribute captures the degree of deficit applied, with possible values such as &quot;Low Reduction&quot;, &quot;Medium Reduction&quot;, and &quot;High Reduction&quot;.</rdfs:comment>
        <rdfs:label xml:lang="en">hasWaterReductionPercentage</rdfs:label>
    </owl:DatatypeProperty>
    


    <!-- http://www.semanticweb.org/cra/ontologies/AgriWaterMgmt#hasWaterRequirementPerStage -->

    <owl:DatatypeProperty rdf:about="http://www.semanticweb.org/cra/ontologies/AgriWaterMgmt#hasWaterRequirementPerStage">
        <rdfs:domain rdf:resource="http://www.semanticweb.org/cra/ontologies/AgriWaterMgmt#CropGrowthStages"/>
        <rdfs:domain>
            <owl:Class>
                <owl:unionOf rdf:parseType="Collection">
                    <owl:Restriction>
                        <owl:onProperty rdf:resource="http://www.semanticweb.org/cra/ontologies/AgriWaterMgmt#hasWaterRequirementPerStage"/>
                        <owl:hasValue>High Requirement</owl:hasValue>
                    </owl:Restriction>
                    <owl:Restriction>
                        <owl:onProperty rdf:resource="http://www.semanticweb.org/cra/ontologies/AgriWaterMgmt#hasWaterRequirementPerStage"/>
                        <owl:hasValue>Low Requirement</owl:hasValue>
                    </owl:Restriction>
                    <owl:Restriction>
                        <owl:onProperty rdf:resource="http://www.semanticweb.org/cra/ontologies/AgriWaterMgmt#hasWaterRequirementPerStage"/>
                        <owl:hasValue>Moderate Requirement</owl:hasValue>
                    </owl:Restriction>
                </owl:unionOf>
            </owl:Class>
        </rdfs:domain>
        <rdfs:range rdf:resource="http://www.w3.org/2001/XMLSchema#string"/>
        <rdfs:comment xml:lang="en">Indicates the amount of water needed at each growth stage. Its values include &quot;Low Requirement&quot;, &quot;Moderate Requirement &quot; and &quot;High Requirement &quot;.</rdfs:comment>
        <rdfs:label xml:lang="en">hasWaterRequirementPerStage</rdfs:label>
    </owl:DatatypeProperty>
    


    <!-- http://www.semanticweb.org/cra/ontologies/AgriWaterMgmt#hasWaterRetentionCapacity -->

    <owl:DatatypeProperty rdf:about="http://www.semanticweb.org/cra/ontologies/AgriWaterMgmt#hasWaterRetentionCapacity">
        <rdfs:domain rdf:resource="http://www.semanticweb.org/cra/ontologies/AgriWaterMgmt#Soil_Water"/>
        <rdfs:domain>
            <owl:Class>
                <owl:unionOf rdf:parseType="Collection">
                    <owl:Restriction>
                        <owl:onProperty rdf:resource="http://www.semanticweb.org/cra/ontologies/AgriWaterMgmt#hasWaterRetentionCapacity"/>
                        <owl:hasValue>High Capacity</owl:hasValue>
                    </owl:Restriction>
                    <owl:Restriction>
                        <owl:onProperty rdf:resource="http://www.semanticweb.org/cra/ontologies/AgriWaterMgmt#hasWaterRetentionCapacity"/>
                        <owl:hasValue>Low Capacity</owl:hasValue>
                    </owl:Restriction>
                    <owl:Restriction>
                        <owl:onProperty rdf:resource="http://www.semanticweb.org/cra/ontologies/AgriWaterMgmt#hasWaterRetentionCapacity"/>
                        <owl:hasValue>Medium Capacity</owl:hasValue>
                    </owl:Restriction>
                </owl:unionOf>
            </owl:Class>
        </rdfs:domain>
        <rdfs:range rdf:resource="http://www.w3.org/2001/XMLSchema#string"/>
        <rdfs:comment xml:lang="en">Refers to the ability of the soil to hold water for plant use. It indicates how much water the soil can retain after irrigation or rainfall. Possible values can include &quot;Low Capacity&quot;, &quot;Medium Capacity&quot;, and &quot;High Capacity&quot;.</rdfs:comment>
        <rdfs:label xml:lang="en">hasWaterRetentionCapacity</rdfs:label>
    </owl:DatatypeProperty>
    


    <!-- http://www.semanticweb.org/cra/ontologies/AgriWaterMgmt#hasWaterScarcityLevel -->

    <owl:DatatypeProperty rdf:about="http://www.semanticweb.org/cra/ontologies/AgriWaterMgmt#hasWaterScarcityLevel">
        <rdfs:domain rdf:resource="http://www.semanticweb.org/cra/ontologies/AgriWaterMgmt#AridRegions"/>
        <rdfs:domain>
            <owl:Class>
                <owl:unionOf rdf:parseType="Collection">
                    <owl:Restriction>
                        <owl:onProperty rdf:resource="http://www.semanticweb.org/cra/ontologies/AgriWaterMgmt#hasWaterScarcityLevel"/>
                        <owl:hasValue>Low Scarcity</owl:hasValue>
                    </owl:Restriction>
                    <owl:Restriction>
                        <owl:onProperty rdf:resource="http://www.semanticweb.org/cra/ontologies/AgriWaterMgmt#hasWaterScarcityLevel"/>
                        <owl:hasValue>Moderate Scarcity</owl:hasValue>
                    </owl:Restriction>
                    <owl:Restriction>
                        <owl:onProperty rdf:resource="http://www.semanticweb.org/cra/ontologies/AgriWaterMgmt#hasWaterScarcityLevel"/>
                        <owl:hasValue>Severe Scarcity</owl:hasValue>
                    </owl:Restriction>
                </owl:unionOf>
            </owl:Class>
        </rdfs:domain>
        <rdfs:range rdf:resource="http://www.w3.org/2001/XMLSchema#string"/>
        <rdfs:comment xml:lang="en">Describes the level of water scarcity typical of arid regions. Its values include &quot;Severe Scarcity&quot;, &quot;Moderate Scarcity&quot;, and &quot;Low Scarcity&quot;.</rdfs:comment>
        <rdfs:label xml:lang="en">hasWaterScarcityLevel</rdfs:label>
    </owl:DatatypeProperty>
    


    <!-- http://www.semanticweb.org/cra/ontologies/AgriWaterMgmt#hasWaterSource -->

    <owl:DatatypeProperty rdf:about="http://www.semanticweb.org/cra/ontologies/AgriWaterMgmt#hasWaterSource">
        <rdfs:domain>
            <owl:Class>
                <owl:unionOf rdf:parseType="Collection">
                    <owl:Restriction>
                        <owl:onProperty rdf:resource="http://www.semanticweb.org/cra/ontologies/AgriWaterMgmt#hasWaterSource"/>
                        <owl:hasValue>Desaliated Water</owl:hasValue>
                    </owl:Restriction>
                    <owl:Restriction>
                        <owl:onProperty rdf:resource="http://www.semanticweb.org/cra/ontologies/AgriWaterMgmt#hasWaterSource"/>
                        <owl:hasValue>Ground Water</owl:hasValue>
                    </owl:Restriction>
                    <owl:Restriction>
                        <owl:onProperty rdf:resource="http://www.semanticweb.org/cra/ontologies/AgriWaterMgmt#hasWaterSource"/>
                        <owl:hasValue>Recycled Water</owl:hasValue>
                    </owl:Restriction>
                    <owl:Restriction>
                        <owl:onProperty rdf:resource="http://www.semanticweb.org/cra/ontologies/AgriWaterMgmt#hasWaterSource"/>
                        <owl:hasValue>Surface Water</owl:hasValue>
                    </owl:Restriction>
                </owl:unionOf>
            </owl:Class>
        </rdfs:domain>
        <rdfs:range rdf:resource="http://www.w3.org/2001/XMLSchema#string"/>
        <rdfs:label xml:lang="en">It identifies different sources of water utilized in agricultural practices, such as &quot;Desalinated Water&quot;, &quot;Surface Water&quot;, &quot;Ground Water&quot; and &quot;Recycled Water&quot;.</rdfs:label>
        <rdfs:label xml:lang="en">hasWaterSource</rdfs:label>
    </owl:DatatypeProperty>
    


    <!-- http://www.semanticweb.org/cra/ontologies/AgriWaterMgmt#hasWaterStressLevel -->

    <owl:DatatypeProperty rdf:about="http://www.semanticweb.org/cra/ontologies/AgriWaterMgmt#hasWaterStressLevel">
        <rdfs:domain rdf:resource="http://www.semanticweb.org/cra/ontologies/AgriWaterMgmt#CropWaterStress"/>
        <rdfs:domain>
            <owl:Class>
                <owl:unionOf rdf:parseType="Collection">
                    <owl:Restriction>
                        <owl:onProperty rdf:resource="http://www.semanticweb.org/cra/ontologies/AgriWaterMgmt#hasWaterStressLevel"/>
                        <owl:hasValue>High Stress</owl:hasValue>
                    </owl:Restriction>
                    <owl:Restriction>
                        <owl:onProperty rdf:resource="http://www.semanticweb.org/cra/ontologies/AgriWaterMgmt#hasWaterStressLevel"/>
                        <owl:hasValue>Low Stress</owl:hasValue>
                    </owl:Restriction>
                    <owl:Restriction>
                        <owl:onProperty rdf:resource="http://www.semanticweb.org/cra/ontologies/AgriWaterMgmt#hasWaterStressLevel"/>
                        <owl:hasValue>Medium Stress</owl:hasValue>
                    </owl:Restriction>
                </owl:unionOf>
            </owl:Class>
        </rdfs:domain>
        <rdfs:range rdf:resource="http://www.w3.org/2001/XMLSchema#string"/>
        <rdfs:comment xml:lang="en">Level of water stress experienced by a crop due to insufficient or excessive water. Possible values include &quot;Low Stress&quot;, &quot;Medium Stress&quot;, and &quot;High Stress&quot;.</rdfs:comment>
        <rdfs:label xml:lang="en">hasWaterStressLevel</rdfs:label>
    </owl:DatatypeProperty>
    


    <!-- http://www.semanticweb.org/cra/ontologies/AgriWaterMgmt#hasWaterWasteReductionLevel -->

    <owl:DatatypeProperty rdf:about="http://www.semanticweb.org/cra/ontologies/AgriWaterMgmt#hasWaterWasteReductionLevel">
        <rdfs:domain rdf:resource="http://www.semanticweb.org/cra/ontologies/AgriWaterMgmt#WaterEfficiency"/>
        <rdfs:domain>
            <owl:Class>
                <owl:unionOf rdf:parseType="Collection">
                    <owl:Restriction>
                        <owl:onProperty rdf:resource="http://www.semanticweb.org/cra/ontologies/AgriWaterMgmt#hasWaterWasteReductionLevel"/>
                        <owl:hasValue>High Reduction</owl:hasValue>
                    </owl:Restriction>
                    <owl:Restriction>
                        <owl:onProperty rdf:resource="http://www.semanticweb.org/cra/ontologies/AgriWaterMgmt#hasWaterWasteReductionLevel"/>
                        <owl:hasValue>Minimal Reduction</owl:hasValue>
                    </owl:Restriction>
                    <owl:Restriction>
                        <owl:onProperty rdf:resource="http://www.semanticweb.org/cra/ontologies/AgriWaterMgmt#hasWaterWasteReductionLevel"/>
                        <owl:hasValue>Moderate Reduction</owl:hasValue>
                    </owl:Restriction>
                </owl:unionOf>
            </owl:Class>
        </rdfs:domain>
        <rdfs:range rdf:resource="http://www.w3.org/2001/XMLSchema#string"/>
        <rdfs:comment xml:lang="en">Shows how effectively the water efficiency measures reduce water waste. Its values include &quot;Minimal Reduction&quot;, &quot;Moderate Reduction&quot;, and &quot;High Reduction&quot;.</rdfs:comment>
        <rdfs:label xml:lang="en">hasWaterWasteReductionLevel</rdfs:label>
    </owl:DatatypeProperty>
    


    <!-- http://www.semanticweb.org/cra/ontologies/AgriWaterMgmt#haspHLevel -->

    <owl:DatatypeProperty rdf:about="http://www.semanticweb.org/cra/ontologies/AgriWaterMgmt#haspHLevel">
        <rdfs:domain rdf:resource="http://www.semanticweb.org/cra/ontologies/AgriWaterMgmt#SoilAnalysis"/>
        <rdfs:domain rdf:resource="http://www.semanticweb.org/cra/ontologies/AgriWaterMgmt#SoilHealth"/>
        <rdfs:range>
            <rdfs:Datatype>
                <owl:onDatatype rdf:resource="http://www.w3.org/2001/XMLSchema#decimal"/>
                <owl:withRestrictions rdf:parseType="Collection">
                    <rdf:Description>
                        <xsd:minInclusive rdf:datatype="http://www.w3.org/2001/XMLSchema#decimal">0</xsd:minInclusive>
                    </rdf:Description>
                    <rdf:Description>
                        <xsd:maxInclusive rdf:datatype="http://www.w3.org/2001/XMLSchema#decimal">14</xsd:maxInclusive>
                    </rdf:Description>
                </owl:withRestrictions>
            </rdfs:Datatype>
        </rdfs:range>
        <rdfs:comment xml:lang="en">Represents the pH level of the soil, which affects nutrient availability and soil health. Possible values include numerical ranges, indicating acidic to alkaline conditions.</rdfs:comment>
        <rdfs:label xml:lang="en">haspHLevel</rdfs:label>
    </owl:DatatypeProperty>
    


    <!-- 
    ///////////////////////////////////////////////////////////////////////////////////////
    //
    // Classes
    //
    ///////////////////////////////////////////////////////////////////////////////////////
     -->

    


    <!-- http://www.semanticweb.org/cra/ontologies/AgriWaterMgmt#Accessories -->

    <owl:Class rdf:about="http://www.semanticweb.org/cra/ontologies/AgriWaterMgmt#Accessories">
        <rdfs:subClassOf rdf:resource="http://www.semanticweb.org/cra/ontologies/AgriWaterMgmt#AgriculturalEngineering"/>
        <rdfs:comment xml:lang="en">These include valves, bends, plugs, risers, and other small components that contribute to the system&apos;s efficiency but are not listed individually to keep the ontology concise.</rdfs:comment>
        <rdfs:label xml:lang="en">Accessories</rdfs:label>
    </owl:Class>
    


    <!-- http://www.semanticweb.org/cra/ontologies/AgriWaterMgmt#AgriculturalEngineering -->

    <owl:Class rdf:about="http://www.semanticweb.org/cra/ontologies/AgriWaterMgmt#AgriculturalEngineering">
        <rdfs:subClassOf rdf:resource="http://www.semanticweb.org/cra/ontologies/AgriWaterMgmt#Water"/>
        <rdfs:comment xml:lang="en">Agricultural engineering, also known as agricultural and biosystems engineering, is the field of study and application of engineering science and designs principles for agriculture purposes, combining the various disciplines of mechanical, civil, electrical, food science, environmental, software, and chemical engineering to improve the efficiency of farms and agribusiness enterprises as well as to ensure sustainability of natural and renewable resources.</rdfs:comment>
        <rdfs:label xml:lang="en">Agricultural Engineering</rdfs:label>
    </owl:Class>
    


    <!-- http://www.semanticweb.org/cra/ontologies/AgriWaterMgmt#AridRegions -->

    <owl:Class rdf:about="http://www.semanticweb.org/cra/ontologies/AgriWaterMgmt#AridRegions">
        <rdfs:subClassOf rdf:resource="http://www.semanticweb.org/cra/ontologies/AgriWaterMgmt#Regions"/>
        <rdfs:comment xml:lang="en">Arid regions are characterized by low rainfall, typically less than 250 mm per year, resulting in a scarcity of water resources and posing significant challenges for agriculture and habitation.</rdfs:comment>
        <rdfs:label xml:lang="en">Arid Regions</rdfs:label>
    </owl:Class>
    


    <!-- http://www.semanticweb.org/cra/ontologies/AgriWaterMgmt#ClimateChange -->

    <owl:Class rdf:about="http://www.semanticweb.org/cra/ontologies/AgriWaterMgmt#ClimateChange">
        <owl:equivalentClass>
            <owl:Class>
                <owl:intersectionOf rdf:parseType="Collection">
                    <rdf:Description rdf:about="http://www.semanticweb.org/cra/ontologies/AgriWaterMgmt#WeatherCondition"/>
                    <owl:Restriction>
                        <owl:onProperty rdf:resource="http://www.semanticweb.org/cra/ontologies/AgriWaterMgmt#causes"/>
                        <owl:someValuesFrom rdf:resource="http://www.semanticweb.org/cra/ontologies/AgriWaterMgmt#Drought"/>
                    </owl:Restriction>
                </owl:intersectionOf>
            </owl:Class>
        </owl:equivalentClass>
        <rdfs:subClassOf rdf:resource="http://www.semanticweb.org/cra/ontologies/AgriWaterMgmt#WeatherCondition"/>
        <rdfs:comment xml:lang="en">The long-term alteration of temperature and typical weather patterns in a place, often influenced by human activity. Climate change has profound impacts on water availability, agricultural practices, and ecosystem sustainability.</rdfs:comment>
        <rdfs:label xml:lang="en">Climate Change</rdfs:label>
    </owl:Class>
    


    <!-- http://www.semanticweb.org/cra/ontologies/AgriWaterMgmt#Couplers -->

    <owl:Class rdf:about="http://www.semanticweb.org/cra/ontologies/AgriWaterMgmt#Couplers">
        <rdfs:subClassOf rdf:resource="http://www.semanticweb.org/cra/ontologies/AgriWaterMgmt#AgriculturalEngineering"/>
        <rdfs:comment xml:lang="en">Used in Sprinkler Irrigation systems for connecting two pipes and uncoupling quickly and easily, ensuring that water flows smoothly throughout the system.</rdfs:comment>
        <rdfs:label xml:lang="en">Couplers</rdfs:label>
    </owl:Class>
    


    <!-- http://www.semanticweb.org/cra/ontologies/AgriWaterMgmt#CropEvapotranspiration -->

    <owl:Class rdf:about="http://www.semanticweb.org/cra/ontologies/AgriWaterMgmt#CropEvapotranspiration">
        <rdfs:subClassOf rdf:resource="http://www.semanticweb.org/cra/ontologies/AgriWaterMgmt#Crops"/>
        <rdfs:comment xml:lang="en">The combined process of evaporation from the soil and transpiration from plants, which determines the water loss from a crop system. It is a critical factor in water management and irrigation planning.</rdfs:comment>
        <rdfs:label xml:lang="en">Crop Evapotranspiration</rdfs:label>
    </owl:Class>
    


    <!-- http://www.semanticweb.org/cra/ontologies/AgriWaterMgmt#CropGrowthStages -->

    <owl:Class rdf:about="http://www.semanticweb.org/cra/ontologies/AgriWaterMgmt#CropGrowthStages">
        <rdfs:subClassOf rdf:resource="http://www.semanticweb.org/cra/ontologies/AgriWaterMgmt#Crops"/>
        <rdfs:comment xml:lang="en">The various phases of development that crops undergo from germination to maturity. Each stage has specific water and nutrient requirements, which are crucial for effective management.</rdfs:comment>
        <rdfs:label xml:lang="en">Crop Growth Stages</rdfs:label>
    </owl:Class>
    


    <!-- http://www.semanticweb.org/cra/ontologies/AgriWaterMgmt#CropIrrigationRequirements -->

    <owl:Class rdf:about="http://www.semanticweb.org/cra/ontologies/AgriWaterMgmt#CropIrrigationRequirements">
        <owl:equivalentClass>
            <owl:Restriction>
                <owl:onProperty rdf:resource="http://www.semanticweb.org/cra/ontologies/AgriWaterMgmt#isMetBy"/>
                <owl:someValuesFrom rdf:resource="http://www.semanticweb.org/cra/ontologies/AgriWaterMgmt#IrrigationSystems"/>
            </owl:Restriction>
        </owl:equivalentClass>
        <rdfs:subClassOf rdf:resource="http://www.semanticweb.org/cra/ontologies/AgriWaterMgmt#Crops"/>
        <rdfs:comment xml:lang="en">The specific water needs of a crop during its growth stages, including the frequency and amount of irrigation required to maintain optimal soil moisture levels for healthy growth.</rdfs:comment>
        <rdfs:label xml:lang="en">Crop Irrigation Requirements</rdfs:label>
    </owl:Class>
    


    <!-- http://www.semanticweb.org/cra/ontologies/AgriWaterMgmt#CropWaterStress -->

    <owl:Class rdf:about="http://www.semanticweb.org/cra/ontologies/AgriWaterMgmt#CropWaterStress">
        <owl:equivalentClass>
            <owl:Restriction>
                <owl:onProperty rdf:resource="http://www.semanticweb.org/cra/ontologies/AgriWaterMgmt#isMitigatedBy"/>
                <owl:someValuesFrom rdf:resource="http://www.semanticweb.org/cra/ontologies/AgriWaterMgmt#WaterEfficiency"/>
            </owl:Restriction>
        </owl:equivalentClass>
        <rdfs:subClassOf rdf:resource="http://www.semanticweb.org/cra/ontologies/AgriWaterMgmt#Crops"/>
        <rdfs:comment xml:lang="en">The physiological condition experienced by crops when water availability is insufficient or excessive for optimal growth. Water stress can affect crop yield, quality, and overall health, leading to reduced productivity.</rdfs:comment>
        <rdfs:label xml:lang="en">Crop Water Stress</rdfs:label>
    </owl:Class>
    


    <!-- http://www.semanticweb.org/cra/ontologies/AgriWaterMgmt#Crops -->

    <owl:Class rdf:about="http://www.semanticweb.org/cra/ontologies/AgriWaterMgmt#Crops">
        <rdfs:subClassOf rdf:resource="http://www.semanticweb.org/cra/ontologies/AgriWaterMgmt#Water"/>
        <rdfs:comment xml:lang="en">A cultivated plant that is grown commercially on a large scale.</rdfs:comment>
        <rdfs:label xml:lang="en">Crops</rdfs:label>
    </owl:Class>
    


    <!-- http://www.semanticweb.org/cra/ontologies/AgriWaterMgmt#DesalinatedWater -->

    <owl:Class rdf:about="http://www.semanticweb.org/cra/ontologies/AgriWaterMgmt#DesalinatedWater">
        <owl:equivalentClass>
            <owl:Restriction>
                <owl:onProperty rdf:resource="http://www.semanticweb.org/cra/ontologies/AgriWaterMgmt#supplements"/>
                <owl:someValuesFrom rdf:resource="http://www.semanticweb.org/cra/ontologies/AgriWaterMgmt#WaterResources"/>
            </owl:Restriction>
        </owl:equivalentClass>
        <rdfs:subClassOf rdf:resource="http://www.semanticweb.org/cra/ontologies/AgriWaterMgmt#WaterResources"/>
        <rdfs:comment xml:lang="en">Refers to water that has been purified by removing salt and other minerals, typically from seawater or brackish water, using technologies such as reverse osmosis. Desalinated water is an important source in areas facing freshwater scarcity.</rdfs:comment>
        <rdfs:label xml:lang="en">Desalinated Water</rdfs:label>
    </owl:Class>
    


    <!-- http://www.semanticweb.org/cra/ontologies/AgriWaterMgmt#DripIrrigation -->

    <owl:Class rdf:about="http://www.semanticweb.org/cra/ontologies/AgriWaterMgmt#DripIrrigation">
        <rdfs:subClassOf rdf:resource="http://www.semanticweb.org/cra/ontologies/AgriWaterMgmt#IrrigationSystems"/>
        <rdfs:comment xml:lang="en">Also called localized irrigation, is a highly efficient irrigation method that delivers water directly to the roots of plants through a network of tubing and emitters. This system minimizes evaporation and runoff, making it ideal for water conservation.</rdfs:comment>
        <rdfs:label xml:lang="en">Drip Irrigation</rdfs:label>
    </owl:Class>
    


    <!-- http://www.semanticweb.org/cra/ontologies/AgriWaterMgmt#Drought -->

    <owl:Class rdf:about="http://www.semanticweb.org/cra/ontologies/AgriWaterMgmt#Drought">
        <owl:equivalentClass>
            <owl:Restriction>
                <owl:onProperty rdf:resource="http://www.semanticweb.org/cra/ontologies/AgriWaterMgmt#increasesNeedFor"/>
                <owl:someValuesFrom rdf:resource="http://www.semanticweb.org/cra/ontologies/AgriWaterMgmt#WaterConservation"/>
            </owl:Restriction>
        </owl:equivalentClass>
        <rdfs:subClassOf rdf:resource="http://www.semanticweb.org/cra/ontologies/AgriWaterMgmt#WeatherCondition"/>
        <rdfs:comment xml:lang="en">A prolonged period of abnormally low rainfall, leading to a shortage of water. Drought can significantly impact agriculture, water resources, and sustainability efforts.</rdfs:comment>
        <rdfs:label xml:lang="en">Drought</rdfs:label>
    </owl:Class>
    


    <!-- http://www.semanticweb.org/cra/ontologies/AgriWaterMgmt#Environmental_Impact -->

    <owl:Class rdf:about="http://www.semanticweb.org/cra/ontologies/AgriWaterMgmt#Environmental_Impact">
        <rdfs:subClassOf rdf:resource="http://www.semanticweb.org/cra/ontologies/AgriWaterMgmt#SustainabilityAndEnvironmentalImpact"/>
        <rdfs:comment xml:lang="en">Refers to the direct or indirect effect that an activity, project, or policy has on the environment, including land, water, air, and biodiversity.</rdfs:comment>
        <rdfs:label xml:lang="en">Environmental Impact</rdfs:label>
    </owl:Class>
    


    <!-- http://www.semanticweb.org/cra/ontologies/AgriWaterMgmt#GroundWater -->

    <owl:Class rdf:about="http://www.semanticweb.org/cra/ontologies/AgriWaterMgmt#GroundWater">
        <owl:equivalentClass>
            <owl:Restriction>
                <owl:onProperty rdf:resource="http://www.semanticweb.org/cra/ontologies/AgriWaterMgmt#supports"/>
                <owl:someValuesFrom rdf:resource="http://www.semanticweb.org/cra/ontologies/AgriWaterMgmt#IrrigatedAreas"/>
            </owl:Restriction>
        </owl:equivalentClass>
        <rdfs:subClassOf rdf:resource="http://www.semanticweb.org/cra/ontologies/AgriWaterMgmt#WaterResources"/>
        <rdfs:comment xml:lang="en">Refers to water located beneath the Earth&apos;s surface in soil pore spaces and in the fractures of rock formations. Groundwater is a critical water resource for agriculture, drinking water, and industrial processes, especially in arid regions.</rdfs:comment>
        <rdfs:label xml:lang="en">Groundwater</rdfs:label>
    </owl:Class>
    


    <!-- http://www.semanticweb.org/cra/ontologies/AgriWaterMgmt#IrrigatedAreas -->

    <owl:Class rdf:about="http://www.semanticweb.org/cra/ontologies/AgriWaterMgmt#IrrigatedAreas">
        <rdfs:subClassOf rdf:resource="http://www.semanticweb.org/cra/ontologies/AgriWaterMgmt#Regions"/>
        <rdfs:comment xml:lang="en">Irrigated areas refer to regions of land where water is supplied to crops through various irrigation methods, enhancing agricultural productivity and enabling cultivation in otherwise arid environments.</rdfs:comment>
        <rdfs:label xml:lang="en">Irrigated Areas</rdfs:label>
    </owl:Class>
    


    <!-- http://www.semanticweb.org/cra/ontologies/AgriWaterMgmt#IrrigationScheduling -->

    <owl:Class rdf:about="http://www.semanticweb.org/cra/ontologies/AgriWaterMgmt#IrrigationScheduling">
        <rdfs:subClassOf rdf:resource="http://www.semanticweb.org/cra/ontologies/AgriWaterMgmt#AgriculturalEngineering"/>
        <rdfs:comment xml:lang="en">The planning and timing of irrigation to meet the water requirements of crops while minimizing water wastage and ensuring efficient water use.</rdfs:comment>
        <rdfs:label xml:lang="en">Irrigation Scheduling</rdfs:label>
    </owl:Class>
    


    <!-- http://www.semanticweb.org/cra/ontologies/AgriWaterMgmt#IrrigationSystems -->

    <owl:Class rdf:about="http://www.semanticweb.org/cra/ontologies/AgriWaterMgmt#IrrigationSystems">
        <owl:equivalentClass>
            <owl:Restriction>
                <owl:onProperty rdf:resource="http://www.semanticweb.org/cra/ontologies/AgriWaterMgmt#supports"/>
                <owl:someValuesFrom rdf:resource="http://www.semanticweb.org/cra/ontologies/AgriWaterMgmt#WaterConservation"/>
            </owl:Restriction>
        </owl:equivalentClass>
        <rdfs:subClassOf rdf:resource="http://www.semanticweb.org/cra/ontologies/AgriWaterMgmt#Water"/>
        <rdfs:comment xml:lang="en">Supplying dry land with water by means of ditches etc.</rdfs:comment>
        <rdfs:label xml:lang="en">Irrigation Systems</rdfs:label>
    </owl:Class>
    


    <!-- http://www.semanticweb.org/cra/ontologies/AgriWaterMgmt#IrrigationTechnology -->

    <owl:Class rdf:about="http://www.semanticweb.org/cra/ontologies/AgriWaterMgmt#IrrigationTechnology">
        <owl:equivalentClass>
            <owl:Restriction>
                <owl:onProperty rdf:resource="http://www.semanticweb.org/cra/ontologies/AgriWaterMgmt#improves"/>
                <owl:someValuesFrom rdf:resource="http://www.semanticweb.org/cra/ontologies/AgriWaterMgmt#WaterEfficiency"/>
            </owl:Restriction>
        </owl:equivalentClass>
        <rdfs:subClassOf rdf:resource="http://www.semanticweb.org/cra/ontologies/AgriWaterMgmt#AgriculturalEngineering"/>
        <rdfs:comment xml:lang="en">Technologies designed to improve the efficiency of water distribution for irrigation purposes. This includes smart irrigation systems, automated irrigation controllers, and water-saving technologies to optimize water use in agriculture.</rdfs:comment>
        <rdfs:label xml:lang="en">Irrigation Technology</rdfs:label>
    </owl:Class>
    


    <!-- http://www.semanticweb.org/cra/ontologies/AgriWaterMgmt#PrecisionAgriculture -->

    <owl:Class rdf:about="http://www.semanticweb.org/cra/ontologies/AgriWaterMgmt#PrecisionAgriculture">
        <owl:equivalentClass>
            <owl:Class>
                <owl:intersectionOf rdf:parseType="Collection">
                    <owl:Restriction>
                        <owl:onProperty rdf:resource="http://www.semanticweb.org/cra/ontologies/AgriWaterMgmt#improves"/>
                        <owl:someValuesFrom rdf:resource="http://www.semanticweb.org/cra/ontologies/AgriWaterMgmt#WaterEfficiency"/>
                    </owl:Restriction>
                    <owl:Restriction>
                        <owl:onProperty rdf:resource="http://www.semanticweb.org/cra/ontologies/AgriWaterMgmt#requires"/>
                        <owl:someValuesFrom rdf:resource="http://www.semanticweb.org/cra/ontologies/AgriWaterMgmt#WaterSensors"/>
                    </owl:Restriction>
                </owl:intersectionOf>
            </owl:Class>
        </owl:equivalentClass>
        <rdfs:subClassOf rdf:resource="http://www.semanticweb.org/cra/ontologies/AgriWaterMgmt#AgriculturalEngineering"/>
        <rdfs:comment xml:lang="en">An agricultural management system based on observing, measuring, and responding to variability in crops and fields, using advanced technologies such as sensors, satellite imagery, and GPS for optimized water use, fertilization, and pest management.</rdfs:comment>
        <rdfs:label xml:lang="en">Precision Agriculture</rdfs:label>
    </owl:Class>
    


    <!-- http://www.semanticweb.org/cra/ontologies/AgriWaterMgmt#PumpUnit -->

    <owl:Class rdf:about="http://www.semanticweb.org/cra/ontologies/AgriWaterMgmt#PumpUnit">
        <rdfs:subClassOf rdf:resource="http://www.semanticweb.org/cra/ontologies/AgriWaterMgmt#AgriculturalEngineering"/>
        <rdfs:comment xml:lang="en">Part of Sprinkler Irrigation systems, responsible for supplying the pressure needed to distribute water through the system.</rdfs:comment>
        <rdfs:label xml:lang="en">Pump Unit</rdfs:label>
    </owl:Class>
    


    <!-- http://www.semanticweb.org/cra/ontologies/AgriWaterMgmt#RainwaterHarvesting -->

    <owl:Class rdf:about="http://www.semanticweb.org/cra/ontologies/AgriWaterMgmt#RainwaterHarvesting">
        <owl:equivalentClass>
            <owl:Restriction>
                <owl:onProperty rdf:resource="http://www.semanticweb.org/cra/ontologies/AgriWaterMgmt#enhances"/>
                <owl:someValuesFrom rdf:resource="http://www.semanticweb.org/cra/ontologies/AgriWaterMgmt#WaterConservation"/>
            </owl:Restriction>
        </owl:equivalentClass>
        <rdfs:subClassOf rdf:resource="http://www.semanticweb.org/cra/ontologies/AgriWaterMgmt#WeatherCondition"/>
        <rdfs:label xml:lang="en">Rainwater Harvesting</rdfs:label>
        <rdfs:label xml:lang="en">The collection and storage of rainwater for reuse, rather than letting it run off. Rainwater harvesting is an important technique in water-scarce regions to supplement water supply.</rdfs:label>
    </owl:Class>
    


    <!-- http://www.semanticweb.org/cra/ontologies/AgriWaterMgmt#RecycledWater -->

    <owl:Class rdf:about="http://www.semanticweb.org/cra/ontologies/AgriWaterMgmt#RecycledWater">
        <owl:equivalentClass>
            <owl:Restriction>
                <owl:onProperty rdf:resource="http://www.semanticweb.org/cra/ontologies/AgriWaterMgmt#isUsedIn"/>
                <owl:someValuesFrom rdf:resource="http://www.semanticweb.org/cra/ontologies/AgriWaterMgmt#SustainableAgriculture"/>
            </owl:Restriction>
        </owl:equivalentClass>
        <rdfs:subClassOf rdf:resource="http://www.semanticweb.org/cra/ontologies/AgriWaterMgmt#WaterResources"/>
        <rdfs:comment xml:lang="en">Refers to treated wastewater that has been purified for reuse in various applications, such as irrigation, industrial processes, and groundwater replenishment. Recycling water helps to conserve freshwater resources and reduce the environmental impact of water consumption.</rdfs:comment>
        <rdfs:label xml:lang="en">Recycled Water</rdfs:label>
    </owl:Class>
    


    <!-- http://www.semanticweb.org/cra/ontologies/AgriWaterMgmt#Regions -->

    <owl:Class rdf:about="http://www.semanticweb.org/cra/ontologies/AgriWaterMgmt#Regions">
        <rdfs:subClassOf rdf:resource="http://www.semanticweb.org/cra/ontologies/AgriWaterMgmt#Water"/>
        <rdfs:comment xml:lang="en">Geographical areas that have distinct climate, soil, and water availability characteristics, impacting agricultural practices and water management strategies.</rdfs:comment>
        <rdfs:label xml:lang="en">Regions</rdfs:label>
    </owl:Class>
    


    <!-- http://www.semanticweb.org/cra/ontologies/AgriWaterMgmt#RegulatedDeficitIrrigation -->

    <owl:Class rdf:about="http://www.semanticweb.org/cra/ontologies/AgriWaterMgmt#RegulatedDeficitIrrigation">
        <rdfs:subClassOf rdf:resource="http://www.semanticweb.org/cra/ontologies/AgriWaterMgmt#IrrigationSystems"/>
        <rdfs:comment xml:lang="en">A strategic irrigation method that allows for controlled water deficits during certain growth periods to improve water efficiency and crop yield.</rdfs:comment>
        <rdfs:label xml:lang="en">Regulated Deficit Irrigation</rdfs:label>
    </owl:Class>
    


    <!-- http://www.semanticweb.org/cra/ontologies/AgriWaterMgmt#RuralAreas -->

    <owl:Class rdf:about="http://www.semanticweb.org/cra/ontologies/AgriWaterMgmt#RuralAreas">
        <rdfs:subClassOf rdf:resource="http://www.semanticweb.org/cra/ontologies/AgriWaterMgmt#Regions"/>
        <rdfs:comment xml:lang="en">Rural areas are regions located outside urban centers, often characterized by agricultural land use, lower population density, and greater dependence on natural resources, including water for irrigation and livestock.</rdfs:comment>
        <rdfs:label xml:lang="en">Rural Areas</rdfs:label>
    </owl:Class>
    


    <!-- http://www.semanticweb.org/cra/ontologies/AgriWaterMgmt#SoilAnalysis -->

    <owl:Class rdf:about="http://www.semanticweb.org/cra/ontologies/AgriWaterMgmt#SoilAnalysis">
        <rdfs:subClassOf rdf:resource="http://www.semanticweb.org/cra/ontologies/AgriWaterMgmt#SoilManagement"/>
        <rdfs:comment xml:lang="en">The process of testing soil for nutrients, pH, and other characteristics to inform agricultural practices.</rdfs:comment>
        <rdfs:label xml:lang="en">Soil Analysis</rdfs:label>
    </owl:Class>
    


    <!-- http://www.semanticweb.org/cra/ontologies/AgriWaterMgmt#SoilConservation -->

    <owl:Class rdf:about="http://www.semanticweb.org/cra/ontologies/AgriWaterMgmt#SoilConservation">
        <rdfs:subClassOf rdf:resource="http://www.semanticweb.org/cra/ontologies/AgriWaterMgmt#SoilManagement"/>
        <rdfs:comment xml:lang="en">Soil conservation encompasses a range of practices aimed at preventing soil erosion, maintaining soil fertility, and promoting sustainable land use, thereby preserving the natural resource base for future generations.</rdfs:comment>
        <rdfs:label xml:lang="en">Soil Conservation</rdfs:label>
    </owl:Class>
    


    <!-- http://www.semanticweb.org/cra/ontologies/AgriWaterMgmt#SoilHealth -->

    <owl:Class rdf:about="http://www.semanticweb.org/cra/ontologies/AgriWaterMgmt#SoilHealth">
        <rdfs:subClassOf rdf:resource="http://www.semanticweb.org/cra/ontologies/AgriWaterMgmt#SoilManagement"/>
        <rdfs:comment xml:lang="en">Refers to the ability of soil to sustain plant and animal life, maintain water quality, and support human health.</rdfs:comment>
        <rdfs:label xml:lang="en">Soil Health</rdfs:label>
    </owl:Class>
    


    <!-- http://www.semanticweb.org/cra/ontologies/AgriWaterMgmt#SoilManagement -->

    <owl:Class rdf:about="http://www.semanticweb.org/cra/ontologies/AgriWaterMgmt#SoilManagement">
        <owl:equivalentClass>
            <owl:Restriction>
                <owl:onProperty rdf:resource="http://www.semanticweb.org/cra/ontologies/AgriWaterMgmt#controls"/>
                <owl:someValuesFrom rdf:resource="http://www.semanticweb.org/cra/ontologies/AgriWaterMgmt#SoilSalinity"/>
            </owl:Restriction>
        </owl:equivalentClass>
        <rdfs:subClassOf rdf:resource="http://www.semanticweb.org/cra/ontologies/AgriWaterMgmt#Water"/>
        <rdfs:comment xml:lang="en">Soil management is the application of operations, practices, and treatments to protect soil and enhance its performance.</rdfs:comment>
        <rdfs:label xml:lang="en">Soil Management</rdfs:label>
    </owl:Class>
    


    <!-- http://www.semanticweb.org/cra/ontologies/AgriWaterMgmt#SoilMoisture -->

    <owl:Class rdf:about="http://www.semanticweb.org/cra/ontologies/AgriWaterMgmt#SoilMoisture">
        <rdfs:subClassOf rdf:resource="http://www.semanticweb.org/cra/ontologies/AgriWaterMgmt#SoilManagement"/>
        <rdfs:comment xml:lang="en">Refers to the volumetric amount of water held in the soil at a given time, expressed as a percentage of the soil&apos;s total volume. It is crucial for plant growth and agricultural productivity, influencing irrigation practices and water management strategies.</rdfs:comment>
        <rdfs:label xml:lang="en">Soil Moisture</rdfs:label>
    </owl:Class>
    


    <!-- http://www.semanticweb.org/cra/ontologies/AgriWaterMgmt#SoilQuality -->

    <owl:Class rdf:about="http://www.semanticweb.org/cra/ontologies/AgriWaterMgmt#SoilQuality">
        <rdfs:subClassOf rdf:resource="http://www.semanticweb.org/cra/ontologies/AgriWaterMgmt#SoilManagement"/>
        <rdfs:comment xml:lang="en">Represents the capacity of soil to function, to sustain plant and animal productivity, maintain environmental quality, and promote plant and human health.</rdfs:comment>
        <rdfs:label xml:lang="en">Soil Quality</rdfs:label>
    </owl:Class>
    


    <!-- http://www.semanticweb.org/cra/ontologies/AgriWaterMgmt#SoilSalinity -->

    <owl:Class rdf:about="http://www.semanticweb.org/cra/ontologies/AgriWaterMgmt#SoilSalinity">
        <rdfs:subClassOf rdf:resource="http://www.semanticweb.org/cra/ontologies/AgriWaterMgmt#SoilManagement"/>
        <rdfs:comment xml:lang="en">Soil salinity is the concentration of soluble salts in soil, which can negatively impact crop growth and soil health, often resulting from inadequate drainage and excessive irrigation practices.</rdfs:comment>
        <rdfs:label xml:lang="en">Soil Salinity</rdfs:label>
    </owl:Class>
    


    <!-- http://www.semanticweb.org/cra/ontologies/AgriWaterMgmt#Soil_Water -->

    <owl:Class rdf:about="http://www.semanticweb.org/cra/ontologies/AgriWaterMgmt#Soil_Water">
        <rdfs:subClassOf rdf:resource="http://www.semanticweb.org/cra/ontologies/AgriWaterMgmt#SoilManagement"/>
        <rdfs:comment xml:lang="en">Refers to the water that is held in the soil and is available for plants, including both readily available water and water that may be retained but less accessible.</rdfs:comment>
        <rdfs:label xml:lang="en">Soil Water</rdfs:label>
    </owl:Class>
    


    <!-- http://www.semanticweb.org/cra/ontologies/AgriWaterMgmt#SprinklerHead -->

    <owl:Class rdf:about="http://www.semanticweb.org/cra/ontologies/AgriWaterMgmt#SprinklerHead">
        <rdfs:subClassOf rdf:resource="http://www.semanticweb.org/cra/ontologies/AgriWaterMgmt#AgriculturalEngineering"/>
        <rdfs:comment xml:lang="en">A device used in Sprinkler Irrigation systems to distribute water over a specific area in the form of droplets. It helps to ensure efficient water application to crops.</rdfs:comment>
        <rdfs:label xml:lang="en">Sprinkler Head</rdfs:label>
    </owl:Class>
    


    <!-- http://www.semanticweb.org/cra/ontologies/AgriWaterMgmt#SprinklerIrrigation -->

    <owl:Class rdf:about="http://www.semanticweb.org/cra/ontologies/AgriWaterMgmt#SprinklerIrrigation">
        <owl:equivalentClass>
            <owl:Class>
                <owl:intersectionOf rdf:parseType="Collection">
                    <rdf:Description rdf:about="http://www.semanticweb.org/cra/ontologies/AgriWaterMgmt#IrrigationSystems"/>
                    <owl:Restriction>
                        <owl:onProperty rdf:resource="http://www.semanticweb.org/cra/ontologies/AgriWaterMgmt#hasPart"/>
                        <owl:someValuesFrom rdf:resource="http://www.semanticweb.org/cra/ontologies/AgriWaterMgmt#Accessories"/>
                    </owl:Restriction>
                    <owl:Restriction>
                        <owl:onProperty rdf:resource="http://www.semanticweb.org/cra/ontologies/AgriWaterMgmt#hasPart"/>
                        <owl:someValuesFrom rdf:resource="http://www.semanticweb.org/cra/ontologies/AgriWaterMgmt#Couplers"/>
                    </owl:Restriction>
                    <owl:Restriction>
                        <owl:onProperty rdf:resource="http://www.semanticweb.org/cra/ontologies/AgriWaterMgmt#hasPart"/>
                        <owl:someValuesFrom rdf:resource="http://www.semanticweb.org/cra/ontologies/AgriWaterMgmt#PumpUnit"/>
                    </owl:Restriction>
                    <owl:Restriction>
                        <owl:onProperty rdf:resource="http://www.semanticweb.org/cra/ontologies/AgriWaterMgmt#hasPart"/>
                        <owl:someValuesFrom rdf:resource="http://www.semanticweb.org/cra/ontologies/AgriWaterMgmt#SprinklerHead"/>
                    </owl:Restriction>
                    <owl:Restriction>
                        <owl:onProperty rdf:resource="http://www.semanticweb.org/cra/ontologies/AgriWaterMgmt#hasPart"/>
                        <owl:someValuesFrom rdf:resource="http://www.semanticweb.org/cra/ontologies/AgriWaterMgmt#Tubings"/>
                    </owl:Restriction>
                </owl:intersectionOf>
            </owl:Class>
        </owl:equivalentClass>
        <rdfs:subClassOf rdf:resource="http://www.semanticweb.org/cra/ontologies/AgriWaterMgmt#IrrigationSystems"/>
        <rdfs:comment xml:lang="en">A method of applying water to crops in the form of small droplets, simulating rainfall. Sprinklers can be stationary or portable, and they are suitable for a variety of crops and field sizes.</rdfs:comment>
        <rdfs:label xml:lang="en">Sprinkler Irrigation</rdfs:label>
    </owl:Class>
    


    <!-- http://www.semanticweb.org/cra/ontologies/AgriWaterMgmt#SubsurfaceIrrigation -->

    <owl:Class rdf:about="http://www.semanticweb.org/cra/ontologies/AgriWaterMgmt#SubsurfaceIrrigation">
        <rdfs:subClassOf rdf:resource="http://www.semanticweb.org/cra/ontologies/AgriWaterMgmt#IrrigationSystems"/>
        <rdfs:comment xml:lang="en">An irrigation system where water is applied below the soil surface, directly to the root zone of crops. This method can reduce evaporation and water loss while providing moisture to the plants.</rdfs:comment>
        <rdfs:label xml:lang="en">Subsurface Irrigation</rdfs:label>
    </owl:Class>
    


    <!-- http://www.semanticweb.org/cra/ontologies/AgriWaterMgmt#SurfaceIrrigation -->

    <owl:Class rdf:about="http://www.semanticweb.org/cra/ontologies/AgriWaterMgmt#SurfaceIrrigation">
        <rdfs:subClassOf rdf:resource="http://www.semanticweb.org/cra/ontologies/AgriWaterMgmt#IrrigationSystems"/>
        <rdfs:comment xml:lang="en">An irrigation method that distributes water over the soil surface by gravity. This includes furrow, flood, and basin irrigation, commonly used in various agricultural settings.</rdfs:comment>
        <rdfs:label xml:lang="en">Surface Irrigation</rdfs:label>
    </owl:Class>
    


    <!-- http://www.semanticweb.org/cra/ontologies/AgriWaterMgmt#SurfaceWater -->

    <owl:Class rdf:about="http://www.semanticweb.org/cra/ontologies/AgriWaterMgmt#SurfaceWater">
        <owl:equivalentClass>
            <owl:Restriction>
                <owl:onProperty rdf:resource="http://www.semanticweb.org/cra/ontologies/AgriWaterMgmt#isUsedIn"/>
                <owl:someValuesFrom rdf:resource="http://www.semanticweb.org/cra/ontologies/AgriWaterMgmt#IrrigationSystems"/>
            </owl:Restriction>
        </owl:equivalentClass>
        <rdfs:subClassOf rdf:resource="http://www.semanticweb.org/cra/ontologies/AgriWaterMgmt#WaterResources"/>
        <rdfs:comment xml:lang="en">Refers to water that is found on the surface of the Earth, such as in rivers, lakes, and reservoirs. Surface water is a major source of water for human consumption, agriculture, and industry, and its management is crucial for sustaining ecosystems and communities.</rdfs:comment>
        <rdfs:label xml:lang="en">Surface Water</rdfs:label>
    </owl:Class>
    


    <!-- http://www.semanticweb.org/cra/ontologies/AgriWaterMgmt#SustainabilityAndEnvironmentalImpact -->

    <owl:Class rdf:about="http://www.semanticweb.org/cra/ontologies/AgriWaterMgmt#SustainabilityAndEnvironmentalImpact">
        <rdfs:subClassOf rdf:resource="http://www.semanticweb.org/cra/ontologies/AgriWaterMgmt#Water"/>
        <rdfs:comment xml:lang="en">Refers to the practices, policies, and principles aimed at ensuring the long-term viability of resources while minimizing harm to the environment. This includes efforts to balance environmental, economic, and social goals, while managing resources responsibly to protect ecosystems and reduce pollution and waste.</rdfs:comment>
        <rdfs:label xml:lang="en">Sustainability and Environmental Impact</rdfs:label>
    </owl:Class>
    


    <!-- http://www.semanticweb.org/cra/ontologies/AgriWaterMgmt#SustainableAgriculture -->

    <owl:Class rdf:about="http://www.semanticweb.org/cra/ontologies/AgriWaterMgmt#SustainableAgriculture">
        <owl:equivalentClass>
            <owl:Class>
                <owl:intersectionOf rdf:parseType="Collection">
                    <owl:Restriction>
                        <owl:onProperty rdf:resource="http://www.semanticweb.org/cra/ontologies/AgriWaterMgmt#maintains"/>
                        <owl:someValuesFrom rdf:resource="http://www.semanticweb.org/cra/ontologies/AgriWaterMgmt#SoilHealth"/>
                    </owl:Restriction>
                    <owl:Restriction>
                        <owl:onProperty rdf:resource="http://www.semanticweb.org/cra/ontologies/AgriWaterMgmt#reduces"/>
                        <owl:someValuesFrom rdf:resource="http://www.semanticweb.org/cra/ontologies/AgriWaterMgmt#Environmental_Impact"/>
                    </owl:Restriction>
                </owl:intersectionOf>
            </owl:Class>
        </owl:equivalentClass>
        <rdfs:subClassOf rdf:resource="http://www.semanticweb.org/cra/ontologies/AgriWaterMgmt#SustainabilityAndEnvironmentalImpact"/>
        <rdfs:comment xml:lang="en">Agricultural practices that prioritize environmental health, social equity, and economic viability, ensuring that farming can continue for generations.</rdfs:comment>
        <rdfs:label xml:lang="en">Sustainable Agriculture</rdfs:label>
    </owl:Class>
    


    <!-- http://www.semanticweb.org/cra/ontologies/AgriWaterMgmt#Tubings -->

    <owl:Class rdf:about="http://www.semanticweb.org/cra/ontologies/AgriWaterMgmt#Tubings">
        <rdfs:subClassOf rdf:resource="http://www.semanticweb.org/cra/ontologies/AgriWaterMgmt#AgriculturalEngineering"/>
        <rdfs:comment xml:lang="en">These include mainline, submains and laterals, which transport water from the source to the sprinkler heads in Sprinkler Irrigation systems.</rdfs:comment>
        <rdfs:label xml:lang="en">Tubings</rdfs:label>
    </owl:Class>
    


    <!-- http://www.semanticweb.org/cra/ontologies/AgriWaterMgmt#Water -->

    <owl:Class rdf:about="http://www.semanticweb.org/cra/ontologies/AgriWaterMgmt#Water">
        <rdfs:comment xml:lang="en">The integrated management of water resources that aims to meet the water needs of agricultural production while ensuring environmental protection, promoting efficient water use, and addressing the impacts of climate change. This approach emphasizes the importance of water conservation, reuse, and sustainable practices to secure water availability for future generations.</rdfs:comment>
        <rdfs:label xml:lang="en">Sustainable Water Management</rdfs:label>
    </owl:Class>
    


    <!-- http://www.semanticweb.org/cra/ontologies/AgriWaterMgmt#WaterConservation -->

    <owl:Class rdf:about="http://www.semanticweb.org/cra/ontologies/AgriWaterMgmt#WaterConservation">
        <owl:equivalentClass>
            <owl:Restriction>
                <owl:onProperty rdf:resource="http://www.semanticweb.org/cra/ontologies/AgriWaterMgmt#optimizes"/>
                <owl:someValuesFrom rdf:resource="http://www.semanticweb.org/cra/ontologies/AgriWaterMgmt#WaterUse"/>
            </owl:Restriction>
        </owl:equivalentClass>
        <rdfs:subClassOf rdf:resource="http://www.semanticweb.org/cra/ontologies/AgriWaterMgmt#WaterManagement"/>
        <rdfs:comment xml:lang="en">Refers to the strategies and practices employed to manage and reduce water usage, ensuring that water is used efficiently and waste is minimized. This includes techniques such as reducing water loss, optimizing water use in agriculture, and recycling wastewater for reuse.</rdfs:comment>
        <rdfs:label xml:lang="en">Water Conservation</rdfs:label>
    </owl:Class>
    


    <!-- http://www.semanticweb.org/cra/ontologies/AgriWaterMgmt#WaterEfficiency -->

    <owl:Class rdf:about="http://www.semanticweb.org/cra/ontologies/AgriWaterMgmt#WaterEfficiency">
        <owl:equivalentClass>
            <owl:Restriction>
                <owl:onProperty rdf:resource="http://www.semanticweb.org/cra/ontologies/AgriWaterMgmt#reduces"/>
                <owl:someValuesFrom rdf:resource="http://www.semanticweb.org/cra/ontologies/AgriWaterMgmt#CropWaterStress"/>
            </owl:Restriction>
        </owl:equivalentClass>
        <rdfs:subClassOf rdf:resource="http://www.semanticweb.org/cra/ontologies/AgriWaterMgmt#WaterManagement"/>
        <rdfs:comment xml:lang="en">Refers to the optimal use of water resources, ensuring that water is utilized in a manner that maximizes its utility while minimizing waste. Water efficiency is crucial for sustainable development and the preservation of water supplies.</rdfs:comment>
        <rdfs:label xml:lang="en">Water Efficiency</rdfs:label>
    </owl:Class>
    


    <!-- http://www.semanticweb.org/cra/ontologies/AgriWaterMgmt#WaterManagement -->

    <owl:Class rdf:about="http://www.semanticweb.org/cra/ontologies/AgriWaterMgmt#WaterManagement">
        <owl:equivalentClass>
            <owl:Restriction>
                <owl:onProperty rdf:resource="http://www.semanticweb.org/cra/ontologies/AgriWaterMgmt#allocates"/>
                <owl:someValuesFrom rdf:resource="http://www.semanticweb.org/cra/ontologies/AgriWaterMgmt#WaterResources"/>
            </owl:Restriction>
        </owl:equivalentClass>
        <rdfs:subClassOf rdf:resource="http://www.semanticweb.org/cra/ontologies/AgriWaterMgmt#Water"/>
        <rdfs:comment xml:lang="en">Water resource management is the activity of planning, developing, distributing and managing the optimum use of water resources.</rdfs:comment>
        <rdfs:label xml:lang="en">Water Management</rdfs:label>
    </owl:Class>
    


    <!-- http://www.semanticweb.org/cra/ontologies/AgriWaterMgmt#WaterOptimization -->

    <owl:Class rdf:about="http://www.semanticweb.org/cra/ontologies/AgriWaterMgmt#WaterOptimization">
        <rdfs:subClassOf rdf:resource="http://www.semanticweb.org/cra/ontologies/AgriWaterMgmt#WaterManagement"/>
        <rdfs:comment xml:lang="en">The process of managing and adjusting water resources in order to achieve maximum efficiency in usage, ensuring that the available water meets the needs of various sectors without compromising future availability.</rdfs:comment>
        <rdfs:label xml:lang="en">Water Optimization</rdfs:label>
    </owl:Class>
    


    <!-- http://www.semanticweb.org/cra/ontologies/AgriWaterMgmt#WaterPolicy -->

    <owl:Class rdf:about="http://www.semanticweb.org/cra/ontologies/AgriWaterMgmt#WaterPolicy">
        <rdfs:subClassOf rdf:resource="http://www.semanticweb.org/cra/ontologies/AgriWaterMgmt#WaterManagement"/>
        <rdfs:comment xml:lang="en">Refers to the laws, regulations, and guidelines set by governments or regulatory bodies to govern water use, distribution, and conservation. Effective water policies are essential for ensuring equitable access to water and protecting water resources.</rdfs:comment>
        <rdfs:label xml:lang="en">Water Policy</rdfs:label>
    </owl:Class>
    


    <!-- http://www.semanticweb.org/cra/ontologies/AgriWaterMgmt#WaterResources -->

    <owl:Class rdf:about="http://www.semanticweb.org/cra/ontologies/AgriWaterMgmt#WaterResources">
        <owl:equivalentClass>
            <owl:Restriction>
                <owl:onProperty rdf:resource="http://www.semanticweb.org/cra/ontologies/AgriWaterMgmt#isUsedIn"/>
                <owl:someValuesFrom rdf:resource="http://www.semanticweb.org/cra/ontologies/AgriWaterMgmt#IrrigationSystems"/>
            </owl:Restriction>
        </owl:equivalentClass>
        <rdfs:subClassOf rdf:resource="http://www.semanticweb.org/cra/ontologies/AgriWaterMgmt#Water"/>
        <rdfs:comment xml:lang="en">Water resources are natural resources of water that are potentially useful for humans, for example as a source of drinking water supply or irrigation water.</rdfs:comment>
        <rdfs:label>Water Resources</rdfs:label>
    </owl:Class>
    


    <!-- http://www.semanticweb.org/cra/ontologies/AgriWaterMgmt#WaterRights -->

    <owl:Class rdf:about="http://www.semanticweb.org/cra/ontologies/AgriWaterMgmt#WaterRights">
        <rdfs:subClassOf rdf:resource="http://www.semanticweb.org/cra/ontologies/AgriWaterMgmt#WaterManagement"/>
        <rdfs:comment xml:lang="en">Refers to the legal entitlements that individuals or organizations have regarding the use and access to water resources. Water rights regulate the allocation and usage of water in a manner that ensures fairness and sustainability.</rdfs:comment>
        <rdfs:label xml:lang="en">Water Rights</rdfs:label>
    </owl:Class>
    


    <!-- http://www.semanticweb.org/cra/ontologies/AgriWaterMgmt#WaterSensors -->

    <owl:Class rdf:about="http://www.semanticweb.org/cra/ontologies/AgriWaterMgmt#WaterSensors">
        <rdfs:subClassOf rdf:resource="http://www.semanticweb.org/cra/ontologies/AgriWaterMgmt#AgriculturalEngineering"/>
        <rdfs:comment xml:lang="en">Devices used to monitor and measure soil moisture, water levels, or other key parameters in agricultural water management systems to ensure precise water distribution and minimize waste.</rdfs:comment>
        <rdfs:label xml:lang="en">Water Sensors</rdfs:label>
    </owl:Class>
    


    <!-- http://www.semanticweb.org/cra/ontologies/AgriWaterMgmt#WaterUse -->

    <owl:Class rdf:about="http://www.semanticweb.org/cra/ontologies/AgriWaterMgmt#WaterUse">
        <rdfs:subClassOf rdf:resource="http://www.semanticweb.org/cra/ontologies/AgriWaterMgmt#WaterManagement"/>
        <rdfs:comment xml:lang="en">Refers to the various ways water is utilized, including domestic, agricultural, industrial, and environmental purposes. Efficient and sustainable water use is key to managing the growing demand for water resources.</rdfs:comment>
        <rdfs:label xml:lang="en">Water Use</rdfs:label>
    </owl:Class>
    


    <!-- http://www.semanticweb.org/cra/ontologies/AgriWaterMgmt#WeatherCondition -->

    <owl:Class rdf:about="http://www.semanticweb.org/cra/ontologies/AgriWaterMgmt#WeatherCondition">
        <rdfs:subClassOf rdf:resource="http://www.semanticweb.org/cra/ontologies/AgriWaterMgmt#Water"/>
        <rdfs:comment xml:lang="en">The atmospheric conditions that comprise the state of the atmosphere in terms of temperature and wind and clouds and precipitation.</rdfs:comment>
        <rdfs:label xml:lang="en">Weather Conditions</rdfs:label>
    </owl:Class>
    


    <!-- 
    ///////////////////////////////////////////////////////////////////////////////////////
    //
    // Individuals
    //
    ///////////////////////////////////////////////////////////////////////////////////////
     -->

    


    <!-- http://www.semanticweb.org/cra/ontologies/AgriWaterMgmt#Bend -->

    <owl:NamedIndividual rdf:about="http://www.semanticweb.org/cra/ontologies/AgriWaterMgmt#Bend">
        <rdf:type rdf:resource="http://www.semanticweb.org/cra/ontologies/AgriWaterMgmt#Accessories"/>
    </owl:NamedIndividual>
    


    <!-- http://www.semanticweb.org/cra/ontologies/AgriWaterMgmt#ButterflyValve -->

    <owl:NamedIndividual rdf:about="http://www.semanticweb.org/cra/ontologies/AgriWaterMgmt#ButterflyValve">
        <rdf:type rdf:resource="http://www.semanticweb.org/cra/ontologies/AgriWaterMgmt#Accessories"/>
    </owl:NamedIndividual>
    


    <!-- http://www.semanticweb.org/cra/ontologies/AgriWaterMgmt#Couplings -->

    <owl:NamedIndividual rdf:about="http://www.semanticweb.org/cra/ontologies/AgriWaterMgmt#Couplings">
        <rdf:type rdf:resource="http://www.semanticweb.org/cra/ontologies/AgriWaterMgmt#Accessories"/>
    </owl:NamedIndividual>
    


    <!-- http://www.semanticweb.org/cra/ontologies/AgriWaterMgmt#DripIrrigationSystem_Australia -->

    <owl:NamedIndividual rdf:about="http://www.semanticweb.org/cra/ontologies/AgriWaterMgmt#DripIrrigationSystem_Australia">
        <rdf:type rdf:resource="http://www.semanticweb.org/cra/ontologies/AgriWaterMgmt#DripIrrigation"/>
    </owl:NamedIndividual>
    


    <!-- http://www.semanticweb.org/cra/ontologies/AgriWaterMgmt#DripIrrigationSystem_Israel -->

    <owl:NamedIndividual rdf:about="http://www.semanticweb.org/cra/ontologies/AgriWaterMgmt#DripIrrigationSystem_Israel">
        <rdf:type rdf:resource="http://www.semanticweb.org/cra/ontologies/AgriWaterMgmt#DripIrrigation"/>
    </owl:NamedIndividual>
    


    <!-- http://www.semanticweb.org/cra/ontologies/AgriWaterMgmt#Elbows -->

    <owl:NamedIndividual rdf:about="http://www.semanticweb.org/cra/ontologies/AgriWaterMgmt#Elbows">
        <rdf:type rdf:resource="http://www.semanticweb.org/cra/ontologies/AgriWaterMgmt#Accessories"/>
    </owl:NamedIndividual>
    


    <!-- http://www.semanticweb.org/cra/ontologies/AgriWaterMgmt#FertilizerApplicator -->

    <owl:NamedIndividual rdf:about="http://www.semanticweb.org/cra/ontologies/AgriWaterMgmt#FertilizerApplicator">
        <rdf:type rdf:resource="http://www.semanticweb.org/cra/ontologies/AgriWaterMgmt#Accessories"/>
    </owl:NamedIndividual>
    


    <!-- http://www.semanticweb.org/cra/ontologies/AgriWaterMgmt#Flange -->

    <owl:NamedIndividual rdf:about="http://www.semanticweb.org/cra/ontologies/AgriWaterMgmt#Flange">
        <rdf:type rdf:resource="http://www.semanticweb.org/cra/ontologies/AgriWaterMgmt#Accessories"/>
    </owl:NamedIndividual>
    


    <!-- http://www.semanticweb.org/cra/ontologies/AgriWaterMgmt#Hydrants -->

    <owl:NamedIndividual rdf:about="http://www.semanticweb.org/cra/ontologies/AgriWaterMgmt#Hydrants">
        <rdf:type rdf:resource="http://www.semanticweb.org/cra/ontologies/AgriWaterMgmt#Accessories"/>
    </owl:NamedIndividual>
    


    <!-- http://www.semanticweb.org/cra/ontologies/AgriWaterMgmt#Nipple -->

    <owl:NamedIndividual rdf:about="http://www.semanticweb.org/cra/ontologies/AgriWaterMgmt#Nipple">
        <rdf:type rdf:resource="http://www.semanticweb.org/cra/ontologies/AgriWaterMgmt#Accessories"/>
    </owl:NamedIndividual>
    


    <!-- http://www.semanticweb.org/cra/ontologies/AgriWaterMgmt#Plugs -->

    <owl:NamedIndividual rdf:about="http://www.semanticweb.org/cra/ontologies/AgriWaterMgmt#Plugs">
        <rdf:type rdf:resource="http://www.semanticweb.org/cra/ontologies/AgriWaterMgmt#Accessories"/>
    </owl:NamedIndividual>
    


    <!-- http://www.semanticweb.org/cra/ontologies/AgriWaterMgmt#PressureGauge -->

    <owl:NamedIndividual rdf:about="http://www.semanticweb.org/cra/ontologies/AgriWaterMgmt#PressureGauge">
        <rdf:type rdf:resource="http://www.semanticweb.org/cra/ontologies/AgriWaterMgmt#Accessories"/>
    </owl:NamedIndividual>
    


    <!-- http://www.semanticweb.org/cra/ontologies/AgriWaterMgmt#Reducers -->

    <owl:NamedIndividual rdf:about="http://www.semanticweb.org/cra/ontologies/AgriWaterMgmt#Reducers">
        <rdf:type rdf:resource="http://www.semanticweb.org/cra/ontologies/AgriWaterMgmt#Accessories"/>
    </owl:NamedIndividual>
    


    <!-- http://www.semanticweb.org/cra/ontologies/AgriWaterMgmt#Tees -->

    <owl:NamedIndividual rdf:about="http://www.semanticweb.org/cra/ontologies/AgriWaterMgmt#Tees">
        <rdf:type rdf:resource="http://www.semanticweb.org/cra/ontologies/AgriWaterMgmt#Accessories"/>
    </owl:NamedIndividual>
    


    <!-- http://www.semanticweb.org/cra/ontologies/AgriWaterMgmt#WaterMeters -->

    <owl:NamedIndividual rdf:about="http://www.semanticweb.org/cra/ontologies/AgriWaterMgmt#WaterMeters">
        <rdf:type rdf:resource="http://www.semanticweb.org/cra/ontologies/AgriWaterMgmt#Accessories"/>
    </owl:NamedIndividual>
    


    <!-- 
    ///////////////////////////////////////////////////////////////////////////////////////
    //
    // General axioms
    //
    ///////////////////////////////////////////////////////////////////////////////////////
     -->

    <rdf:Description>
        <rdf:type rdf:resource="http://www.w3.org/2002/07/owl#AllDisjointClasses"/>
        <owl:members rdf:parseType="Collection">
            <rdf:Description rdf:about="http://www.semanticweb.org/cra/ontologies/AgriWaterMgmt#AgriculturalEngineering"/>
            <rdf:Description rdf:about="http://www.semanticweb.org/cra/ontologies/AgriWaterMgmt#Crops"/>
            <rdf:Description rdf:about="http://www.semanticweb.org/cra/ontologies/AgriWaterMgmt#IrrigationSystems"/>
            <rdf:Description rdf:about="http://www.semanticweb.org/cra/ontologies/AgriWaterMgmt#SoilManagement"/>
            <rdf:Description rdf:about="http://www.semanticweb.org/cra/ontologies/AgriWaterMgmt#SustainabilityAndEnvironmentalImpact"/>
            <rdf:Description rdf:about="http://www.semanticweb.org/cra/ontologies/AgriWaterMgmt#WaterManagement"/>
            <rdf:Description rdf:about="http://www.semanticweb.org/cra/ontologies/AgriWaterMgmt#WaterResources"/>
            <rdf:Description rdf:about="http://www.semanticweb.org/cra/ontologies/AgriWaterMgmt#WeatherCondition"/>
        </owl:members>
    </rdf:Description>
    <rdf:Description>
        <rdf:type rdf:resource="http://www.w3.org/2002/07/owl#AllDisjointClasses"/>
        <owl:members rdf:parseType="Collection">
            <rdf:Description rdf:about="http://www.semanticweb.org/cra/ontologies/AgriWaterMgmt#WaterConservation"/>
            <rdf:Description rdf:about="http://www.semanticweb.org/cra/ontologies/AgriWaterMgmt#WaterEfficiency"/>
            <rdf:Description rdf:about="http://www.semanticweb.org/cra/ontologies/AgriWaterMgmt#WaterOptimization"/>
            <rdf:Description rdf:about="http://www.semanticweb.org/cra/ontologies/AgriWaterMgmt#WaterPolicy"/>
            <rdf:Description rdf:about="http://www.semanticweb.org/cra/ontologies/AgriWaterMgmt#WaterRights"/>
            <rdf:Description rdf:about="http://www.semanticweb.org/cra/ontologies/AgriWaterMgmt#WaterUse"/>
        </owl:members>
    </rdf:Description>
    <rdf:Description>
        <rdf:type rdf:resource="http://www.w3.org/2002/07/owl#AllDisjointClasses"/>
        <owl:members rdf:parseType="Collection">
            <rdf:Description rdf:about="http://www.semanticweb.org/cra/ontologies/AgriWaterMgmt#WaterConservation"/>
            <rdf:Description rdf:about="http://www.semanticweb.org/cra/ontologies/AgriWaterMgmt#WaterEfficiency"/>
            <rdf:Description rdf:about="http://www.semanticweb.org/cra/ontologies/AgriWaterMgmt#WaterPolicy"/>
            <rdf:Description rdf:about="http://www.semanticweb.org/cra/ontologies/AgriWaterMgmt#WaterRights"/>
        </owl:members>
    </rdf:Description>
</rdf:RDF>



<!-- Generated by the OWL API (version 4.5.29.2024-05-13T12:11:03Z) https://github.com/owlcs/owlapi -->

